<rdf:RDF xmlns:www="http://www.people#" xmlns:skos="http://www.w3.org/2004/02/skos/core#" xmlns:ns1="http://www.semanticweb.org/OntEur#" xmlns:society="http://www.semanticweb.org/society#" xmlns:rdfs="http://www.w3.org/2000/01/rdf-schema#" xmlns:owl="http://www.w3.org/2002/07/owl#" xmlns:rdf="http://www.w3.org/1999/02/22-rdf-syntax-ns#" xml:base="http://www.semanticweb.org/society_merged"><owl:Ontology rdf:about="http://www.semanticweb.org/society_merged"/><owl:ObjectProperty rdf:about="http://www.semanticweb.org/society#born_in"><rdfs:domain rdf:resource="http://www.semanticweb.org/society#people"/><rdfs:range rdf:resource="http://www.semanticweb.org/society#city"/></owl:ObjectProperty><owl:ObjectProperty rdf:about="http://www.semanticweb.org/society#is"><rdfs:domain rdf:resource="http://www.semanticweb.org/society#people"/><rdfs:range rdf:resource="http://www.semanticweb.org/society#status"/></owl:ObjectProperty><owl:ObjectProperty rdf:about="http://www.semanticweb.org/society#work_as"><rdfs:domain rdf:resource="http://www.semanticweb.org/society#people"/><rdfs:range rdf:resource="http://www.semanticweb.org/society#jobs"/></owl:ObjectProperty><owl:Class rdf:about="http://www.semanticweb.org/society#city"/><owl:Class rdf:about="http://www.semanticweb.org/society#jobs"/><owl:Class rdf:about="http://www.semanticweb.org/society#status"/><owl:NamedIndividual rdf:about="http://www.semanticweb.org/society#ajaccio"><rdf:type rdf:resource="http://www.semanticweb.org/society#city"/></owl:NamedIndividual><owl:NamedIndividual rdf:about="http://www.semanticweb.org/society#napoleone"><rdf:type rdf:resource="http://www.semanticweb.org/society#people"/><society:born_in rdf:resource="http://www.semanticweb.org/society#ajaccio"/></owl:NamedIndividual><owl:Class rdf:about="http://www.semanticweb.org/society#people"><owl:equivalentClass rdf:resource="http://www.people#People"/></owl:Class><owl:NamedIndividual rdf:about="http://www.semanticweb.org/OntEur#calzamaglia_antica"><rdf:type rdf:resource="http://thesaurus.europeanafashion.eu/thesaurus/10290"/><ns1:made_of rdf:resource="http://www.semanticweb.org/OntEur#wool"/></owl:NamedIndividual><owl:NamedIndividual rdf:about="http://www.semanticweb.org/OntEur#cotton"><rdf:type rdf:resource="http://thesaurus.europeanafashion.eu/thesaurus/10354"/></owl:NamedIndividual><owl:NamedIndividual rdf:about="http://www.semanticweb.org/OntEur#gonna_antica"><rdf:type rdf:resource="http://thesaurus.europeanafashion.eu/thesaurus/10864"/><ns1:made_of rdf:resource="http://www.semanticweb.org/OntEur#silk"/></owl:NamedIndividual><owl:NamedIndividual rdf:about="http://www.semanticweb.org/OntEur#silk"><rdf:type rdf:resource="http://thesaurus.europeanafashion.eu/thesaurus/10352"/></owl:NamedIndividual><owl:NamedIndividual rdf:about="http://www.semanticweb.org/OntEur#wool"><rdf:type rdf:resource="http://thesaurus.europeanafashion.eu/thesaurus/10351"/></owl:NamedIndividual><owl:Class rdf:about="http://thesaurus.europeanafashion.eu/thesaurus/10347"><rdfs:subClassOf rdf:resource="http://thesaurus.europeanafashion.eu/thesaurus/10346"/><rdfs:label xml:lang="de">Naturfasern</rdfs:label><rdfs:label xml:lang="pt">fibras naturais</rdfs:label><rdfs:label xml:lang="es">fibras naturales</rdfs:label><rdfs:label xml:lang="it">fibre naturali</rdfs:label><rdfs:label xml:lang="fr">fibres naturelles</rdfs:label><rdfs:label xml:lang="en">natural fibres</rdfs:label><rdfs:label xml:lang="sv">naturfiber</rdfs:label><rdfs:label xml:lang="nl">natuurlijke vezels</rdfs:label><rdfs:label xml:lang="nl">natuurvezel</rdfs:label><rdfs:label xml:lang="sr">prirodna vlakna</rdfs:label><rdfs:label xml:lang="el">φυσικές ίνες</rdfs:label><rdfs:label xml:lang="he">סיבים טבעיים</rdfs:label><skos:exactMatch rdf:resource="http://vocab.getty.edu/aat/300014027"/><skos:scopeNote xml:lang="en">Fiber obtained from an animal, vegetable, or mineral source used for conversion into non-woven fabrics (felt, paper) or woven cloth. (AAT)</skos:scopeNote></owl:Class><owl:Class rdf:about="http://thesaurus.europeanafashion.eu/thesaurus/10358"><rdfs:subClassOf rdf:resource="http://thesaurus.europeanafashion.eu/thesaurus/10346"/><rdfs:label xml:lang="de">chemische Fasern</rdfs:label><rdfs:label xml:lang="nl">chemische vezels</rdfs:label><rdfs:label xml:lang="es">fibras químicas</rdfs:label><rdfs:label xml:lang="pt">fibras químicas</rdfs:label><rdfs:label xml:lang="it">fibre chimiche</rdfs:label><rdfs:label xml:lang="fr">fibres chimiques</rdfs:label><rdfs:label xml:lang="sr">hemijska vlakna</rdfs:label><rdfs:label xml:lang="en">manmade fibres</rdfs:label><rdfs:label xml:lang="sv">regenererade fibrer</rdfs:label><rdfs:label xml:lang="nl">synthetische vezels</rdfs:label><rdfs:label xml:lang="el">χημικές ίνες</rdfs:label><rdfs:label xml:lang="he">סיבים כימיים</rdfs:label></owl:Class><owl:Class rdf:about="http://thesaurus.europeanafashion.eu/thesaurus/10543"><rdfs:subClassOf rdf:resource="http://thesaurus.europeanafashion.eu/thesaurus/10346"/><rdfs:label xml:lang="de">Materialien zur Dekoration, Besatz und technischen Ausrüstung</rdfs:label><rdfs:label xml:lang="sv">material för dekoration och applikation</rdfs:label><rdfs:label xml:lang="nl">materialen voor decoratie, applicatie en technische afwerking</rdfs:label><rdfs:label xml:lang="es">materiales para decoración, aplicación y acabados técnicos</rdfs:label><rdfs:label xml:lang="it">materiali per decorazione, applicazione e rifinitura tecnica</rdfs:label><rdfs:label xml:lang="en">materials for decoration, application and finishing</rdfs:label><rdfs:label xml:lang="sr">materijali za ukrašavanje, aplikaciju i tehničku doradu</rdfs:label><rdfs:label xml:lang="fr">matériaux pour pour la décoration, l'application et les finitions</rdfs:label><rdfs:label xml:lang="el">υλικά διακοσμητικά, επίθετα και για φινίρισμα</rdfs:label><rdfs:label xml:lang="he">חומרים לקישוט, יישום וגימור טכני</rdfs:label></owl:Class><owl:Class rdf:about="http://thesaurus.europeanafashion.eu/thesaurus/10348"><rdfs:subClassOf rdf:resource="http://thesaurus.europeanafashion.eu/thesaurus/10347"/><rdfs:label xml:lang="de">Fasern mineralischen Ursprungs</rdfs:label><rdfs:label xml:lang="pt">fibras de origem mineral</rdfs:label><rdfs:label xml:lang="es">fibras de origen mineral</rdfs:label><rdfs:label xml:lang="it">fibre di origine minerale</rdfs:label><rdfs:label xml:lang="fr">fibres d'origines minérales</rdfs:label><rdfs:label xml:lang="en">mineral fibres</rdfs:label><rdfs:label xml:lang="nl">minerale vezels</rdfs:label><rdfs:label xml:lang="sv">mineralfibrer</rdfs:label><rdfs:label xml:lang="nl">vezels van minerale oorsprong</rdfs:label><rdfs:label xml:lang="sr">vlakna mineralnog porekla</rdfs:label><rdfs:label xml:lang="el">ίνες μεταλλικές</rdfs:label><rdfs:label xml:lang="he">סיבים מינרליים מקוריים</rdfs:label></owl:Class><owl:Class rdf:about="http://thesaurus.europeanafashion.eu/thesaurus/10350"><rdfs:subClassOf rdf:resource="http://thesaurus.europeanafashion.eu/thesaurus/10347"/><rdfs:label xml:lang="de">Fasern tierischen Ursprungs</rdfs:label><rdfs:label xml:lang="en">animal fibres</rdfs:label><rdfs:label xml:lang="sv">animaliska fibrer</rdfs:label><rdfs:label xml:lang="nl">dierlijke vezels</rdfs:label><rdfs:label xml:lang="pt">fibras de origem animal</rdfs:label><rdfs:label xml:lang="es">fibras de origen animal</rdfs:label><rdfs:label xml:lang="it">fibre di origine animale</rdfs:label><rdfs:label xml:lang="fr">fibres d'origine animale</rdfs:label><rdfs:label xml:lang="nl">vezels van dierlijke oorsprong</rdfs:label><rdfs:label xml:lang="sr">vlakna životinjskog porekla</rdfs:label><rdfs:label xml:lang="el">ίνες ζωικής προέλευσης</rdfs:label><rdfs:label xml:lang="he">סיבים מבעלי חיים</rdfs:label><skos:exactMatch rdf:resource="http://vocab.getty.edu/aat/300386673"/><skos:scopeNote xml:lang="en">Any fiber obtained from animal sources., for example sheep wool, alpaca, mohair, angora, and silk. In general, animal fibers do not burn as readily as vegetable fibers, but instead tend to char and emit mildly nitrogenous odors characteristic of burnt hair. Except for silk, all animal fibers can be microscopically characterized by their tiny surface scales and center shaft. (AAT)</skos:scopeNote></owl:Class><owl:Class rdf:about="http://thesaurus.europeanafashion.eu/thesaurus/10353"><rdfs:subClassOf rdf:resource="http://thesaurus.europeanafashion.eu/thesaurus/10347"/><rdfs:label xml:lang="de">Pflanzenfasern</rdfs:label><rdfs:label xml:lang="pt">fibras de origem vegetal</rdfs:label><rdfs:label xml:lang="es">fibras de origen vegetal</rdfs:label><rdfs:label xml:lang="it">fibre di origine vegetale</rdfs:label><rdfs:label xml:lang="fr">fibres d'origine végétale</rdfs:label><rdfs:label xml:lang="nl">plantaardige vezels</rdfs:label><rdfs:label xml:lang="sv">vegetabiliska fibrer</rdfs:label><rdfs:label xml:lang="en">vegetable fibres</rdfs:label><rdfs:label xml:lang="nl">vezels van plantaardige oorsprong</rdfs:label><rdfs:label xml:lang="sr">vlakna biljnog porekla</rdfs:label><rdfs:label xml:lang="el">ίνες φυτικής προέλευσης</rdfs:label><rdfs:label xml:lang="he">סיבים צמחיים</rdfs:label><skos:exactMatch rdf:resource="http://vocab.getty.edu/aat/300014031"/><skos:scopeNote xml:lang="en">Natural fiber made from plant material, often used in papermaking. (AAT)</skos:scopeNote></owl:Class><owl:Class rdf:about="http://thesaurus.europeanafashion.eu/thesaurus/10472"><rdfs:subClassOf rdf:resource="http://thesaurus.europeanafashion.eu/thesaurus/10348"/><rdfs:label xml:lang="de">Asbest</rdfs:label><rdfs:label xml:lang="fr">amiante</rdfs:label><rdfs:label xml:lang="es">amianto</rdfs:label><rdfs:label xml:lang="it">amianto</rdfs:label><rdfs:label xml:lang="pt">amianto</rdfs:label><rdfs:label xml:lang="nl">asbest</rdfs:label><rdfs:label xml:lang="sv">asbest</rdfs:label><rdfs:label xml:lang="en">asbestos</rdfs:label><rdfs:label xml:lang="es">asbestos</rdfs:label><rdfs:label xml:lang="sr">azbest</rdfs:label><rdfs:label xml:lang="el">αμίαντος</rdfs:label><rdfs:label xml:lang="he">אזבסט</rdfs:label><skos:exactMatch rdf:resource="http://vocab.getty.edu/aat/300011071"/><skos:scopeNote xml:lang="en">A commercial term for any of several fibrous magnesium silicate minerals readily separable into thin, strong fiber that is flexible, noncombustible, heat resistant, and chemically inert; used in a wide variety of industrial products. It was used by the ancient Greeks, Egyptians, and Chinese as a fireproof material. In the 19th and early 20th centuries, asbestos was used for fireproofing and insulating houses: small asbestos fibers were mixed with binders and compressed into boards, paper, pipe covering, ironing board covers, shingles, tiles, and sprayed onto ceilings. Long asbestos fibers were woven into fabrics for used in brake linings, heat-resistant shields, gloves, and fireproof garments and blankets. Health concerns have limited the use of asbestos since the early 1960s. In the U.S., it was declared a hazardous material in 1986. (AAT)</skos:scopeNote></owl:Class><owl:Class rdf:about="http://thesaurus.europeanafashion.eu/thesaurus/10545"><rdfs:subClassOf rdf:resource="http://thesaurus.europeanafashion.eu/thesaurus/10348"/><rdfs:label xml:lang="de">Metall</rdfs:label><rdfs:label xml:lang="nl">metaal</rdfs:label><rdfs:label xml:lang="en">metal</rdfs:label><rdfs:label xml:lang="es">metal</rdfs:label><rdfs:label xml:lang="sr">metal</rdfs:label><rdfs:label xml:lang="sv">metall</rdfs:label><rdfs:label xml:lang="it">metallo</rdfs:label><rdfs:label xml:lang="fr">métal</rdfs:label><rdfs:label xml:lang="el">μέταλλο</rdfs:label><rdfs:label xml:lang="he">מתכת</rdfs:label><skos:exactMatch rdf:resource="http://vocab.getty.edu/aat/300010900"/><skos:scopeNote xml:lang="en">Any of a large group of substances that typically show a characteristic luster, are good conductors of electricity and heat, are opaque, can be fused, and are usually malleable or ductile. (AAT)</skos:scopeNote></owl:Class><owl:Class rdf:about="http://thesaurus.europeanafashion.eu/thesaurus/10557"><rdfs:subClassOf rdf:resource="http://thesaurus.europeanafashion.eu/thesaurus/10348"/><rdfs:label xml:lang="de">Glas</rdfs:label><rdfs:label xml:lang="nl">glas</rdfs:label><rdfs:label xml:lang="sv">glas</rdfs:label><rdfs:label xml:lang="en">glass</rdfs:label><rdfs:label xml:lang="sr">staklo</rdfs:label><rdfs:label xml:lang="fr">verre</rdfs:label><rdfs:label xml:lang="it">vetro</rdfs:label><rdfs:label xml:lang="es">vidrio</rdfs:label><rdfs:label xml:lang="el">γυαλί</rdfs:label><rdfs:label xml:lang="he">זכוכית</rdfs:label><skos:exactMatch rdf:resource="http://vocab.getty.edu/aat/300010797"/><skos:scopeNote xml:lang="en">An amorphous, inorganic substance made by fusing silica (silicon dioxide) with a basic oxide; generally transparent but often translucent or opaque. Its characteristic properties are its hardness and rigidity at ordinary temperatures, its capacity for plastic working at elevated temperatures, and its resistance to weathering and to most chemicals except hydrofluoric acid. Used for both utilitarian and decorative purposes, it can be formed into various shapes, colored or decorated. Glass originated as a glaze in Mesopotamia in about 3500 BCE and the first objects made wholly of glass date to about 2500 BCE. (AAT)</skos:scopeNote></owl:Class><owl:Class rdf:about="http://thesaurus.europeanafashion.eu/thesaurus/10558"><rdfs:subClassOf rdf:resource="http://thesaurus.europeanafashion.eu/thesaurus/10348"/><rdfs:label xml:lang="de">Spiegel</rdfs:label><rdfs:label xml:lang="es">espejo</rdfs:label><rdfs:label xml:lang="fr">miroir</rdfs:label><rdfs:label xml:lang="en">mirror</rdfs:label><rdfs:label xml:lang="sr">ogledalo</rdfs:label><rdfs:label xml:lang="it">specchio</rdfs:label><rdfs:label xml:lang="sv">spegelgals</rdfs:label><rdfs:label xml:lang="nl">spiegel</rdfs:label><rdfs:label xml:lang="el">καθρέφτης</rdfs:label><rdfs:label xml:lang="he">ראי / מראה</rdfs:label><skos:exactMatch rdf:resource="http://vocab.getty.edu/aat/300037682"/><skos:scopeNote xml:lang="en">Objects with a highly polished surface, often framed, which are designed to reflect images. (AAT)</skos:scopeNote></owl:Class><owl:Class rdf:about="http://thesaurus.europeanafashion.eu/thesaurus/10559"><rdfs:subClassOf rdf:resource="http://thesaurus.europeanafashion.eu/thesaurus/10348"/><rdfs:label xml:lang="de">Gummi</rdfs:label><rdfs:label xml:lang="de">Kautschuk</rdfs:label><rdfs:label xml:lang="fr">caoutchouc</rdfs:label><rdfs:label xml:lang="es">caucho</rdfs:label><rdfs:label xml:lang="es">goma</rdfs:label><rdfs:label xml:lang="it">gomma</rdfs:label><rdfs:label xml:lang="sr">guma</rdfs:label><rdfs:label xml:lang="sv">gummi</rdfs:label><rdfs:label xml:lang="en">rubber</rdfs:label><rdfs:label xml:lang="nl">rubber</rdfs:label><rdfs:label xml:lang="el">λάστιχο</rdfs:label><rdfs:label xml:lang="he">גומי</rdfs:label><skos:exactMatch rdf:resource="http://vocab.getty.edu/aat/300012941"/><skos:scopeNote xml:lang="en">A natural hydrocarbon polymer formed from the resinous latex of trees of the Hevea and Parthenium genera. To prepare natural rubber, the latex is collected from a cut in the bark, precipitated with acid, then washed and dried. Rubber is very elastic and was used for bowls, shoe soles, adhesives, and bouncy balls. However, when cooled, rubber becomes brittle and when warmed it becomes sweaty and tacky. Prior to the development of synthetic resins, unvulcanized rubber was used for adhesive tapes and crepe shoe soles. In 1839, Charles Goodyear discovered that rubber can be hardened with the vulcanization process in which sulfur is used to initiate crosslinking of the hydrocarbon strands. Higher sulfur content produces a harder, denser material. Vulcanized rubber is used to make rubber bands, foams, fabric coatings, small objects, combs, pens, and musical instruments. Vulcanized rubber, however, will emit sulfur when exposed to light or heat causing the rubber to degrade and become brittle. Since the 19th century, small amounts of wax have been added to the rubber during vulcanization. The wax slowly migrates to the surface and provides a thin layer of protection from oxidation. (AAT)</skos:scopeNote></owl:Class><owl:Class rdf:about="http://thesaurus.europeanafashion.eu/thesaurus/10561"><rdfs:subClassOf rdf:resource="http://thesaurus.europeanafashion.eu/thesaurus/10348"/><rdfs:label xml:lang="de">Stein</rdfs:label><rdfs:label xml:lang="sr">kamen</rdfs:label><rdfs:label xml:lang="es">piedra</rdfs:label><rdfs:label xml:lang="fr">pierre</rdfs:label><rdfs:label xml:lang="it">pietra</rdfs:label><rdfs:label xml:lang="nl">steen</rdfs:label><rdfs:label xml:lang="sv">sten</rdfs:label><rdfs:label xml:lang="en">stone</rdfs:label><rdfs:label xml:lang="el">πέτρα</rdfs:label><rdfs:label xml:lang="he">אבן</rdfs:label><skos:exactMatch rdf:resource="http://vocab.getty.edu/aat/300011176"/><skos:scopeNote xml:lang="en">General term for rock that has been cut, shaped, crushed, or otherwise formed for use in construction or other purposes. Includes the specific archaeological and anthropological sense of individual stones which may be decorated or ornamented and which may be used in ritual contexts. These are usually not carved or dressed, and so differ from sculptures made from stone. (AAT)</skos:scopeNote></owl:Class><owl:Class rdf:about="http://thesaurus.europeanafashion.eu/thesaurus/10564"><rdfs:subClassOf rdf:resource="http://thesaurus.europeanafashion.eu/thesaurus/10348"/><rdfs:label xml:lang="de">Gips</rdfs:label><rdfs:label xml:lang="es">escayola</rdfs:label><rdfs:label xml:lang="it">gesso</rdfs:label><rdfs:label xml:lang="nl">gips</rdfs:label><rdfs:label xml:lang="sr">gips</rdfs:label><rdfs:label xml:lang="sv">gips</rdfs:label><rdfs:label xml:lang="en">plaster</rdfs:label><rdfs:label xml:lang="nl">pleister</rdfs:label><rdfs:label xml:lang="fr">plâtre</rdfs:label><rdfs:label xml:lang="el">γύψος</rdfs:label><rdfs:label xml:lang="he">ג'ייד</rdfs:label><rdfs:label xml:lang="he">גבס</rdfs:label><skos:exactMatch rdf:resource="http://vocab.getty.edu/aat/300014922"/><skos:scopeNote xml:lang="en">Refers to a soft, plastic material that can be spread or daubed on a wall, ceiling, or other surface, where it afterwards hardens. In the context of art and architecture, it generally refers specifically to a mixture of water, lime, and sand, often combined with other materials, such as animal hair, to give the resulting material strength, texture, and if the surface is to be painted, porosity. (AAT)</skos:scopeNote></owl:Class><owl:Class rdf:about="http://thesaurus.europeanafashion.eu/thesaurus/10565"><rdfs:subClassOf rdf:resource="http://thesaurus.europeanafashion.eu/thesaurus/10348"/><rdfs:label xml:lang="de">Keramik</rdfs:label><rdfs:label xml:lang="it">ceramica</rdfs:label><rdfs:label xml:lang="en">ceramics</rdfs:label><rdfs:label xml:lang="es">cerámica</rdfs:label><rdfs:label xml:lang="fr">céramique</rdfs:label><rdfs:label xml:lang="nl">keramiek</rdfs:label><rdfs:label xml:lang="sv">keramik</rdfs:label><rdfs:label xml:lang="sr">keramika</rdfs:label><rdfs:label xml:lang="el">κεραμικά</rdfs:label><rdfs:label xml:lang="he">חרס</rdfs:label><rdfs:label xml:lang="he">קרמיקה</rdfs:label><skos:exactMatch rdf:resource="http://vocab.getty.edu/aat/300235507"/><skos:scopeNote xml:lang="en">Refers to any of various hard, brittle, heat-resistant and corrosion-resistant materials made by shaping and then firing a nonmetallic mineral, such as clay, at a high temperature. (AAT)</skos:scopeNote></owl:Class><owl:Class rdf:about="http://thesaurus.europeanafashion.eu/thesaurus/10567"><rdfs:subClassOf rdf:resource="http://thesaurus.europeanafashion.eu/thesaurus/10348"/><rdfs:label xml:lang="de">Speisestärke</rdfs:label><rdfs:label xml:lang="de">Stärke</rdfs:label><rdfs:label xml:lang="es">almidón</rdfs:label><rdfs:label xml:lang="it">amido</rdfs:label><rdfs:label xml:lang="pt">amido</rdfs:label><rdfs:label xml:lang="fr">amidon</rdfs:label><rdfs:label xml:lang="sr">skrob</rdfs:label><rdfs:label xml:lang="en">starch</rdfs:label><rdfs:label xml:lang="nl">stijfsel</rdfs:label><rdfs:label xml:lang="sv">stärkelse</rdfs:label><rdfs:label xml:lang="el">άμυλο</rdfs:label><rdfs:label xml:lang="he">עמילן</rdfs:label><skos:exactMatch rdf:resource="http://vocab.getty.edu/aat/300012959"/><skos:scopeNote xml:lang="en">Substance made of carbohydrate granules of varying sizes obtained from roots, bulbs, and seeds of most plants. Starch is primarily obtained from rice, wheat, corn, potatoes, cassava (tapioca), sago, and arrowroot. It is a mixture of the soluble straight-chain amylose molecules and the insoluble, branched-chain amylopectin molecules. When starch is heated, the granules swell and form a thick, tacky jelly upon cooling. Starchy adhesives have been used since at least 3500 BCE in Egypt. More recently starch has been used for sizing fabric, canvas, and paper, as an adhesive for paper cartons, bottle labels, gummed tape, and envelopes. Soluble starch has been used for priming canvas and as a binder in watercolor paints. Starch is sensitive to moisture and biodegradation. Starchy paste films become brittle with age. (AAT)</skos:scopeNote></owl:Class><owl:Class rdf:about="http://thesaurus.europeanafashion.eu/thesaurus/10569"><rdfs:subClassOf rdf:resource="http://thesaurus.europeanafashion.eu/thesaurus/10348"/><rdfs:label xml:lang="de">Glas</rdfs:label><rdfs:label xml:lang="de">Kristall</rdfs:label><rdfs:label xml:lang="de">Quarz</rdfs:label><rdfs:label xml:lang="es">cristal</rdfs:label><rdfs:label xml:lang="fr">cristal</rdfs:label><rdfs:label xml:lang="it">cristallo</rdfs:label><rdfs:label xml:lang="en">crystal</rdfs:label><rdfs:label xml:lang="nl">kristal</rdfs:label><rdfs:label xml:lang="sr">kristal</rdfs:label><rdfs:label xml:lang="sv">kristall</rdfs:label><rdfs:label xml:lang="el">κρύσταλλο</rdfs:label><rdfs:label xml:lang="he">בדולח</rdfs:label><skos:exactMatch rdf:resource="http://vocab.getty.edu/aat/300221157"/><skos:scopeNote xml:lang="en">A solid body having a characteristic internal structure and enclosed by systematically arranged plane surfaces. (AAT)</skos:scopeNote></owl:Class><owl:Class rdf:about="http://thesaurus.europeanafashion.eu/thesaurus/10570"><rdfs:subClassOf rdf:resource="http://thesaurus.europeanafashion.eu/thesaurus/10348"/><rdfs:label xml:lang="de">Emaille</rdfs:label><rdfs:label xml:lang="nl">email</rdfs:label><rdfs:label xml:lang="sr">emajl</rdfs:label><rdfs:label xml:lang="sv">emalj</rdfs:label><rdfs:label xml:lang="en">enamel</rdfs:label><rdfs:label xml:lang="es">esmalte</rdfs:label><rdfs:label xml:lang="it">smalto</rdfs:label><rdfs:label xml:lang="fr">émail</rdfs:label><rdfs:label xml:lang="el">σμάλτο</rdfs:label><rdfs:label xml:lang="he">אמייל</rdfs:label><skos:exactMatch rdf:resource="http://vocab.getty.edu/aat/300014910"/><skos:scopeNote xml:lang="en">A semi-transparent or opaque vitreous, porcelain-like coating applied by fusion to metal, glass, or ceramic, having a glossy appearance after hardening. Enamel is typically made from powdered fusible glasses (e.g., quartz, feldspar, clay, soda, and borax) and opaque colorants (e.g., cobalt blue, tin oxide) mixed with oil or water, then painted or sprayed on the object and fired up to 800 C. Enamel is used to protect a surface, to decorate objects in various colors and patterns, to form a surface for encaustic painting, and for other purposes. (AAT)</skos:scopeNote></owl:Class><owl:Class rdf:about="http://thesaurus.europeanafashion.eu/thesaurus/10764"><rdfs:subClassOf rdf:resource="http://thesaurus.europeanafashion.eu/thesaurus/10348"/><rdfs:label xml:lang="de">Bakelit</rdfs:label><rdfs:label xml:lang="de">Bakelite</rdfs:label><rdfs:label xml:lang="it">bachelite</rdfs:label><rdfs:label xml:lang="nl">bakeliet</rdfs:label><rdfs:label xml:lang="sr">bakelit</rdfs:label><rdfs:label xml:lang="sv">bakelit</rdfs:label><rdfs:label xml:lang="en">bakelite</rdfs:label><rdfs:label xml:lang="fr">bakelite</rdfs:label><rdfs:label xml:lang="es">baquelita</rdfs:label><rdfs:label xml:lang="el">βακελίτης</rdfs:label><rdfs:label xml:lang="he">בקליט</rdfs:label><skos:exactMatch rdf:resource="http://vocab.getty.edu/aat/300014544"/><skos:scopeNote xml:lang="en">The original trademarked name for phenol-formaldehyde resin, but now used to refer to a range of different types of plastic. The method for manufacturing the original resin was devised in 1909 by L. H. Baekeland in the United States, and the name Bakelite is a registered trademark of the Union Carbide Corporation. It is a hard, infusible, and chemically resistant plastic, nonconductor of electricity, and used in electrical appliances, industrial applications, in molding and casting operations, as an adhesive, in paints, and in baked-enamel coatings. (AAT)</skos:scopeNote></owl:Class><owl:Class rdf:about="http://thesaurus.europeanafashion.eu/thesaurus/10766"><rdfs:subClassOf rdf:resource="http://thesaurus.europeanafashion.eu/thesaurus/10348"/><rdfs:label xml:lang="en">Lucite</rdfs:label><rdfs:label xml:lang="fr">Lucite</rdfs:label><rdfs:label xml:lang="nl">Lucite</rdfs:label><rdfs:label xml:lang="it">Lucite® (polimetacrilato)</rdfs:label><rdfs:label xml:lang="de">Plexiglas®</rdfs:label><rdfs:label xml:lang="es">lucite</rdfs:label><rdfs:label xml:lang="sv">lucite</rdfs:label><rdfs:label xml:lang="sr">poli(metil metakrilat)</rdfs:label><rdfs:label xml:lang="es">vidrio acrílico</rdfs:label><rdfs:label xml:lang="el">λουσίτης</rdfs:label><rdfs:label xml:lang="he">פרספקס</rdfs:label><skos:exactMatch rdf:resource="http://vocab.getty.edu/aat/300014434"/><skos:scopeNote xml:lang="en">Methyl methacrylate made by E. I. du Pont de Nemours and Company, Inc., marketed in rolling powder and in rolls, tubes, and cast and molded sheets. (AAT)</skos:scopeNote></owl:Class><owl:Class rdf:about="http://thesaurus.europeanafashion.eu/thesaurus/11062"><rdfs:subClassOf rdf:resource="http://thesaurus.europeanafashion.eu/thesaurus/10348"/><rdfs:label xml:lang="de">Ton</rdfs:label><rdfs:label xml:lang="fr">argile</rdfs:label><rdfs:label xml:lang="it">argilla</rdfs:label><rdfs:label xml:lang="en">clay</rdfs:label><rdfs:label xml:lang="sr">glina</rdfs:label><rdfs:label xml:lang="nl">klei</rdfs:label><rdfs:label xml:lang="sv">lera</rdfs:label><rdfs:label xml:lang="el">πηλός</rdfs:label><rdfs:label xml:lang="he">חימר</rdfs:label><skos:exactMatch rdf:resource="http://vocab.getty.edu/aat/300010439"/><skos:scopeNote xml:lang="en">Naturally occurring sediments that are produced by chemical actions resulting during the weathering of rocks. It is often the term applied to all earths that form a paste with water and harden when heated. (AAT)</skos:scopeNote></owl:Class><owl:Class rdf:about="http://thesaurus.europeanafashion.eu/thesaurus/11064"><rdfs:subClassOf rdf:resource="http://thesaurus.europeanafashion.eu/thesaurus/10348"/><rdfs:label xml:lang="de">Glimmer</rdfs:label><rdfs:label xml:lang="sv">glimmer</rdfs:label><rdfs:label xml:lang="sr">liskun</rdfs:label><rdfs:label xml:lang="en">mica</rdfs:label><rdfs:label xml:lang="fr">mica</rdfs:label><rdfs:label xml:lang="it">mica</rdfs:label><rdfs:label xml:lang="nl">mica</rdfs:label><rdfs:label xml:lang="sr">tinjac</rdfs:label><rdfs:label xml:lang="el">μαρμαρυγίας</rdfs:label><rdfs:label xml:lang="he">מיקה</rdfs:label><skos:exactMatch rdf:resource="http://vocab.getty.edu/aat/300011124"/><skos:scopeNote xml:lang="en">Group of monoclinic minerals with perfect basal cleavage. (AAT)</skos:scopeNote></owl:Class><owl:Class rdf:about="http://thesaurus.europeanafashion.eu/thesaurus/10521"><rdfs:subClassOf rdf:resource="http://thesaurus.europeanafashion.eu/thesaurus/10545"/><rdfs:label xml:lang="de">Metallfaden</rdfs:label><rdfs:label xml:lang="de">Metallgespinstfaden</rdfs:label><rdfs:label xml:lang="fr">fil métallique</rdfs:label><rdfs:label xml:lang="it">filo di metallo</rdfs:label><rdfs:label xml:lang="es">hilo metálico</rdfs:label><rdfs:label xml:lang="nl">metaaldraad</rdfs:label><rdfs:label xml:lang="en">metal thread</rdfs:label><rdfs:label xml:lang="sv">metalltråd</rdfs:label><rdfs:label xml:lang="sr">metalna nit</rdfs:label><rdfs:label xml:lang="el">μεταλλική κλωστή</rdfs:label><rdfs:label xml:lang="he">חוטי מתכת</rdfs:label><skos:exactMatch rdf:resource="http://vocab.getty.edu/aat/300379384"/><skos:scopeNote xml:lang="en">Manufactured fiber made wholly or in part from metal. (AAT)</skos:scopeNote></owl:Class><owl:Class rdf:about="http://thesaurus.europeanafashion.eu/thesaurus/10546"><rdfs:subClassOf rdf:resource="http://thesaurus.europeanafashion.eu/thesaurus/10545"/><rdfs:label xml:lang="de">Gold</rdfs:label><rdfs:label xml:lang="en">gold</rdfs:label><rdfs:label xml:lang="nl">goud</rdfs:label><rdfs:label xml:lang="sv">guld</rdfs:label><rdfs:label xml:lang="fr">or</rdfs:label><rdfs:label xml:lang="es">oro</rdfs:label><rdfs:label xml:lang="it">oro</rdfs:label><rdfs:label xml:lang="pt">ouro</rdfs:label><rdfs:label xml:lang="sr">zlato</rdfs:label><rdfs:label xml:lang="el">χρυσός</rdfs:label><rdfs:label xml:lang="he">זהב</rdfs:label><skos:exactMatch rdf:resource="http://vocab.getty.edu/aat/300011021"/><skos:scopeNote xml:lang="en">Pure metallic element having symbol Au and atomic number 79; a soft, inert, shiny reddish yellow metal that is very malleable and ductile. Gold has been highly valued and found in artifacts dating to before 5000 BCE. Native gold, found in quartz veins (vein gold) and alluvial deposits (placer gold), generally contains some silver and copper. Gold is purified by dissolution in mercury or cyanide solutions, by melting, or by electrodeposition. The purity of commercial gold is expressed in karats which is the number of parts of gold in 24 parts of the alloy. Today gold is primarily used for monetary systems and for jewelry. (AAT)</skos:scopeNote></owl:Class><owl:Class rdf:about="http://thesaurus.europeanafashion.eu/thesaurus/10547"><rdfs:subClassOf rdf:resource="http://thesaurus.europeanafashion.eu/thesaurus/10545"/><rdfs:label xml:lang="de">Silber</rdfs:label><rdfs:label xml:lang="fr">argent</rdfs:label><rdfs:label xml:lang="it">argento</rdfs:label><rdfs:label xml:lang="es">plata</rdfs:label><rdfs:label xml:lang="pt">prata</rdfs:label><rdfs:label xml:lang="en">silver</rdfs:label><rdfs:label xml:lang="sv">silver</rdfs:label><rdfs:label xml:lang="sr">srebro</rdfs:label><rdfs:label xml:lang="nl">zilver</rdfs:label><rdfs:label xml:lang="el">ασήμι</rdfs:label><rdfs:label xml:lang="he">כסף</rdfs:label><skos:exactMatch rdf:resource="http://vocab.getty.edu/aat/300011029"/><skos:scopeNote xml:lang="en">Pure metallic element having symbol Ag and atomic number 47; a malleable, ductile, white metal with characteristic sheen, considered a precious metal. Silver is widely distributed throughout the world, occurring rarely as metallic silver (in Peru, Norway) but more often as silver-gold alloys and silver ore. Today silver is obtained as a byproduct in the refinement of gold, lead, copper, or zinc ores. Silver was smelted from the ore galena as early as 3800 BCE. As a pure metal, silver is second to gold in malleability and ductility, can be polished to a highly reflective surface, and used -- typically in an alloy -- in jewelry, coinage, photography, mirrors, electrical contacts, and tableware. (AAT)</skos:scopeNote></owl:Class><owl:Class rdf:about="http://thesaurus.europeanafashion.eu/thesaurus/10548"><rdfs:subClassOf rdf:resource="http://thesaurus.europeanafashion.eu/thesaurus/10545"/><rdfs:label xml:lang="de">Kupfer</rdfs:label><rdfs:label xml:lang="sr">bakar</rdfs:label><rdfs:label xml:lang="es">cobre</rdfs:label><rdfs:label xml:lang="pt">cobre</rdfs:label><rdfs:label xml:lang="en">copper</rdfs:label><rdfs:label xml:lang="fr">cuivre</rdfs:label><rdfs:label xml:lang="nl">koper</rdfs:label><rdfs:label xml:lang="sv">koppar</rdfs:label><rdfs:label xml:lang="it">rame</rdfs:label><rdfs:label xml:lang="el">χαλκός</rdfs:label><rdfs:label xml:lang="he">נחושת</rdfs:label><skos:exactMatch rdf:resource="http://vocab.getty.edu/aat/300011020"/><skos:scopeNote xml:lang="en">Pure metallic element having the symbol Cu and atomic number 29; a reddish brown, ductile metal that is present in the earth's crust, occurring as a native metal and as ores of sulfide, sulfate and carbonate (azurite, malachite, etc.). It was the first metal used by humans, probably from about 8000 BCE, in the regions of Mesopotamia and India. By about 3800 BCE copper was made into bronze for weapons and knives. Today, copper is one of the most widely used metals because it has high electrical and thermal conductivity, can be easily fabricated, is ductile and polishes well. In moist air, copper forms a protective green film of basic carbonate. Metallic copper combines well with other metals to form alloys, most commonly brass and bronze. Copper and its alloys are used for wire, electrical devices, pipes, cooking vessels, ammunition, ornamental trim, roofing, grillwork, coins, musical instruments, jewelry, and sculptures. (AAT)</skos:scopeNote></owl:Class><owl:Class rdf:about="http://thesaurus.europeanafashion.eu/thesaurus/10549"><rdfs:subClassOf rdf:resource="http://thesaurus.europeanafashion.eu/thesaurus/10545"/><rdfs:label xml:lang="de">Stahl</rdfs:label><rdfs:label xml:lang="it">acciaio</rdfs:label><rdfs:label xml:lang="es">acero</rdfs:label><rdfs:label xml:lang="fr">acier</rdfs:label><rdfs:label xml:lang="nl">staal</rdfs:label><rdfs:label xml:lang="en">steel</rdfs:label><rdfs:label xml:lang="sv">stål</rdfs:label><rdfs:label xml:lang="sr">čelik</rdfs:label><rdfs:label xml:lang="el">ατσάλι</rdfs:label><rdfs:label xml:lang="he">פלדה</rdfs:label><skos:exactMatch rdf:resource="http://vocab.getty.edu/aat/300133751"/><skos:scopeNote xml:lang="en">Any of various hard, strong, durable, malleable alloys of iron and carbon, often with other elements such as manganese, chromium, nickel, molybdenum, copper, tungsten, cobalt, or silicon; widely used as a structural material. (AAT)</skos:scopeNote></owl:Class><owl:Class rdf:about="http://thesaurus.europeanafashion.eu/thesaurus/10550"><rdfs:subClassOf rdf:resource="http://thesaurus.europeanafashion.eu/thesaurus/10545"/><rdfs:label xml:lang="de">Aluminium</rdfs:label><rdfs:label xml:lang="it">alluminio</rdfs:label><rdfs:label xml:lang="sr">aluminijum</rdfs:label><rdfs:label xml:lang="es">aluminio</rdfs:label><rdfs:label xml:lang="en">aluminium</rdfs:label><rdfs:label xml:lang="fr">aluminium</rdfs:label><rdfs:label xml:lang="nl">aluminium</rdfs:label><rdfs:label xml:lang="sv">aluminium</rdfs:label><rdfs:label xml:lang="en">aluminum</rdfs:label><rdfs:label xml:lang="el">αλουμίνιο</rdfs:label><rdfs:label xml:lang="he">אלומיניום</rdfs:label><skos:exactMatch rdf:resource="http://vocab.getty.edu/aat/300011015"/><skos:scopeNote xml:lang="en">Pure metallic element having symbol Al and atomic number 13; a hard, strong, silver white metal. This metal is also processed and formed, usually in combination with other substances, to make objects and materials. (AAT)</skos:scopeNote></owl:Class><owl:Class rdf:about="http://thesaurus.europeanafashion.eu/thesaurus/10551"><rdfs:subClassOf rdf:resource="http://thesaurus.europeanafashion.eu/thesaurus/10545"/><rdfs:label xml:lang="de">Zinn</rdfs:label><rdfs:label xml:lang="sr">beli lim</rdfs:label><rdfs:label xml:lang="es">estaño</rdfs:label><rdfs:label xml:lang="sr">kalaj</rdfs:label><rdfs:label xml:lang="it">stagno</rdfs:label><rdfs:label xml:lang="sv">tenn</rdfs:label><rdfs:label xml:lang="en">tin</rdfs:label><rdfs:label xml:lang="nl">tin</rdfs:label><rdfs:label xml:lang="fr">étain</rdfs:label><rdfs:label xml:lang="el">τσίγκος</rdfs:label><rdfs:label xml:lang="he">בדיל</rdfs:label><skos:exactMatch rdf:resource="http://vocab.getty.edu/aat/300133748"/><skos:scopeNote xml:lang="en">Pure metallic element having symbol Sn and atomic number 50; a soft, pliable, silvery white metal. Use also for this metal as processed and formed, usually in combination with other substances, to make various objects and materials. (AAT)</skos:scopeNote></owl:Class><owl:Class rdf:about="http://thesaurus.europeanafashion.eu/thesaurus/10552"><rdfs:subClassOf rdf:resource="http://thesaurus.europeanafashion.eu/thesaurus/10545"/><rdfs:label xml:lang="de">Eisen</rdfs:label><rdfs:label xml:lang="fr">fer</rdfs:label><rdfs:label xml:lang="it">ferro</rdfs:label><rdfs:label xml:lang="pt">ferro</rdfs:label><rdfs:label xml:lang="sr">gvožđe</rdfs:label><rdfs:label xml:lang="es">hierro</rdfs:label><rdfs:label xml:lang="nl">ijzer</rdfs:label><rdfs:label xml:lang="en">iron</rdfs:label><rdfs:label xml:lang="sv">järn</rdfs:label><rdfs:label xml:lang="el">σίδερο</rdfs:label><rdfs:label xml:lang="he">מגהץ</rdfs:label><skos:exactMatch rdf:resource="http://vocab.getty.edu/aat/300011002"/><skos:scopeNote xml:lang="en">Pure metallic element having symbol Fe and atomic number 26; metallic iron is silvery in color, lustrous, soft, ductile, malleable, and slightly magnetic; it rusts when exposed to moist air. It is rarely found as a native metal (telluric iron) except in meteorites (meteoric iron). Iron is most often found throughout the world as iron oxides (hematite, magnetite, limonite, and siderite) mixed with other ores. (AAT)</skos:scopeNote></owl:Class><owl:Class rdf:about="http://thesaurus.europeanafashion.eu/thesaurus/10553"><rdfs:subClassOf rdf:resource="http://thesaurus.europeanafashion.eu/thesaurus/10545"/><rdfs:label xml:lang="de">Blei</rdfs:label><rdfs:label xml:lang="sv">bly</rdfs:label><rdfs:label xml:lang="pt">chumbo</rdfs:label><rdfs:label xml:lang="en">lead</rdfs:label><rdfs:label xml:lang="nl">lood</rdfs:label><rdfs:label xml:lang="sr">olovo</rdfs:label><rdfs:label xml:lang="it">piombo</rdfs:label><rdfs:label xml:lang="fr">plomb</rdfs:label><rdfs:label xml:lang="es">plomo</rdfs:label><rdfs:label xml:lang="el">μόλυβδος</rdfs:label><rdfs:label xml:lang="he">עופרת</rdfs:label><skos:exactMatch rdf:resource="http://vocab.getty.edu/aat/300011022"/><skos:scopeNote xml:lang="en">Pure metallic element having symbol Pb and atomic number 82; soft, dense ductile metal of a dull gray color, shiny when freshly cut, occuring naturally most often as a sulfide in the mineral galena. Other lead minerals include anglesite (lead sulfate) and cerussite (lead carbonate). Native metallic lead was found and used from about 3600-2600 BCE when the technique for obtaining lead from roasting the sulfide ore (galena) was discovered. Lead was used to make small cast items such as coins and statuettes, plumbing pipes, spires, statues, cisterns, gargoyles, pigments (lead white, litharge, orange mineral, etc.), as a component in pottery glazes, for roofing, flashing, stained glass windows, as a soft solder, and as radiation shielding. (AAT)</skos:scopeNote></owl:Class><owl:Class rdf:about="http://thesaurus.europeanafashion.eu/thesaurus/10554"><rdfs:subClassOf rdf:resource="http://thesaurus.europeanafashion.eu/thesaurus/10545"/><rdfs:label xml:lang="de">Chrom</rdfs:label><rdfs:label xml:lang="en">chrome</rdfs:label><rdfs:label xml:lang="fr">chrome</rdfs:label><rdfs:label xml:lang="nl">chroom</rdfs:label><rdfs:label xml:lang="es">cromo</rdfs:label><rdfs:label xml:lang="it">cromo</rdfs:label><rdfs:label xml:lang="sr">hrom</rdfs:label><rdfs:label xml:lang="sv">krom</rdfs:label><rdfs:label xml:lang="el">χρώμιο</rdfs:label><rdfs:label xml:lang="he">כרום</rdfs:label><skos:exactMatch rdf:resource="http://vocab.getty.edu/aat/300011019"/><skos:scopeNote xml:lang="en">Pure metallic element having symbol Cr and atomic number 24; an extremely hard, silvery white metal with a bluish tinge. Use also for the metal as processed and formed, usually in combination with other substances, to make various objects and materials, notably stainless steel, heat-resistant alloy, high-strength alloy steel, and for wear-resistant electroplating. (AAT)</skos:scopeNote></owl:Class><owl:Class rdf:about="http://thesaurus.europeanafashion.eu/thesaurus/10555"><rdfs:subClassOf rdf:resource="http://thesaurus.europeanafashion.eu/thesaurus/10545"/><rdfs:label xml:lang="de">Messing</rdfs:label><rdfs:label xml:lang="es">azófar</rdfs:label><rdfs:label xml:lang="en">brass</rdfs:label><rdfs:label xml:lang="fr">laiton</rdfs:label><rdfs:label xml:lang="es">latón</rdfs:label><rdfs:label xml:lang="sr">mesing</rdfs:label><rdfs:label xml:lang="nl">messing</rdfs:label><rdfs:label xml:lang="sv">mässing</rdfs:label><rdfs:label xml:lang="it">ottone</rdfs:label><rdfs:label xml:lang="el">ορείχαλκος</rdfs:label><rdfs:label xml:lang="he">פליז</rdfs:label><skos:exactMatch rdf:resource="http://vocab.getty.edu/aat/300010946"/><skos:scopeNote xml:lang="en">Alloy of copper and zinc, usually with copper as the major alloying element and zinc up to 40&#37; by weight. (AAT)</skos:scopeNote></owl:Class><owl:Class rdf:about="http://thesaurus.europeanafashion.eu/thesaurus/10556"><rdfs:subClassOf rdf:resource="http://thesaurus.europeanafashion.eu/thesaurus/10545"/><rdfs:label xml:lang="de">Bronze</rdfs:label><rdfs:label xml:lang="es">bronce</rdfs:label><rdfs:label xml:lang="nl">brons</rdfs:label><rdfs:label xml:lang="sv">brons</rdfs:label><rdfs:label xml:lang="sr">bronza</rdfs:label><rdfs:label xml:lang="en">bronze</rdfs:label><rdfs:label xml:lang="fr">bronze</rdfs:label><rdfs:label xml:lang="it">bronzo</rdfs:label><rdfs:label xml:lang="el">μπρούντζος</rdfs:label><rdfs:label xml:lang="he">ברונזה</rdfs:label><skos:exactMatch rdf:resource="http://vocab.getty.edu/aat/300010957"/><skos:scopeNote xml:lang="en">Refers to a broad range of alloys of copper, specifically any non-ferrous alloy of copper, tin, and zinc or other trace metals. Bronze was made before 3,000 BCE -- possibly as early as 10,000 BCE, although its common use in tools and decorative items is dated only in later artifacts. The proportions of copper and tin vary widely, from 70 to 95 percent copper in surviving ancient artifacts. Because of the copper base, bronze may be very malleable and easy to work. By the Middle Ages in Europe, it was recognized that using the metals in certain proportions could yield specific properties. Some modern bronzes contain no tin at all, substituting other metals such as aluminum, manganese, and even zinc. Historically, the term was used interchangeably with latten. U.S. standard bronze is composed of 90&#37; copper, 7&#37; tin and 3&#37; zinc. Ancient bronze alloys sometimes contained up to 14&#37; tin. (AAT)</skos:scopeNote></owl:Class><owl:Class rdf:about="http://thesaurus.europeanafashion.eu/thesaurus/11055"><rdfs:subClassOf rdf:resource="http://thesaurus.europeanafashion.eu/thesaurus/10545"/><rdfs:label xml:lang="de">Metalllegierung</rdfs:label><rdfs:label xml:lang="fr">alliage</rdfs:label><rdfs:label xml:lang="en">alloy</rdfs:label><rdfs:label xml:lang="it">lega</rdfs:label><rdfs:label xml:lang="nl">legering</rdfs:label><rdfs:label xml:lang="sv">legering</rdfs:label><rdfs:label xml:lang="sr">legura</rdfs:label><rdfs:label xml:lang="el">κράμα</rdfs:label><rdfs:label xml:lang="he">סגסוגת</rdfs:label><skos:exactMatch rdf:resource="http://vocab.getty.edu/aat/300010902"/><skos:scopeNote xml:lang="en">Substance having metallic properties, consisting of two or more metallic elements or of metallic and nonmetallic elements, which are miscible with each other when molten, and do not separate into distinct layers when solid. (AAT)</skos:scopeNote></owl:Class><owl:Class rdf:about="http://thesaurus.europeanafashion.eu/thesaurus/11056"><rdfs:subClassOf rdf:resource="http://thesaurus.europeanafashion.eu/thesaurus/10545"/><rdfs:label xml:lang="de">Zinnober</rdfs:label><rdfs:label xml:lang="sr">cinabarit</rdfs:label><rdfs:label xml:lang="fr">cinabre</rdfs:label><rdfs:label xml:lang="it">cinabro</rdfs:label><rdfs:label xml:lang="en">cinnabar</rdfs:label><rdfs:label xml:lang="nl">cinnaber</rdfs:label><rdfs:label xml:lang="sv">cinnober</rdfs:label><rdfs:label xml:lang="el">κιννάβαρη</rdfs:label><rdfs:label xml:lang="he">צינובר</rdfs:label><skos:exactMatch rdf:resource="http://vocab.getty.edu/aat/300311452"/><skos:scopeNote xml:lang="en">A soft, dense, red, native ore composed of mercuric sulfide, found in deposits in veins near volcanic rocks or hot springs around the world. Cinnabar was mined in the Roman Empire for use as a pigment and for its mercury content; it has been the main source of mercury throughout the centuries. The toxic stone was also used for decoration and a talisman in Mayan tombs, as a colorant in Chinese carved lacquerware, in ink used by high officials in the Byzantine Empire, and other applications. Cinnabar is chemically identical to synthetic red mercuric sulfide, which is called vermilion. (AAT)</skos:scopeNote></owl:Class><owl:Class rdf:about="http://thesaurus.europeanafashion.eu/thesaurus/10349"><rdfs:subClassOf rdf:resource="http://thesaurus.europeanafashion.eu/thesaurus/10521"/><rdfs:label xml:lang="de">Goldfaden</rdfs:label><rdfs:label xml:lang="de">Goldgespinstfaden</rdfs:label><rdfs:label xml:lang="fr">fil d'or</rdfs:label><rdfs:label xml:lang="it">filo d'oro</rdfs:label><rdfs:label xml:lang="en">gold thread</rdfs:label><rdfs:label xml:lang="nl">gouddraad</rdfs:label><rdfs:label xml:lang="sv">guldtråd</rdfs:label><rdfs:label xml:lang="es">hilo de oro</rdfs:label><rdfs:label xml:lang="pt">ouro</rdfs:label><rdfs:label xml:lang="sr">zlatna nit</rdfs:label><rdfs:label xml:lang="el">χρυσοκλωστή</rdfs:label><rdfs:label xml:lang="he">חוט זהב (לתפירה)</rdfs:label></owl:Class><owl:Class rdf:about="http://thesaurus.europeanafashion.eu/thesaurus/10470"><rdfs:subClassOf rdf:resource="http://thesaurus.europeanafashion.eu/thesaurus/10521"/><rdfs:label xml:lang="de">Silberfaden</rdfs:label><rdfs:label xml:lang="de">Silbergespinstfaden</rdfs:label><rdfs:label xml:lang="fr">fil d'argent</rdfs:label><rdfs:label xml:lang="it">filo d'argento</rdfs:label><rdfs:label xml:lang="es">hilo de plata</rdfs:label><rdfs:label xml:lang="pt">prata</rdfs:label><rdfs:label xml:lang="en">silver thread</rdfs:label><rdfs:label xml:lang="sv">silvertråd</rdfs:label><rdfs:label xml:lang="sr">srebrna nit</rdfs:label><rdfs:label xml:lang="nl">zilverdraad</rdfs:label><rdfs:label xml:lang="el">ασημοκλωστή</rdfs:label><rdfs:label xml:lang="he">חוט (כסף)</rdfs:label></owl:Class><owl:Class rdf:about="http://thesaurus.europeanafashion.eu/thesaurus/10471"><rdfs:subClassOf rdf:resource="http://thesaurus.europeanafashion.eu/thesaurus/10521"/><rdfs:label xml:lang="de">Kupferfaden</rdfs:label><rdfs:label xml:lang="de">Kupfergespinstfaden</rdfs:label><rdfs:label xml:lang="sr">bakarna nit</rdfs:label><rdfs:label xml:lang="pt">cobre</rdfs:label><rdfs:label xml:lang="en">copper thread</rdfs:label><rdfs:label xml:lang="fr">fil de cuivre</rdfs:label><rdfs:label xml:lang="it">filo di rame</rdfs:label><rdfs:label xml:lang="es">hilo de cobre</rdfs:label><rdfs:label xml:lang="nl">koperdraad</rdfs:label><rdfs:label xml:lang="sv">koppartråd</rdfs:label><rdfs:label xml:lang="el">μπρούντζινο νήμα</rdfs:label><rdfs:label xml:lang="he">חוט נחושת</rdfs:label></owl:Class><owl:Class rdf:about="http://thesaurus.europeanafashion.eu/thesaurus/10474"><rdfs:subClassOf rdf:resource="http://thesaurus.europeanafashion.eu/thesaurus/10521"/><rdfs:label xml:lang="de">Stahlfaden</rdfs:label><rdfs:label xml:lang="de">Stahlgespinstfaden</rdfs:label><rdfs:label xml:lang="pt">aço</rdfs:label><rdfs:label xml:lang="fr">fil d'acier</rdfs:label><rdfs:label xml:lang="it">fil di ferro</rdfs:label><rdfs:label xml:lang="es">hilo de acero</rdfs:label><rdfs:label xml:lang="nl">staaldraad</rdfs:label><rdfs:label xml:lang="en">steel thread</rdfs:label><rdfs:label xml:lang="sv">ståltråd</rdfs:label><rdfs:label xml:lang="sr">čelična nit</rdfs:label><rdfs:label xml:lang="el">ατσαλόνημα</rdfs:label><rdfs:label xml:lang="he">חוט פלדה</rdfs:label></owl:Class><owl:Class rdf:about="http://thesaurus.europeanafashion.eu/thesaurus/10475"><rdfs:subClassOf rdf:resource="http://thesaurus.europeanafashion.eu/thesaurus/10521"/><rdfs:label xml:lang="de">Aluminiumfaden</rdfs:label><rdfs:label xml:lang="de">Aluminiumgespinstfaden</rdfs:label><rdfs:label xml:lang="sr">aluminijumska nit</rdfs:label><rdfs:label xml:lang="en">aluminium thread</rdfs:label><rdfs:label xml:lang="nl">aluminiumdraad</rdfs:label><rdfs:label xml:lang="sv">aluminiumtråd</rdfs:label><rdfs:label xml:lang="pt">alumínio</rdfs:label><rdfs:label xml:lang="fr">fil d'aluminium</rdfs:label><rdfs:label xml:lang="it">filo d'alluminio</rdfs:label><rdfs:label xml:lang="es">hilo de aluminio</rdfs:label><rdfs:label xml:lang="el">νήμα αλουμινίου</rdfs:label><rdfs:label xml:lang="he">חוט אלומיניום</rdfs:label></owl:Class><owl:Class rdf:about="http://thesaurus.europeanafashion.eu/thesaurus/10473"><rdfs:subClassOf rdf:resource="http://thesaurus.europeanafashion.eu/thesaurus/10557"/><rdfs:label xml:lang="de">Glasfaser</rdfs:label><rdfs:label xml:lang="en">fiberglass</rdfs:label><rdfs:label xml:lang="es">fibra de vidrio</rdfs:label><rdfs:label xml:lang="pt">fibra de vidro</rdfs:label><rdfs:label xml:lang="it">fibra di vetro</rdfs:label><rdfs:label xml:lang="fr">fibre de verre</rdfs:label><rdfs:label xml:lang="sv">glasfiber</rdfs:label><rdfs:label xml:lang="en">glass fibre</rdfs:label><rdfs:label xml:lang="nl">glasvezel</rdfs:label><rdfs:label xml:lang="sr">staklena vlakna</rdfs:label><rdfs:label xml:lang="el">υαλοβάμβακας</rdfs:label><rdfs:label xml:lang="he">סיבי זכוכית</rdfs:label><skos:exactMatch rdf:resource="http://vocab.getty.edu/aat/300183781"/><skos:scopeNote xml:lang="en">Generic term for glass fibers, glass fabrics, and resins reinforced with glass fibers; fiberglass is strong, lightweight, nonflammable, with a high tensile strength. The material dates to 1893, when spun glass fibers were made into fabric by Edward D. Libbey and exhibited at the Columbian Exhibition in Chicago. Owen-Corning developed several processes for making fine, continuous glass fibers in the 1930s, which were sold under the trademark of ‘Fiberglas.’ Over time, the term 'fiberglass' became generally used for all glass fiber products. (AAT)</skos:scopeNote></owl:Class><owl:Class rdf:about="http://thesaurus.europeanafashion.eu/thesaurus/10763"><rdfs:subClassOf rdf:resource="http://thesaurus.europeanafashion.eu/thesaurus/10557"/><rdfs:label xml:lang="en">Plexiglas</rdfs:label><rdfs:label xml:lang="fr">Plexiglas</rdfs:label><rdfs:label xml:lang="de">Plexiglas®</rdfs:label><rdfs:label xml:lang="it">Plexiglas® (polimetacrilato)</rdfs:label><rdfs:label xml:lang="sr">pleksiglas</rdfs:label><rdfs:label xml:lang="nl">plexiglas</rdfs:label><rdfs:label xml:lang="sv">plexiglas</rdfs:label><rdfs:label xml:lang="es">plexiglás</rdfs:label><rdfs:label xml:lang="el">πλέξιγκλας</rdfs:label><rdfs:label xml:lang="he">פלקסיגלס</rdfs:label><skos:exactMatch rdf:resource="http://vocab.getty.edu/aat/300014436"/><skos:scopeNote xml:lang="en">Proprietary name for polymerized methyl methacrylate, used as a substitute for glass in products such as windows, skylights, illuminated signs, and aircraft. Plexiglas was trademarked by Rohm and Haas AG in Germany ca. 1930s. (AAT)</skos:scopeNote></owl:Class><owl:Class rdf:about="http://thesaurus.europeanafashion.eu/thesaurus/11057"><rdfs:subClassOf rdf:resource="http://thesaurus.europeanafashion.eu/thesaurus/10557"/><rdfs:label xml:lang="de">Glaspaste</rdfs:label><rdfs:label xml:lang="sv">glasmassa</rdfs:label><rdfs:label xml:lang="en">glass paste</rdfs:label><rdfs:label xml:lang="it">pasta di vetro</rdfs:label><rdfs:label xml:lang="fr">pâte de verre</rdfs:label><rdfs:label xml:lang="nl">pâte de verre</rdfs:label><rdfs:label xml:lang="sr">staklena pasta</rdfs:label><rdfs:label xml:lang="el">υαλόμαζα</rdfs:label><rdfs:label xml:lang="he">דבק זכוכית</rdfs:label><skos:exactMatch rdf:resource="http://vocab.getty.edu/aat/300010803"/><skos:scopeNote xml:lang="en">A brilliant glass of high lead content used for the manufacture of artificial gems; also an imitation gem made of this material. (AAT)</skos:scopeNote></owl:Class><owl:Class rdf:about="http://thesaurus.europeanafashion.eu/thesaurus/10560"><rdfs:subClassOf rdf:resource="http://thesaurus.europeanafashion.eu/thesaurus/10559"/><rdfs:label xml:lang="de">Ebonit</rdfs:label><rdfs:label xml:lang="de">Hartgummi</rdfs:label><rdfs:label xml:lang="de">Hartkautschuk</rdfs:label><rdfs:label xml:lang="it">ebanite</rdfs:label><rdfs:label xml:lang="nl">eboniet</rdfs:label><rdfs:label xml:lang="sr">ebonit</rdfs:label><rdfs:label xml:lang="sv">ebonit</rdfs:label><rdfs:label xml:lang="es">ebonita</rdfs:label><rdfs:label xml:lang="en">ebonite</rdfs:label><rdfs:label xml:lang="nl">hardrubber</rdfs:label><rdfs:label xml:lang="nl">vulcaniet</rdfs:label><rdfs:label xml:lang="en">vulcanite</rdfs:label><rdfs:label xml:lang="fr">ébonite</rdfs:label><rdfs:label xml:lang="el">εβονίτης</rdfs:label><rdfs:label xml:lang="he">הבנית</rdfs:label><skos:exactMatch rdf:resource="http://vocab.getty.edu/aat/300380359"/><skos:scopeNote xml:lang="en">Vulcanite is as an old trade name for a dark, brittle, moldable hard rubber that was produced by heating (‘vulcanizing’) a preparation of india rubber and sulfur. It was marketed in the U.S. as vulcanite and in England as ebonite. Vulcanite was used for small items such as buttons, brooches, and combs, finishes on camera bodies, and for insulation. (AAT)</skos:scopeNote></owl:Class><owl:Class rdf:about="http://thesaurus.europeanafashion.eu/thesaurus/10562"><rdfs:subClassOf rdf:resource="http://thesaurus.europeanafashion.eu/thesaurus/10561"/><rdfs:label xml:lang="de">Aventurin</rdfs:label><rdfs:label xml:lang="de">Aventurin-Quarz</rdfs:label><rdfs:label xml:lang="nl">aventurien</rdfs:label><rdfs:label xml:lang="nl">aventurijn</rdfs:label><rdfs:label xml:lang="sv">aventurin</rdfs:label><rdfs:label xml:lang="fr">aventurine</rdfs:label><rdfs:label xml:lang="it">avventurina</rdfs:label><rdfs:label xml:lang="sr">venturin</rdfs:label><rdfs:label xml:lang="es">venturina</rdfs:label><rdfs:label xml:lang="en">venturine</rdfs:label><rdfs:label xml:lang="el">αβεντουρίνη</rdfs:label><rdfs:label xml:lang="he">אבקת זהב</rdfs:label></owl:Class><owl:Class rdf:about="http://thesaurus.europeanafashion.eu/thesaurus/10563"><rdfs:subClassOf rdf:resource="http://thesaurus.europeanafashion.eu/thesaurus/10561"/><rdfs:label xml:lang="de">Gagat</rdfs:label><rdfs:label xml:lang="de">Jet</rdfs:label><rdfs:label xml:lang="de">Jett</rdfs:label><rdfs:label xml:lang="es">azabache</rdfs:label><rdfs:label xml:lang="sr">gagat</rdfs:label><rdfs:label xml:lang="sv">gagat</rdfs:label><rdfs:label xml:lang="it">giaietto</rdfs:label><rdfs:label xml:lang="nl">git</rdfs:label><rdfs:label xml:lang="fr">jais</rdfs:label><rdfs:label xml:lang="en">jet</rdfs:label><rdfs:label xml:lang="nl">jet</rdfs:label><rdfs:label xml:lang="el">λιγνίτης</rdfs:label><rdfs:label xml:lang="he">סילון</rdfs:label><skos:exactMatch rdf:resource="http://vocab.getty.edu/aat/300045514"/><skos:scopeNote xml:lang="en">A dense, black, semiprecious form of lignite that takes a brilliant polish and is used ornamentally, particularly in Victorian mourning jewelry. (AAT)</skos:scopeNote></owl:Class><owl:Class rdf:about="http://thesaurus.europeanafashion.eu/thesaurus/10925"><rdfs:subClassOf rdf:resource="http://thesaurus.europeanafashion.eu/thesaurus/10561"/><rdfs:label xml:lang="de">Marmor</rdfs:label><rdfs:label xml:lang="en">marble</rdfs:label><rdfs:label xml:lang="fr">marbre</rdfs:label><rdfs:label xml:lang="nl">marmer</rdfs:label><rdfs:label xml:lang="it">marmo</rdfs:label><rdfs:label xml:lang="sv">marmor</rdfs:label><rdfs:label xml:lang="sr">mermer</rdfs:label><rdfs:label xml:lang="el">μάρμαρο</rdfs:label><rdfs:label xml:lang="he">שיש</rdfs:label><skos:exactMatch rdf:resource="http://vocab.getty.edu/aat/300011443"/><skos:scopeNote xml:lang="en">A metamorphic, hard, dense, crystalline stone primarily composed of calcium carbonate; it is limestone or dolomite that has been metamorphosed with heat and pressure. Pure calcite marble is white, but impurities produce a wide variety of coloring and patterns. It is finely grained and polishes to a smooth, high gloss. It is used primarily for statuary and buildings. Marble has been quarried from sites around the world since at least the 7th century BCE. The term can also refer more broadly to any crystallized carbonate rock, including true marble and certain types of limestone, that will take a polish and can be used for architectural and ornamental purposes. (AAT)</skos:scopeNote></owl:Class><owl:Class rdf:about="http://thesaurus.europeanafashion.eu/thesaurus/10926"><rdfs:subClassOf rdf:resource="http://thesaurus.europeanafashion.eu/thesaurus/10561"/><rdfs:label xml:lang="de">Türkis (Kallait)</rdfs:label><rdfs:label xml:lang="sr">tirkiz</rdfs:label><rdfs:label xml:lang="it">turchese</rdfs:label><rdfs:label xml:lang="nl">turkoois</rdfs:label><rdfs:label xml:lang="sv">turkos</rdfs:label><rdfs:label xml:lang="en">turquoise</rdfs:label><rdfs:label xml:lang="fr">turquoise</rdfs:label><rdfs:label xml:lang="el">τυρκουάζ</rdfs:label><rdfs:label xml:lang="he">טורקיז</rdfs:label><skos:exactMatch rdf:resource="http://vocab.getty.edu/aat/300011164"/><skos:scopeNote xml:lang="en">A triclinic mineral of blue, blue green, or yellowish green color. (AAT)</skos:scopeNote></owl:Class><owl:Class rdf:about="http://thesaurus.europeanafashion.eu/thesaurus/11058"><rdfs:subClassOf rdf:resource="http://thesaurus.europeanafashion.eu/thesaurus/10561"/><rdfs:label xml:lang="de">Achat-Quarz</rdfs:label><rdfs:label xml:lang="nl">agaat</rdfs:label><rdfs:label xml:lang="sv">agat</rdfs:label><rdfs:label xml:lang="it">agata</rdfs:label><rdfs:label xml:lang="en">agate</rdfs:label><rdfs:label xml:lang="fr">agate</rdfs:label><rdfs:label xml:lang="sr">ahat</rdfs:label><rdfs:label xml:lang="el">αχάτης</rdfs:label><rdfs:label xml:lang="he">אגט</rdfs:label><rdfs:label xml:lang="he">נופך</rdfs:label><skos:exactMatch rdf:resource="http://vocab.getty.edu/aat/300011135"/><skos:scopeNote xml:lang="en">Cryptocrystalline chalcedony, showing a variegated banded structure and waxy luster. Agate bands are caused by the deposition of successive mineral layers from solution and may be either straight, wavy, or concentric. Agate is slightly harder than quartz. It has been gathered or mined since Neolithic times. It may distinguished from onyx by the parallel structure of the bars in onyx. (AAT)</skos:scopeNote></owl:Class><owl:Class rdf:about="http://thesaurus.europeanafashion.eu/thesaurus/11059"><rdfs:subClassOf rdf:resource="http://thesaurus.europeanafashion.eu/thesaurus/10561"/><rdfs:label xml:lang="de">Karneol</rdfs:label><rdfs:label xml:lang="en">carnelian</rdfs:label><rdfs:label xml:lang="fr">cornaline</rdfs:label><rdfs:label xml:lang="it">corniola</rdfs:label><rdfs:label xml:lang="sr">karneol</rdfs:label><rdfs:label xml:lang="sv">karneol</rdfs:label><rdfs:label xml:lang="nl">kornalijn</rdfs:label><rdfs:label xml:lang="el">καρνεόλιο</rdfs:label><rdfs:label xml:lang="he">קרנליאן</rdfs:label><skos:exactMatch rdf:resource="http://vocab.getty.edu/aat/300133223"/><skos:scopeNote xml:lang="en">A translucent red or orange variety of chalcedony, containing iron impurities. It is often used for seals and signet rings. (AAT)</skos:scopeNote></owl:Class><owl:Class rdf:about="http://thesaurus.europeanafashion.eu/thesaurus/11060"><rdfs:subClassOf rdf:resource="http://thesaurus.europeanafashion.eu/thesaurus/10561"/><rdfs:label xml:lang="de">Sandstein</rdfs:label><rdfs:label xml:lang="it">arenaria</rdfs:label><rdfs:label xml:lang="fr">grès (mat.)</rdfs:label><rdfs:label xml:lang="sr">peščar</rdfs:label><rdfs:label xml:lang="sv">sandsten</rdfs:label><rdfs:label xml:lang="en">sandstone</rdfs:label><rdfs:label xml:lang="nl">zandsteen</rdfs:label><rdfs:label xml:lang="el">αμμόλιθος</rdfs:label><rdfs:label xml:lang="he">אבן חול</rdfs:label><rdfs:label xml:lang="he">קרניאול</rdfs:label><skos:exactMatch rdf:resource="http://vocab.getty.edu/aat/300011376"/><skos:scopeNote xml:lang="en">A consolidated sedimentary rock, consisting of sand grains united with a natural cementing material; the most common sand in sandstone contains quartz, with considerable feldspar, lime, mica, and clayey matter. (AAT)</skos:scopeNote></owl:Class><owl:Class rdf:about="http://thesaurus.europeanafashion.eu/thesaurus/11061"><rdfs:subClassOf rdf:resource="http://thesaurus.europeanafashion.eu/thesaurus/10561"/><rdfs:label xml:lang="de">Jade</rdfs:label><rdfs:label xml:lang="it">giada</rdfs:label><rdfs:label xml:lang="en">jade</rdfs:label><rdfs:label xml:lang="fr">jade</rdfs:label><rdfs:label xml:lang="nl">jade</rdfs:label><rdfs:label xml:lang="sv">jade</rdfs:label><rdfs:label xml:lang="sr">žad</rdfs:label><rdfs:label xml:lang="el">τζαντ</rdfs:label><rdfs:label xml:lang="he">ירקן</rdfs:label><skos:exactMatch rdf:resource="http://vocab.getty.edu/aat/300011119"/><skos:scopeNote xml:lang="en">General term for several varieties of hard and soft, fine-grained rock composed of jadeite, nephrite, serpentine, or other mineralogically related materials; usually having a color ranging from dark green to green-white. Jade takes a high polish and has been used since prehistoric times for jewelry, small utensils, carvings, vases, and other ornamental objects. Some processing techniques have been used to enhance the color of inferior stones: B-jade has been bleached to remove brown stains, while C-jade has been impregnated with resins to increase its translucency; A-jade is untreated. (AAT)</skos:scopeNote></owl:Class><owl:Class rdf:about="http://thesaurus.europeanafashion.eu/thesaurus/10566"><rdfs:subClassOf rdf:resource="http://thesaurus.europeanafashion.eu/thesaurus/10565"/><rdfs:label xml:lang="de">Porzellan</rdfs:label><rdfs:label xml:lang="en">porcelain</rdfs:label><rdfs:label xml:lang="fr">porcelaine</rdfs:label><rdfs:label xml:lang="sr">porcelan</rdfs:label><rdfs:label xml:lang="es">porcelana</rdfs:label><rdfs:label xml:lang="it">porcellana</rdfs:label><rdfs:label xml:lang="nl">porselein</rdfs:label><rdfs:label xml:lang="sv">porslin</rdfs:label><rdfs:label xml:lang="el">πορσελάνη</rdfs:label><rdfs:label xml:lang="he">חרסינה</rdfs:label><skos:exactMatch rdf:resource="http://vocab.getty.edu/aat/300010662"/><skos:scopeNote xml:lang="en">A material comprising white clay, or kaolin, and a feldspathic rock, that react when fired so the clay serves to hold the shape of the object and the rock fuses into a natural glass. In China, it includes any such ware that is highly fired enough to produce a ringing sound when struck. In Europe, it is limited to hard-fired ceramic that is translucent. (AAT)</skos:scopeNote></owl:Class><owl:Class rdf:about="http://thesaurus.europeanafashion.eu/thesaurus/11063"><rdfs:subClassOf rdf:resource="http://thesaurus.europeanafashion.eu/thesaurus/10565"/><rdfs:label xml:lang="de">Terrakotta</rdfs:label><rdfs:label xml:lang="sr">terakota</rdfs:label><rdfs:label xml:lang="en">terra cotta</rdfs:label><rdfs:label xml:lang="it">terra cotta</rdfs:label><rdfs:label xml:lang="nl">terra cotta</rdfs:label><rdfs:label xml:lang="sv">terrakotta</rdfs:label><rdfs:label xml:lang="fr">terre cuite</rdfs:label><rdfs:label xml:lang="el">τερακότα</rdfs:label><rdfs:label xml:lang="he">חומר שרוף לא מזוגג</rdfs:label><rdfs:label xml:lang="he">טרה קוטה</rdfs:label><skos:scopeNote xml:lang="en">A baked or semi-fired material that is usually a mixture of clay, grog, and water; it has been used for pottery, statuettes, lamps, roof tiles, and cornices since ancient times. It may be glazed prior to firing. To produce an item, terracotta is molded or shaped, dried for several days then fired to at least 600 C. It is fireproof, lighter in weight than stone, and usually brownish red in color. (AAT)</skos:scopeNote></owl:Class><owl:Class rdf:about="http://thesaurus.europeanafashion.eu/thesaurus/10815"><rdfs:subClassOf rdf:resource="http://thesaurus.europeanafashion.eu/thesaurus/10566"/><rdfs:label xml:lang="de">Biskuitporzellan</rdfs:label><rdfs:label xml:lang="it">biscotto</rdfs:label><rdfs:label xml:lang="en">biscuit</rdfs:label><rdfs:label xml:lang="fr">biscuit</rdfs:label><rdfs:label xml:lang="nl">biscuit</rdfs:label><rdfs:label xml:lang="sv">biskviporslin</rdfs:label><rdfs:label xml:lang="sr">biskvit</rdfs:label><rdfs:label xml:lang="en">bisque</rdfs:label><rdfs:label xml:lang="de">unglasiertes Porzellan</rdfs:label><rdfs:label xml:lang="el">μπισκουϊ</rdfs:label><rdfs:label xml:lang="he">ביסקוויט</rdfs:label><skos:exactMatch rdf:resource="http://vocab.getty.edu/aat/300242297"/><skos:scopeNote xml:lang="en">Unglazed ceramic material that has been fired only once; generally producing a grainy texture; frequently used for modeling ornament or making small statues, dolls, or vessels. Distinct from parian (porcelain), which is silky in texture and marblelike in appearance. (AAT)</skos:scopeNote></owl:Class><owl:Class rdf:about="http://thesaurus.europeanafashion.eu/thesaurus/10351"><rdfs:subClassOf rdf:resource="http://thesaurus.europeanafashion.eu/thesaurus/10350"/><rdfs:label xml:lang="de">Wolle</rdfs:label><rdfs:label xml:lang="fr">laine</rdfs:label><rdfs:label xml:lang="es">lana</rdfs:label><rdfs:label xml:lang="it">lana</rdfs:label><rdfs:label xml:lang="pt">lã</rdfs:label><rdfs:label xml:lang="sv">ull</rdfs:label><rdfs:label xml:lang="sr">vuna</rdfs:label><rdfs:label xml:lang="nl">wol</rdfs:label><rdfs:label xml:lang="en">wool</rdfs:label><rdfs:label xml:lang="el">μαλλί</rdfs:label><rdfs:label xml:lang="he">צמר</rdfs:label><skos:exactMatch rdf:resource="http://vocab.getty.edu/aat/300014074"/><skos:scopeNote xml:lang="en">Textile made from the animal hair wool. (AAT)</skos:scopeNote></owl:Class><owl:Class rdf:about="http://thesaurus.europeanafashion.eu/thesaurus/10352"><rdfs:subClassOf rdf:resource="http://thesaurus.europeanafashion.eu/thesaurus/10350"/><rdfs:label xml:lang="de">Seide</rdfs:label><rdfs:label xml:lang="es">seda</rdfs:label><rdfs:label xml:lang="pt">seda</rdfs:label><rdfs:label xml:lang="it">seta</rdfs:label><rdfs:label xml:lang="sv">siden</rdfs:label><rdfs:label xml:lang="en">silk</rdfs:label><rdfs:label xml:lang="fr">soie</rdfs:label><rdfs:label xml:lang="sr">svila</rdfs:label><rdfs:label xml:lang="nl">zijde</rdfs:label><rdfs:label xml:lang="el">μετάξι</rdfs:label><rdfs:label xml:lang="he">משי</rdfs:label><skos:exactMatch rdf:resource="http://vocab.getty.edu/aat/300014072"/><skos:scopeNote xml:lang="en">Fine continuous protein fiber consisting primarily of fibroin filaments, secreted by silk caterpillars. (AAT)</skos:scopeNote></owl:Class><owl:Class rdf:about="http://thesaurus.europeanafashion.eu/thesaurus/10476"><rdfs:subClassOf rdf:resource="http://thesaurus.europeanafashion.eu/thesaurus/10350"/><rdfs:label xml:lang="de">Spinnennetzseide</rdfs:label><rdfs:label xml:lang="de">Spinnenseide</rdfs:label><rdfs:label xml:lang="pt">fibra de teia de aranha</rdfs:label><rdfs:label xml:lang="es">hilo de araña</rdfs:label><rdfs:label xml:lang="sr">nit paukove mreže</rdfs:label><rdfs:label xml:lang="it">seta di tela di ragno</rdfs:label><rdfs:label xml:lang="fr">soie d'araignée</rdfs:label><rdfs:label xml:lang="en">spider web fibre</rdfs:label><rdfs:label xml:lang="sv">spindelsilke</rdfs:label><rdfs:label xml:lang="nl">spinnenwebvezel</rdfs:label><rdfs:label xml:lang="nl">spinrag</rdfs:label><rdfs:label xml:lang="el">ιστός αράχνης</rdfs:label><rdfs:label xml:lang="he">סיבי קורי עכביש</rdfs:label></owl:Class><owl:Class rdf:about="http://thesaurus.europeanafashion.eu/thesaurus/10531"><rdfs:subClassOf rdf:resource="http://thesaurus.europeanafashion.eu/thesaurus/10350"/><rdfs:label xml:lang="de">Haar</rdfs:label><rdfs:label xml:lang="nl">haar</rdfs:label><rdfs:label xml:lang="en">hair</rdfs:label><rdfs:label xml:lang="sv">hår</rdfs:label><rdfs:label xml:lang="sr">kosa</rdfs:label><rdfs:label xml:lang="es">pelo</rdfs:label><rdfs:label xml:lang="it">pelo</rdfs:label><rdfs:label xml:lang="fr">poil</rdfs:label><rdfs:label xml:lang="el">τρίχα</rdfs:label><rdfs:label xml:lang="he">שערה</rdfs:label><skos:exactMatch rdf:resource="http://vocab.getty.edu/aat/300011814"/><skos:scopeNote xml:lang="en">The fibrous outgrowths of the skins of various animals, composed of the protein keratin, used with other fibers for making fabrics, as stuffing, and for making brushes. (AAT)</skos:scopeNote></owl:Class><owl:Class rdf:about="http://thesaurus.europeanafashion.eu/thesaurus/10534"><rdfs:subClassOf rdf:resource="http://thesaurus.europeanafashion.eu/thesaurus/10350"/><rdfs:label xml:lang="de">Fell</rdfs:label><rdfs:label xml:lang="de">Haut</rdfs:label><rdfs:label xml:lang="de">Leder</rdfs:label><rdfs:label xml:lang="sv">hud</rdfs:label><rdfs:label xml:lang="nl">huid</rdfs:label><rdfs:label xml:lang="sr">koža</rdfs:label><rdfs:label xml:lang="sv">läder</rdfs:label><rdfs:label xml:lang="fr">peau</rdfs:label><rdfs:label xml:lang="it">pelle</rdfs:label><rdfs:label xml:lang="es">piel</rdfs:label><rdfs:label xml:lang="en">skin</rdfs:label><rdfs:label xml:lang="sv">skinn</rdfs:label><rdfs:label xml:lang="el">τομάρι</rdfs:label><rdfs:label xml:lang="he">עור</rdfs:label><skos:exactMatch rdf:resource="http://vocab.getty.edu/aat/300011840"/><skos:scopeNote xml:lang="en">Integument of animals such as sheep, calves, or goats, separated from the body, with or without hair, whether green, dry, tanned, or dressed. For the integument of large animals use hide. For tanned skin, use leather. For dried and stretched skin, use parchment or vellum. (AAT)</skos:scopeNote></owl:Class><owl:Class rdf:about="http://thesaurus.europeanafashion.eu/thesaurus/10539"><rdfs:subClassOf rdf:resource="http://thesaurus.europeanafashion.eu/thesaurus/10350"/><rdfs:label xml:lang="de">Fell</rdfs:label><rdfs:label xml:lang="de">Pelz</rdfs:label><rdfs:label xml:lang="nl">bont</rdfs:label><rdfs:label xml:lang="fr">fourrure</rdfs:label><rdfs:label xml:lang="en">fur</rdfs:label><rdfs:label xml:lang="sr">krzno</rdfs:label><rdfs:label xml:lang="it">pelliccia</rdfs:label><rdfs:label xml:lang="nl">pels</rdfs:label><rdfs:label xml:lang="es">piel (de pelo largo)</rdfs:label><rdfs:label xml:lang="sv">päls</rdfs:label><rdfs:label xml:lang="nl">vacht</rdfs:label><rdfs:label xml:lang="el">γούνα</rdfs:label><rdfs:label xml:lang="he">פרווה</rdfs:label><skos:exactMatch rdf:resource="http://vocab.getty.edu/aat/300011811"/><skos:scopeNote xml:lang="en">Fine, soft, thick, hairy coat of a mammal, usually consisting of a double coat of hair that includes a layer of comparatively short, soft, curly barbed hair next to the skin, protected by longer, smoother, stiffer hair growing up through it. (AAT)</skos:scopeNote></owl:Class><owl:Class rdf:about="http://thesaurus.europeanafashion.eu/thesaurus/10582"><rdfs:subClassOf rdf:resource="http://thesaurus.europeanafashion.eu/thesaurus/10350"/><rdfs:label xml:lang="de">Muschel</rdfs:label><rdfs:label xml:lang="es">concha</rdfs:label><rdfs:label xml:lang="it">conchiglia</rdfs:label><rdfs:label xml:lang="fr">coquillage</rdfs:label><rdfs:label xml:lang="fr">coquille</rdfs:label><rdfs:label xml:lang="nl">schelp</rdfs:label><rdfs:label xml:lang="en">seashell</rdfs:label><rdfs:label xml:lang="en">shell</rdfs:label><rdfs:label xml:lang="sv">snäckskal</rdfs:label><rdfs:label xml:lang="sr">školjka</rdfs:label><rdfs:label xml:lang="el">κοχύλι</rdfs:label><rdfs:label xml:lang="he">צדף</rdfs:label><skos:exactMatch rdf:resource="http://vocab.getty.edu/aat/300011829"/><skos:scopeNote xml:lang="en">Hard outer covering of invertebrate creatures, composed of calcareous or chitinous material. (AAT)</skos:scopeNote></owl:Class><owl:Class rdf:about="http://thesaurus.europeanafashion.eu/thesaurus/10583"><rdfs:subClassOf rdf:resource="http://thesaurus.europeanafashion.eu/thesaurus/10350"/><rdfs:label xml:lang="de">Schildkröte</rdfs:label><rdfs:label xml:lang="es">carey</rdfs:label><rdfs:label xml:lang="sr">kornjačevina</rdfs:label><rdfs:label xml:lang="nl">schilpad(schaal)</rdfs:label><rdfs:label xml:lang="sv">sköldpadd</rdfs:label><rdfs:label xml:lang="it">tartaruga</rdfs:label><rdfs:label xml:lang="en">turtle</rdfs:label><rdfs:label xml:lang="fr">écaille de tortue</rdfs:label><rdfs:label xml:lang="el">ταρταρούγα</rdfs:label><rdfs:label xml:lang="he">שריון צב</rdfs:label></owl:Class><owl:Class rdf:about="http://thesaurus.europeanafashion.eu/thesaurus/10584"><rdfs:subClassOf rdf:resource="http://thesaurus.europeanafashion.eu/thesaurus/10350"/><rdfs:label xml:lang="de">Koralle</rdfs:label><rdfs:label xml:lang="fr">corail</rdfs:label><rdfs:label xml:lang="en">coral</rdfs:label><rdfs:label xml:lang="es">coral</rdfs:label><rdfs:label xml:lang="it">corallo</rdfs:label><rdfs:label xml:lang="nl">koraal</rdfs:label><rdfs:label xml:lang="sr">korali</rdfs:label><rdfs:label xml:lang="sv">korall</rdfs:label><rdfs:label xml:lang="el">κοράλλι</rdfs:label><rdfs:label xml:lang="he">אלמוג</rdfs:label><skos:exactMatch rdf:resource="http://vocab.getty.edu/aat/300011800"/><skos:scopeNote xml:lang="en">Hard material consisting of calcium carbonate derived from the skeletal deposits of certain marine animals. (AAT)</skos:scopeNote></owl:Class><owl:Class rdf:about="http://thesaurus.europeanafashion.eu/thesaurus/10585"><rdfs:subClassOf rdf:resource="http://thesaurus.europeanafashion.eu/thesaurus/10350"/><rdfs:label xml:lang="de">Fischbein</rdfs:label><rdfs:label xml:lang="en">baleen</rdfs:label><rdfs:label xml:lang="nl">balein</rdfs:label><rdfs:label xml:lang="es">ballena</rdfs:label><rdfs:label xml:lang="fr">fanon</rdfs:label><rdfs:label xml:lang="it">fanone</rdfs:label><rdfs:label xml:lang="sr">kitova kost</rdfs:label><rdfs:label xml:lang="it">osso di balena</rdfs:label><rdfs:label xml:lang="sr">riblja kost</rdfs:label><rdfs:label xml:lang="sv">valbard</rdfs:label><rdfs:label xml:lang="en">whalebone</rdfs:label><rdfs:label xml:lang="el">μπαλένα</rdfs:label><rdfs:label xml:lang="el">μπανέλα</rdfs:label><rdfs:label xml:lang="he">מזיפה</rdfs:label><skos:exactMatch rdf:resource="http://vocab.getty.edu/aat/300192974"/><skos:scopeNote xml:lang="en">A horny keratinous substance that grows in the mouth of whales. (AAT)</skos:scopeNote></owl:Class><owl:Class rdf:about="http://thesaurus.europeanafashion.eu/thesaurus/10586"><rdfs:subClassOf rdf:resource="http://thesaurus.europeanafashion.eu/thesaurus/10350"/><rdfs:label xml:lang="de">Wachs</rdfs:label><rdfs:label xml:lang="es">cera</rdfs:label><rdfs:label xml:lang="it">cera</rdfs:label><rdfs:label xml:lang="fr">cire</rdfs:label><rdfs:label xml:lang="sv">vax</rdfs:label><rdfs:label xml:lang="sr">vosak</rdfs:label><rdfs:label xml:lang="nl">was</rdfs:label><rdfs:label xml:lang="en">wax</rdfs:label><rdfs:label xml:lang="el">κερί</rdfs:label><rdfs:label xml:lang="he">שעווה</rdfs:label><skos:exactMatch rdf:resource="http://vocab.getty.edu/aat/300014585"/><skos:scopeNote xml:lang="en">Any solid or semi-solid substance that is slightly greasy to touch, usually solid, translucent, and has a low melting point; waxes are not a chemically homogeneous group. Waxes are composed of long chain hydrocarbon compounds, and may contain esters of fatty acids and alcohols, are thermoplastic and melt at low temperatures of between 40 and 100 C. In general, waxes are water-repellent, smooth, soluble in organic solvents, and classified as animal (e.g., beeswax), vegetable (e.g., bayberry), mineral (e.g., paraffin), or synthetic (e.g., polyethylene). Waxes are used for polishes, candles, crayons, sealants, coatings, adhesives, waterproofing, carbon paper, media in encaustic and wax emulsion paintings, and as repellents in wax-resist watercolor paintings. (AAT)</skos:scopeNote></owl:Class><owl:Class rdf:about="http://thesaurus.europeanafashion.eu/thesaurus/10587"><rdfs:subClassOf rdf:resource="http://thesaurus.europeanafashion.eu/thesaurus/10350"/><rdfs:label xml:lang="de">Perlmutt</rdfs:label><rdfs:label xml:lang="es">madreperla</rdfs:label><rdfs:label xml:lang="it">madreperla</rdfs:label><rdfs:label xml:lang="en">mother of pearl</rdfs:label><rdfs:label xml:lang="fr">nacre</rdfs:label><rdfs:label xml:lang="es">nácar</rdfs:label><rdfs:label xml:lang="nl">paarlemoer</rdfs:label><rdfs:label xml:lang="sv">pärlemor</rdfs:label><rdfs:label xml:lang="sr">sedef</rdfs:label><rdfs:label xml:lang="el">φίλντισι</rdfs:label><rdfs:label xml:lang="he">דר</rdfs:label><skos:exactMatch rdf:resource="http://vocab.getty.edu/aat/300011835"/><skos:scopeNote xml:lang="en">Hard, pearly, iridescent internal layer of various kinds of mollusk shell, extensively used for making small articles and inlays. (AAT)</skos:scopeNote></owl:Class><owl:Class rdf:about="http://thesaurus.europeanafashion.eu/thesaurus/10588"><rdfs:subClassOf rdf:resource="http://thesaurus.europeanafashion.eu/thesaurus/10350"/><rdfs:label xml:lang="de">Horn</rdfs:label><rdfs:label xml:lang="es">asta</rdfs:label><rdfs:label xml:lang="fr">corne</rdfs:label><rdfs:label xml:lang="it">corno</rdfs:label><rdfs:label xml:lang="es">cuerno</rdfs:label><rdfs:label xml:lang="nl">hoorn</rdfs:label><rdfs:label xml:lang="en">horn</rdfs:label><rdfs:label xml:lang="sv">horn</rdfs:label><rdfs:label xml:lang="sr">rog</rdfs:label><rdfs:label xml:lang="el">κέρατο</rdfs:label><rdfs:label xml:lang="he">אם הפנינה</rdfs:label><rdfs:label xml:lang="he">קרן יער</rdfs:label><skos:exactMatch rdf:resource="http://vocab.getty.edu/aat/300011826"/><skos:scopeNote xml:lang="en">Outgrowth of modified skin or compacted hair, often occuring in pairs, projecting from the frontal bones on either side of the skull, consisting of a nondeciduous cuticle composed of keratin. Distinguished from antler, which is modified bone. (AAT)</skos:scopeNote></owl:Class><owl:Class rdf:about="http://thesaurus.europeanafashion.eu/thesaurus/10589"><rdfs:subClassOf rdf:resource="http://thesaurus.europeanafashion.eu/thesaurus/10350"/><rdfs:label xml:lang="de">Feder</rdfs:label><rdfs:label xml:lang="en">feather</rdfs:label><rdfs:label xml:lang="sv">fjäder</rdfs:label><rdfs:label xml:lang="sr">pero</rdfs:label><rdfs:label xml:lang="it">piuma</rdfs:label><rdfs:label xml:lang="es">pluma</rdfs:label><rdfs:label xml:lang="fr">plume</rdfs:label><rdfs:label xml:lang="nl">veer</rdfs:label><rdfs:label xml:lang="el">φτερό</rdfs:label><rdfs:label xml:lang="he">נוצה</rdfs:label><skos:exactMatch rdf:resource="http://vocab.getty.edu/aat/300011809"/><skos:scopeNote xml:lang="en">The light, horny, epidermal outgrowths that form the external covering of the body of birds. (AAT)</skos:scopeNote></owl:Class><owl:Class rdf:about="http://thesaurus.europeanafashion.eu/thesaurus/10591"><rdfs:subClassOf rdf:resource="http://thesaurus.europeanafashion.eu/thesaurus/10350"/><rdfs:label xml:lang="de">Elfenbein</rdfs:label><rdfs:label xml:lang="it">avorio</rdfs:label><rdfs:label xml:lang="sv">elfenben</rdfs:label><rdfs:label xml:lang="fr">ivoire</rdfs:label><rdfs:label xml:lang="nl">ivoor</rdfs:label><rdfs:label xml:lang="en">ivory</rdfs:label><rdfs:label xml:lang="es">marfil</rdfs:label><rdfs:label xml:lang="sr">slonovača</rdfs:label><rdfs:label xml:lang="el">ελεφαντόδοντο</rdfs:label><rdfs:label xml:lang="he">שנהב</rdfs:label><skos:exactMatch rdf:resource="http://vocab.getty.edu/aat/300011857"/><skos:scopeNote xml:lang="en">The modified form of dentine found on the tusks of mature elephants, and for similar material from any tusked or large-toothed mammal such as a walrus or narwhal. (AAT)</skos:scopeNote></owl:Class><owl:Class rdf:about="http://thesaurus.europeanafashion.eu/thesaurus/10592"><rdfs:subClassOf rdf:resource="http://thesaurus.europeanafashion.eu/thesaurus/10350"/><rdfs:label xml:lang="de">Bein</rdfs:label><rdfs:label xml:lang="de">Knochen</rdfs:label><rdfs:label xml:lang="nl">been</rdfs:label><rdfs:label xml:lang="sv">ben</rdfs:label><rdfs:label xml:lang="en">bone</rdfs:label><rdfs:label xml:lang="es">hueso</rdfs:label><rdfs:label xml:lang="sr">kost</rdfs:label><rdfs:label xml:lang="fr">os</rdfs:label><rdfs:label xml:lang="it">osso</rdfs:label><rdfs:label xml:lang="pt">osso</rdfs:label><rdfs:label xml:lang="el">κόκαλο</rdfs:label><rdfs:label xml:lang="he">עצם</rdfs:label><skos:exactMatch rdf:resource="http://vocab.getty.edu/aat/300011798"/><skos:scopeNote xml:lang="en">The rigid, calcareous material that is white in color and forms the skeleton of vertebrates; primarily composed of calcium hydroxyapatite with smaller amounts of calcium carbonate, calcium fluoride, magnesium phosphate, and ossein, a high molecular weight protein. Bones have a concentric structure with central lymphatic canals surrounded by a spongy lamellar region protected by a dense outer cortex. Bone has been carved and used since ancient times for many purposes, including fish-hooks, spear heads, needles, handles, and art objects. Bones were also burnt to produce bone black and boiled to produce bone glue. Bone can be distinguished from ivory by being generally whiter, more porous, and less dense. (AAT)</skos:scopeNote></owl:Class><owl:Class rdf:about="http://thesaurus.europeanafashion.eu/thesaurus/10593"><rdfs:subClassOf rdf:resource="http://thesaurus.europeanafashion.eu/thesaurus/10350"/><rdfs:label xml:lang="de">Pergament</rdfs:label><rdfs:label xml:lang="fr">parchemin</rdfs:label><rdfs:label xml:lang="en">parchment</rdfs:label><rdfs:label xml:lang="it">pergamena</rdfs:label><rdfs:label xml:lang="sr">pergament</rdfs:label><rdfs:label xml:lang="sv">pergament</rdfs:label><rdfs:label xml:lang="es">pergamino</rdfs:label><rdfs:label xml:lang="nl">perkament</rdfs:label><rdfs:label xml:lang="el">περγαμηνή</rdfs:label><rdfs:label xml:lang="he">קלף</rdfs:label><skos:exactMatch rdf:resource="http://vocab.getty.edu/aat/300011851"/><skos:scopeNote xml:lang="en">Translucent or opaque material made from calf, sheep, or goat skin which has been limed, dehaired, scraped, and dried under tension to produce a thin, strong material for writing, bookbinding, or other uses. For finer quality calf parchment, use vellum. The terms parchment and vellum sometimes have been and still are both confused and used interchangeably. (AAT)</skos:scopeNote></owl:Class><owl:Class rdf:about="http://thesaurus.europeanafashion.eu/thesaurus/10594"><rdfs:subClassOf rdf:resource="http://thesaurus.europeanafashion.eu/thesaurus/10350"/><rdfs:label xml:lang="de">Pansen</rdfs:label><rdfs:label xml:lang="sv">djurmage</rdfs:label><rdfs:label xml:lang="nl">pens</rdfs:label><rdfs:label xml:lang="sv">tarm</rdfs:label><rdfs:label xml:lang="es">tripa</rdfs:label><rdfs:label xml:lang="en">tripe</rdfs:label><rdfs:label xml:lang="fr">tripe</rdfs:label><rdfs:label xml:lang="sr">tripe</rdfs:label><rdfs:label xml:lang="it">trippa</rdfs:label><rdfs:label xml:lang="el">πατσάς</rdfs:label><rdfs:label xml:lang="he">מעיים</rdfs:label></owl:Class><owl:Class rdf:about="http://thesaurus.europeanafashion.eu/thesaurus/11080"><rdfs:subClassOf rdf:resource="http://thesaurus.europeanafashion.eu/thesaurus/10350"/><rdfs:label xml:lang="de">Kesselstein</rdfs:label><rdfs:label xml:lang="sv">fjäll</rdfs:label><rdfs:label xml:lang="sr">krljušt</rdfs:label><rdfs:label xml:lang="en">scale</rdfs:label><rdfs:label xml:lang="nl">schaal</rdfs:label><rdfs:label xml:lang="it">squama</rdfs:label><rdfs:label xml:lang="fr">écaille</rdfs:label><rdfs:label xml:lang="el">λέπι</rdfs:label><rdfs:label xml:lang="el">φολίδα</rdfs:label><rdfs:label xml:lang="he">קשקש</rdfs:label></owl:Class><owl:Class rdf:about="http://thesaurus.europeanafashion.eu/thesaurus/10811"><rdfs:subClassOf rdf:resource="http://thesaurus.europeanafashion.eu/thesaurus/10351"/><rdfs:label xml:lang="de">Angora</rdfs:label><rdfs:label xml:lang="en">angora</rdfs:label><rdfs:label xml:lang="es">angora</rdfs:label><rdfs:label xml:lang="fr">angora</rdfs:label><rdfs:label xml:lang="it">angora</rdfs:label><rdfs:label xml:lang="nl">angora</rdfs:label><rdfs:label xml:lang="sr">angora</rdfs:label><rdfs:label xml:lang="sv">angora</rdfs:label><rdfs:label xml:lang="el">ανκορά</rdfs:label><rdfs:label xml:lang="he">אנגורה</rdfs:label><skos:exactMatch rdf:resource="http://vocab.getty.edu/aat/300386672"/><skos:scopeNote xml:lang="en">The long, fine hair from any breed of Angora rabbit. The white French rabbit is favored for its high-quality, soft hair. Angora dyes readily, but is difficult to spin because of its fine texture and it does not felt like common rabbit hair. It is usually mixed with sheep wool or other fibers for weaving. (AAT)</skos:scopeNote></owl:Class><owl:Class rdf:about="http://thesaurus.europeanafashion.eu/thesaurus/10812"><rdfs:subClassOf rdf:resource="http://thesaurus.europeanafashion.eu/thesaurus/10351"/><rdfs:label xml:lang="de">Mohair</rdfs:label><rdfs:label xml:lang="en">mohair</rdfs:label><rdfs:label xml:lang="es">mohair</rdfs:label><rdfs:label xml:lang="fr">mohair</rdfs:label><rdfs:label xml:lang="it">mohair</rdfs:label><rdfs:label xml:lang="nl">mohair</rdfs:label><rdfs:label xml:lang="sv">mohair</rdfs:label><rdfs:label xml:lang="sr">moher</rdfs:label><rdfs:label xml:lang="el">μοχέρ</rdfs:label><rdfs:label xml:lang="he">מוהר</rdfs:label><skos:exactMatch rdf:resource="http://vocab.getty.edu/aat/300192989"/><skos:scopeNote xml:lang="en">Long, lustrous hair of the Angora goat, valued for its strength and excellent spinning qualities. (AAT)</skos:scopeNote></owl:Class><owl:Class rdf:about="http://thesaurus.europeanafashion.eu/thesaurus/10813"><rdfs:subClassOf rdf:resource="http://thesaurus.europeanafashion.eu/thesaurus/10351"/><rdfs:label xml:lang="de">Alpaka</rdfs:label><rdfs:label xml:lang="en">alpaca</rdfs:label><rdfs:label xml:lang="es">alpaca</rdfs:label><rdfs:label xml:lang="it">alpaca</rdfs:label><rdfs:label xml:lang="nl">alpaca</rdfs:label><rdfs:label xml:lang="sv">alpacka</rdfs:label><rdfs:label xml:lang="fr">alpaga</rdfs:label><rdfs:label xml:lang="sr">alpaka</rdfs:label><rdfs:label xml:lang="el">μαλλί αλπακά</rdfs:label><rdfs:label xml:lang="he">אלפקה</rdfs:label><skos:exactMatch rdf:resource="http://vocab.getty.edu/aat/300014030"/><skos:scopeNote xml:lang="en">Long, fine, soft hair of Peruvian alpacas. The term may be used to refer to a style of fabric originally made from alpaca hair but now often made from mohair, Icelandic sheep wool, or English wool. (AAT)</skos:scopeNote></owl:Class><owl:Class rdf:about="http://thesaurus.europeanafashion.eu/thesaurus/10814"><rdfs:subClassOf rdf:resource="http://thesaurus.europeanafashion.eu/thesaurus/10351"/><rdfs:label xml:lang="de">Kaschmir</rdfs:label><rdfs:label xml:lang="fr">cachemire</rdfs:label><rdfs:label xml:lang="en">cashmere</rdfs:label><rdfs:label xml:lang="es">cashmere</rdfs:label><rdfs:label xml:lang="it">cashmere</rdfs:label><rdfs:label xml:lang="sv">kashmir</rdfs:label><rdfs:label xml:lang="nl">kasjmier</rdfs:label><rdfs:label xml:lang="sr">kašmir</rdfs:label><rdfs:label xml:lang="el">κασμίρ</rdfs:label><rdfs:label xml:lang="he">צמר או סיב האלפקה</rdfs:label><rdfs:label xml:lang="he">קשמיר</rdfs:label><skos:exactMatch rdf:resource="http://vocab.getty.edu/aat/300192990"/><skos:scopeNote xml:lang="en">Fine, soft, light wool from the undercoat of the Kashmir goat; also yarn or fabric made from the wool. (AAT)</skos:scopeNote></owl:Class><owl:Class rdf:about="http://thesaurus.europeanafashion.eu/thesaurus/10912"><rdfs:subClassOf rdf:resource="http://thesaurus.europeanafashion.eu/thesaurus/10351"/><rdfs:label xml:lang="de">Merinowolle</rdfs:label><rdfs:label xml:lang="it">lana merino</rdfs:label><rdfs:label xml:lang="nl">merino</rdfs:label><rdfs:label xml:lang="en">merino (wool)</rdfs:label><rdfs:label xml:lang="sr">merino vuna</rdfs:label><rdfs:label xml:lang="sv">merinoull</rdfs:label><rdfs:label xml:lang="fr">mérinos</rdfs:label><rdfs:label xml:lang="el">μαλλί μερινό</rdfs:label><rdfs:label xml:lang="he">צמר מרינו</rdfs:label><skos:exactMatch rdf:resource="http://vocab.getty.edu/aat/300380171"/><skos:scopeNote xml:lang="en">Fine, soft, light wool from merino sheep resembling cashmere; also yarn or fabric made from the wool, sometimes in combination with cotton. By extension any fine woolen yarn used in knitwear. (AAT)</skos:scopeNote></owl:Class><owl:Class rdf:about="http://thesaurus.europeanafashion.eu/thesaurus/10913"><rdfs:subClassOf rdf:resource="http://thesaurus.europeanafashion.eu/thesaurus/10351"/><rdfs:label xml:lang="de">Lammwolle</rdfs:label><rdfs:label xml:lang="sr">jagnjeća vuna</rdfs:label><rdfs:label xml:lang="fr">laine d'agneau</rdfs:label><rdfs:label xml:lang="en">lamb's wool</rdfs:label><rdfs:label xml:lang="sv">lammull</rdfs:label><rdfs:label xml:lang="nl">lamswol</rdfs:label><rdfs:label xml:lang="it">lana d'agnello</rdfs:label><rdfs:label xml:lang="el">μαλλί προβάτου</rdfs:label><rdfs:label xml:lang="he">צמר טלה</rdfs:label><skos:exactMatch rdf:resource="http://vocab.getty.edu/aat/300264680"/><skos:scopeNote xml:lang="en">Wool shorn from a lamb seven to eight months old. (AAT)</skos:scopeNote></owl:Class><owl:Class rdf:about="http://thesaurus.europeanafashion.eu/thesaurus/10914"><rdfs:subClassOf rdf:resource="http://thesaurus.europeanafashion.eu/thesaurus/10351"/><rdfs:label xml:lang="de">Kammgarn (Wolle)</rdfs:label><rdfs:label xml:lang="nl">kamgaren</rdfs:label><rdfs:label xml:lang="sv">kamgarn</rdfs:label><rdfs:label xml:lang="fr">laine peignée</rdfs:label><rdfs:label xml:lang="it">lana pettinata</rdfs:label><rdfs:label xml:lang="en">worsted yarn</rdfs:label><rdfs:label xml:lang="sr">češljana vuna</rdfs:label><rdfs:label xml:lang="el">νήμα πλεξίματος</rdfs:label><rdfs:label xml:lang="he">חוט (צמר) שזור וסרוק</rdfs:label><skos:exactMatch rdf:resource="http://vocab.getty.edu/aat/300227943"/><skos:scopeNote xml:lang="en">Smooth compact yarn spun with average to hard twist from long wool fibers that have been carded and combed. (AAT)</skos:scopeNote></owl:Class><owl:Class rdf:about="http://thesaurus.europeanafashion.eu/thesaurus/10915"><rdfs:subClassOf rdf:resource="http://thesaurus.europeanafashion.eu/thesaurus/10352"/><rdfs:label xml:lang="de">Shantung</rdfs:label><rdfs:label xml:lang="nl">shantoeng</rdfs:label><rdfs:label xml:lang="en">shantung</rdfs:label><rdfs:label xml:lang="fr">shantung</rdfs:label><rdfs:label xml:lang="it">shantung</rdfs:label><rdfs:label xml:lang="nl">shantung</rdfs:label><rdfs:label xml:lang="sv">shantungsiden</rdfs:label><rdfs:label xml:lang="en">wild sikl</rdfs:label><rdfs:label xml:lang="sr">šantung svila</rdfs:label><rdfs:label xml:lang="el">σαντούγκ</rdfs:label><rdfs:label xml:lang="he">שנטונג</rdfs:label></owl:Class><owl:Class rdf:about="http://thesaurus.europeanafashion.eu/thesaurus/10532"><rdfs:subClassOf rdf:resource="http://thesaurus.europeanafashion.eu/thesaurus/10531"/><rdfs:label xml:lang="de">Ziegenhaar</rdfs:label><rdfs:label xml:lang="nl">geitenhaar</rdfs:label><rdfs:label xml:lang="sv">gethår</rdfs:label><rdfs:label xml:lang="en">goat hair</rdfs:label><rdfs:label xml:lang="sr">kozja dlaka</rdfs:label><rdfs:label xml:lang="es">pelo de cabra</rdfs:label><rdfs:label xml:lang="it">pelo di capra</rdfs:label><rdfs:label xml:lang="fr">poil de chèvre</rdfs:label><rdfs:label xml:lang="el">τρίχα κατσίκας</rdfs:label><rdfs:label xml:lang="he">שיער עז</rdfs:label><skos:exactMatch rdf:resource="http://vocab.getty.edu/aat/300011818"/><skos:scopeNote xml:lang="en">The hair or hair plus skin of the goat, which is a ruminant quadruped of the genus Capra. (AAT)</skos:scopeNote></owl:Class><owl:Class rdf:about="http://thesaurus.europeanafashion.eu/thesaurus/10533"><rdfs:subClassOf rdf:resource="http://thesaurus.europeanafashion.eu/thesaurus/10531"/><rdfs:label xml:lang="de">Pferdehaar</rdfs:label><rdfs:label xml:lang="de">Rosshaar</rdfs:label><rdfs:label xml:lang="es">crin</rdfs:label><rdfs:label xml:lang="fr">crin</rdfs:label><rdfs:label xml:lang="it">crini di cavallo</rdfs:label><rdfs:label xml:lang="en">horsehair</rdfs:label><rdfs:label xml:lang="sr">konjska dlaka</rdfs:label><rdfs:label xml:lang="nl">paardenhaar</rdfs:label><rdfs:label xml:lang="sv">tagel</rdfs:label><rdfs:label xml:lang="el">τρίχα αλόγου</rdfs:label><rdfs:label xml:lang="he">שיער סוס</rdfs:label><skos:exactMatch rdf:resource="http://vocab.getty.edu/aat/300011819"/><skos:scopeNote xml:lang="en">Hair from the manes and tails of horses, used chiefly as a brush fiber, for musical instrument bows, and for making haircloth.(AAT)</skos:scopeNote></owl:Class><owl:Class rdf:about="http://thesaurus.europeanafashion.eu/thesaurus/10953"><rdfs:subClassOf rdf:resource="http://thesaurus.europeanafashion.eu/thesaurus/10531"/><rdfs:label xml:lang="de">Kamelhaar</rdfs:label><rdfs:label xml:lang="en">camel hair</rdfs:label><rdfs:label xml:lang="it">crini di cammello</rdfs:label><rdfs:label xml:lang="nl">kamelenhaar</rdfs:label><rdfs:label xml:lang="sv">kamelhår</rdfs:label><rdfs:label xml:lang="sr">kamilhar</rdfs:label><rdfs:label xml:lang="sr">kamilja dlaka</rdfs:label><rdfs:label xml:lang="fr">poil de chameau</rdfs:label><rdfs:label xml:lang="el">τρίχα καμήλας</rdfs:label><rdfs:label xml:lang="he">שיער גמלים</rdfs:label><skos:exactMatch rdf:resource="http://vocab.getty.edu/aat/300011816"/><skos:scopeNote xml:lang="en">Fine body hair, or camel wool, used as a textile fiber. For artists' brushes usually made from the hair of squirrels, use camel hair brushes. (AAT)</skos:scopeNote></owl:Class><owl:Class rdf:about="http://thesaurus.europeanafashion.eu/thesaurus/10504"><rdfs:subClassOf rdf:resource="http://thesaurus.europeanafashion.eu/thesaurus/10534"/><rdfs:label xml:lang="de">Leder</rdfs:label><rdfs:label xml:lang="es">cuero</rdfs:label><rdfs:label xml:lang="fr">cuir</rdfs:label><rdfs:label xml:lang="it">cuoio</rdfs:label><rdfs:label xml:lang="sr">koža</rdfs:label><rdfs:label xml:lang="en">leather</rdfs:label><rdfs:label xml:lang="nl">leder</rdfs:label><rdfs:label xml:lang="nl">leer</rdfs:label><rdfs:label xml:lang="sv">läder</rdfs:label><rdfs:label xml:lang="sv">skinn</rdfs:label><rdfs:label xml:lang="el">δέρμα</rdfs:label><rdfs:label xml:lang="he">עור</rdfs:label><skos:exactMatch rdf:resource="http://vocab.getty.edu/aat/300011845"/><skos:scopeNote xml:lang="en">The skin or hide of an animal that has been tanned to render it resistant to putrefication and relatively soft and flexible when dry. For composite material made from scrap leather pieces, use maril. (AAT)</skos:scopeNote></owl:Class><owl:Class rdf:about="http://thesaurus.europeanafashion.eu/thesaurus/10536"><rdfs:subClassOf rdf:resource="http://thesaurus.europeanafashion.eu/thesaurus/10534"/><rdfs:label xml:lang="de">Chevreauleder</rdfs:label><rdfs:label xml:lang="de">Ziegenleder</rdfs:label><rdfs:label xml:lang="nl">geitenleer</rdfs:label><rdfs:label xml:lang="sv">getskinn</rdfs:label><rdfs:label xml:lang="en">goat skin</rdfs:label><rdfs:label xml:lang="sr">kozja koža</rdfs:label><rdfs:label xml:lang="fr">peau de chèvre</rdfs:label><rdfs:label xml:lang="it">pelle di capra</rdfs:label><rdfs:label xml:lang="es">piel de cabra</rdfs:label><rdfs:label xml:lang="el">δέρμα κατσίκας</rdfs:label><rdfs:label xml:lang="he">עור עז</rdfs:label><skos:exactMatch rdf:resource="http://vocab.getty.edu/aat/300255984"/><skos:scopeNote xml:lang="en">The skin of a goat; often tanned as a leather and used in the book and garment trades. (AAT)</skos:scopeNote></owl:Class><owl:Class rdf:about="http://thesaurus.europeanafashion.eu/thesaurus/10538"><rdfs:subClassOf rdf:resource="http://thesaurus.europeanafashion.eu/thesaurus/10534"/><rdfs:label xml:lang="de">Schafleder</rdfs:label><rdfs:label xml:lang="de">Schafpelz</rdfs:label><rdfs:label xml:lang="de">Schafsfell</rdfs:label><rdfs:label xml:lang="de">Schafspelz</rdfs:label><rdfs:label xml:lang="sv">fårskinn</rdfs:label><rdfs:label xml:lang="sr">ovčija koža</rdfs:label><rdfs:label xml:lang="fr">peau de mouton</rdfs:label><rdfs:label xml:lang="it">pelle di pecora</rdfs:label><rdfs:label xml:lang="es">piel de oveja</rdfs:label><rdfs:label xml:lang="nl">schapenleer</rdfs:label><rdfs:label xml:lang="en">sheep skin</rdfs:label><rdfs:label xml:lang="el">δέρμα αρνιού</rdfs:label><rdfs:label xml:lang="he">עור כבשים</rdfs:label><skos:exactMatch rdf:resource="http://vocab.getty.edu/aat/300193374"/><skos:scopeNote xml:lang="en">The skin of a sheep, with or without wool left on, prepared for any of various uses such as in garments, as leather or as parchment. The leather made from sheepskin is soft with little grain, and is not particularly durable. (AAT)</skos:scopeNote></owl:Class><owl:Class rdf:about="http://thesaurus.europeanafashion.eu/thesaurus/10684"><rdfs:subClassOf rdf:resource="http://thesaurus.europeanafashion.eu/thesaurus/10534"/><rdfs:label xml:lang="de">Reptilhaut</rdfs:label><rdfs:label xml:lang="de">Reptilienleder</rdfs:label><rdfs:label xml:lang="de">Reptilleder</rdfs:label><rdfs:label xml:lang="sr">koža gmizavca</rdfs:label><rdfs:label xml:lang="fr">peau de reptile</rdfs:label><rdfs:label xml:lang="it">pelle di rettile</rdfs:label><rdfs:label xml:lang="es">piel de reptil</rdfs:label><rdfs:label xml:lang="nl">reptielleer</rdfs:label><rdfs:label xml:lang="en">reptile skin</rdfs:label><rdfs:label xml:lang="sv">reptilskinn</rdfs:label><rdfs:label xml:lang="el">δέρμα ερπετού</rdfs:label><rdfs:label xml:lang="he">עור זחלים</rdfs:label></owl:Class><owl:Class rdf:about="http://thesaurus.europeanafashion.eu/thesaurus/10685"><rdfs:subClassOf rdf:resource="http://thesaurus.europeanafashion.eu/thesaurus/10534"/><rdfs:label xml:lang="de">Schweinsleder</rdfs:label><rdfs:label xml:lang="fr">peau de porc</rdfs:label><rdfs:label xml:lang="it">pelle di maiale</rdfs:label><rdfs:label xml:lang="es">piel de cerdo</rdfs:label><rdfs:label xml:lang="en">pig skin</rdfs:label><rdfs:label xml:lang="sr">svinjska koža</rdfs:label><rdfs:label xml:lang="sv">svinläder</rdfs:label><rdfs:label xml:lang="nl">varkensleer</rdfs:label><rdfs:label xml:lang="el">δέρμα χοίρου</rdfs:label><rdfs:label xml:lang="he">עור חזיר</rdfs:label></owl:Class><owl:Class rdf:about="http://thesaurus.europeanafashion.eu/thesaurus/10686"><rdfs:subClassOf rdf:resource="http://thesaurus.europeanafashion.eu/thesaurus/10534"/><rdfs:label xml:lang="de">Hirschleder</rdfs:label><rdfs:label xml:lang="fr">daim</rdfs:label><rdfs:label xml:lang="en">deer skin</rdfs:label><rdfs:label xml:lang="sr">jelenska koža</rdfs:label><rdfs:label xml:lang="it">pelle di cervo</rdfs:label><rdfs:label xml:lang="es">piel de ciervo</rdfs:label><rdfs:label xml:lang="nl">reeleer</rdfs:label><rdfs:label xml:lang="sv">rådjursskinn</rdfs:label><rdfs:label xml:lang="el">δέρμα ελαφιού</rdfs:label><rdfs:label xml:lang="he">עור צבי</rdfs:label></owl:Class><owl:Class rdf:about="http://thesaurus.europeanafashion.eu/thesaurus/10687"><rdfs:subClassOf rdf:resource="http://thesaurus.europeanafashion.eu/thesaurus/10534"/><rdfs:label xml:lang="de">Fischhaut</rdfs:label><rdfs:label xml:lang="de">Fischleder</rdfs:label><rdfs:label xml:lang="en">fish skin</rdfs:label><rdfs:label xml:lang="sv">fiskskinn</rdfs:label><rdfs:label xml:lang="fr">peau de poisson</rdfs:label><rdfs:label xml:lang="it">pelle di pesce</rdfs:label><rdfs:label xml:lang="es">piel de pescado</rdfs:label><rdfs:label xml:lang="sr">riblja koža</rdfs:label><rdfs:label xml:lang="nl">vissenleer</rdfs:label><rdfs:label xml:lang="el">δέρμα ψαριού</rdfs:label><rdfs:label xml:lang="he">עור דג</rdfs:label></owl:Class><owl:Class rdf:about="http://thesaurus.europeanafashion.eu/thesaurus/10688"><rdfs:subClassOf rdf:resource="http://thesaurus.europeanafashion.eu/thesaurus/10534"/><rdfs:label xml:lang="de">Vogelbalg</rdfs:label><rdfs:label xml:lang="de">Vogelhaut mit Federkleid</rdfs:label><rdfs:label xml:lang="en">bird skin</rdfs:label><rdfs:label xml:lang="sv">fågelskinn</rdfs:label><rdfs:label xml:lang="sr">koža ptice</rdfs:label><rdfs:label xml:lang="fr">peau d'oiseau</rdfs:label><rdfs:label xml:lang="it">pelle di uccello</rdfs:label><rdfs:label xml:lang="es">piel de pájaro</rdfs:label><rdfs:label xml:lang="nl">vogelhuid</rdfs:label><rdfs:label xml:lang="el">δέρμα πουλιού</rdfs:label><rdfs:label xml:lang="he">עור ציפור</rdfs:label><skos:exactMatch rdf:resource="http://vocab.getty.edu/aat/300379982"/><skos:scopeNote xml:lang="en">The skin of a bird, generally with feathers still attached. (AAT)</skos:scopeNote></owl:Class><owl:Class rdf:about="http://thesaurus.europeanafashion.eu/thesaurus/10750"><rdfs:subClassOf rdf:resource="http://thesaurus.europeanafashion.eu/thesaurus/10534"/><rdfs:label xml:lang="de">Antilopenleder</rdfs:label><rdfs:label xml:lang="en">antelope skin</rdfs:label><rdfs:label xml:lang="nl">antelopeleer</rdfs:label><rdfs:label xml:lang="sv">antilopskinn</rdfs:label><rdfs:label xml:lang="sr">koža antilope</rdfs:label><rdfs:label xml:lang="fr">peau d'antilope</rdfs:label><rdfs:label xml:lang="it">pelle di antilope</rdfs:label><rdfs:label xml:lang="es">piel de antílope</rdfs:label><rdfs:label xml:lang="el">δέρμα αντιλόπης</rdfs:label><rdfs:label xml:lang="he">עור אנטילופה</rdfs:label></owl:Class><owl:Class rdf:about="http://thesaurus.europeanafashion.eu/thesaurus/10751"><rdfs:subClassOf rdf:resource="http://thesaurus.europeanafashion.eu/thesaurus/10534"/><rdfs:label xml:lang="de">Haihaut</rdfs:label><rdfs:label xml:lang="de">Haileder</rdfs:label><rdfs:label xml:lang="nl">haaienleer</rdfs:label><rdfs:label xml:lang="sv">hajskinn</rdfs:label><rdfs:label xml:lang="sr">koža ajkule</rdfs:label><rdfs:label xml:lang="fr">peau de requin</rdfs:label><rdfs:label xml:lang="it">pelle di squalo</rdfs:label><rdfs:label xml:lang="es">piel de tiburón</rdfs:label><rdfs:label xml:lang="en">sharkskin</rdfs:label><rdfs:label xml:lang="el">δέρμα καρχαρία</rdfs:label><rdfs:label xml:lang="he">עור כריש</rdfs:label></owl:Class><owl:Class rdf:about="http://thesaurus.europeanafashion.eu/thesaurus/10923"><rdfs:subClassOf rdf:resource="http://thesaurus.europeanafashion.eu/thesaurus/10534"/><rdfs:label xml:lang="de">Rindsleder</rdfs:label><rdfs:label xml:lang="en">cowhide</rdfs:label><rdfs:label xml:lang="nl">koeienhuid</rdfs:label><rdfs:label xml:lang="sv">kohud</rdfs:label><rdfs:label xml:lang="sv">koskinn</rdfs:label><rdfs:label xml:lang="sr">kravlja koža</rdfs:label><rdfs:label xml:lang="fr">peau de vache</rdfs:label><rdfs:label xml:lang="it">vacchetta</rdfs:label><rdfs:label xml:lang="el">δέρμα αγελάδας</rdfs:label><rdfs:label xml:lang="he">עור פרה</rdfs:label><skos:exactMatch rdf:resource="http://vocab.getty.edu/aat/300265542"/><skos:scopeNote xml:lang="en">Hide of a cow, or the leather made from this hide. (AAT)</skos:scopeNote></owl:Class><owl:Class rdf:about="http://thesaurus.europeanafashion.eu/thesaurus/10924"><rdfs:subClassOf rdf:resource="http://thesaurus.europeanafashion.eu/thesaurus/10534"/><rdfs:label xml:lang="de">Löwenfell</rdfs:label><rdfs:label xml:lang="sr">lavlja koža</rdfs:label><rdfs:label xml:lang="nl">leeuwenhuid</rdfs:label><rdfs:label xml:lang="sv">lejonskinn</rdfs:label><rdfs:label xml:lang="en">lion skin</rdfs:label><rdfs:label xml:lang="fr">peau de lion</rdfs:label><rdfs:label xml:lang="it">pelle di leone</rdfs:label><rdfs:label xml:lang="el">δέρμα λιονταριού</rdfs:label><rdfs:label xml:lang="he">עור אריה</rdfs:label><skos:exactMatch rdf:resource="http://vocab.getty.edu/aat/300343608"/><skos:scopeNote xml:lang="en">The skin of a lion, generally with hair including mane attached. (AAT)</skos:scopeNote></owl:Class><owl:Class rdf:about="http://thesaurus.europeanafashion.eu/thesaurus/11081"><rdfs:subClassOf rdf:resource="http://thesaurus.europeanafashion.eu/thesaurus/10534"/><rdfs:label xml:lang="de">Elefantenhaut</rdfs:label><rdfs:label xml:lang="sv">elefanthud</rdfs:label><rdfs:label xml:lang="en">elephant skin</rdfs:label><rdfs:label xml:lang="nl">olifantenhuid</rdfs:label><rdfs:label xml:lang="fr">peau d'éléphant</rdfs:label><rdfs:label xml:lang="it">pelle di elefante</rdfs:label><rdfs:label xml:lang="sr">slonovska koža</rdfs:label><rdfs:label xml:lang="el">δέρμα ελέφαντα</rdfs:label><rdfs:label xml:lang="he">עור פיל</rdfs:label></owl:Class><owl:Class rdf:about="http://thesaurus.europeanafashion.eu/thesaurus/10689"><rdfs:subClassOf rdf:resource="http://thesaurus.europeanafashion.eu/thesaurus/10504"/><rdfs:label xml:lang="de">Rindleder</rdfs:label><rdfs:label xml:lang="de">Rindsleder</rdfs:label><rdfs:label xml:lang="en">bovine leather</rdfs:label><rdfs:label xml:lang="fr">cuir de vachette</rdfs:label><rdfs:label xml:lang="sr">goveđa koža</rdfs:label><rdfs:label xml:lang="sv">nötkreatursskinn</rdfs:label><rdfs:label xml:lang="it">pelle bovina</rdfs:label><rdfs:label xml:lang="es">piel de vaca</rdfs:label><rdfs:label xml:lang="nl">rundleer</rdfs:label><rdfs:label xml:lang="el">δέρμα βοδιού</rdfs:label><rdfs:label xml:lang="he">פרווה</rdfs:label></owl:Class><owl:Class rdf:about="http://thesaurus.europeanafashion.eu/thesaurus/10748"><rdfs:subClassOf rdf:resource="http://thesaurus.europeanafashion.eu/thesaurus/10504"/><rdfs:label xml:lang="de">Wildleder</rdfs:label><rdfs:label xml:lang="es">ante</rdfs:label><rdfs:label xml:lang="sr">antilop</rdfs:label><rdfs:label xml:lang="fr">daim</rdfs:label><rdfs:label xml:lang="sv">mocka</rdfs:label><rdfs:label xml:lang="it">pelle scamosciata</rdfs:label><rdfs:label xml:lang="en">suede</rdfs:label><rdfs:label xml:lang="fr">suède</rdfs:label><rdfs:label xml:lang="nl">suède</rdfs:label><rdfs:label xml:lang="el">σουέτ</rdfs:label><rdfs:label xml:lang="he">זמש</rdfs:label><skos:exactMatch rdf:resource="http://vocab.getty.edu/aat/300193368"/><skos:scopeNote xml:lang="en">Leather finished by buffing on an emery wheel, usually on the flesh side to produce a napped surface. Distinct from rough calf which is always finished on the flesh side and not polished with an emery wheel. (AAT)</skos:scopeNote></owl:Class><owl:Class rdf:about="http://thesaurus.europeanafashion.eu/thesaurus/10752"><rdfs:subClassOf rdf:resource="http://thesaurus.europeanafashion.eu/thesaurus/10504"/><rdfs:label xml:lang="de">Kunstleder</rdfs:label><rdfs:label xml:lang="nl">imitatieleer</rdfs:label><rdfs:label xml:lang="en">imitation leather</rdfs:label><rdfs:label xml:lang="sv">konstläder</rdfs:label><rdfs:label xml:lang="nl">kunstleer</rdfs:label><rdfs:label xml:lang="en">leatherette</rdfs:label><rdfs:label xml:lang="it">leatherette® (fintapelle)</rdfs:label><rdfs:label xml:lang="es">polipiel</rdfs:label><rdfs:label xml:lang="fr">similicuir</rdfs:label><rdfs:label xml:lang="sr">veštačka koža</rdfs:label><rdfs:label xml:lang="el">δερματίνη</rdfs:label><rdfs:label xml:lang="he">דמוי עור</rdfs:label></owl:Class><owl:Class rdf:about="http://thesaurus.europeanafashion.eu/thesaurus/10753"><rdfs:subClassOf rdf:resource="http://thesaurus.europeanafashion.eu/thesaurus/10504"/><rdfs:label xml:lang="de">Lackleder</rdfs:label><rdfs:label xml:lang="es">charol</rdfs:label><rdfs:label xml:lang="fr">cuir vernis</rdfs:label><rdfs:label xml:lang="sv">lackskinn</rdfs:label><rdfs:label xml:lang="sr">lak</rdfs:label><rdfs:label xml:lang="nl">lakleer</rdfs:label><rdfs:label xml:lang="en">patent leather</rdfs:label><rdfs:label xml:lang="it">vernice</rdfs:label><rdfs:label xml:lang="el">λουστρίνι</rdfs:label><rdfs:label xml:lang="he">לכה</rdfs:label><skos:exactMatch rdf:resource="http://vocab.getty.edu/aat/300193362"/><skos:scopeNote xml:lang="en">Cattle- or horse-hide leather, one side of which is covered with a flexible waterproof film having a lustrous and highly glazed surface produced by successive coats of daub, varnish, and lacquer. (AAT)</skos:scopeNote></owl:Class><owl:Class rdf:about="http://thesaurus.europeanafashion.eu/thesaurus/10794"><rdfs:subClassOf rdf:resource="http://thesaurus.europeanafashion.eu/thesaurus/10504"/><rdfs:label xml:lang="de">Straußenleder</rdfs:label><rdfs:label xml:lang="sr">koža noja</rdfs:label><rdfs:label xml:lang="en">ostrich leather</rdfs:label><rdfs:label xml:lang="fr">peau d'autruche</rdfs:label><rdfs:label xml:lang="it">pelle di struzzo</rdfs:label><rdfs:label xml:lang="nl">struisvogelleer</rdfs:label><rdfs:label xml:lang="sv">strutsskinn</rdfs:label><rdfs:label xml:lang="el">δέρμα στρουθοκαμήλου</rdfs:label><rdfs:label xml:lang="he">עור בת יענה</rdfs:label></owl:Class><owl:Class rdf:about="http://thesaurus.europeanafashion.eu/thesaurus/10810"><rdfs:subClassOf rdf:resource="http://thesaurus.europeanafashion.eu/thesaurus/10504"/><rdfs:label xml:lang="de">Chamois</rdfs:label><rdfs:label xml:lang="de">Chamoisleder</rdfs:label><rdfs:label xml:lang="de">Gamsleder</rdfs:label><rdfs:label xml:lang="de">Sämischleder</rdfs:label><rdfs:label xml:lang="sr">antilop</rdfs:label><rdfs:label xml:lang="it">camoscio</rdfs:label><rdfs:label xml:lang="en">chamois</rdfs:label><rdfs:label xml:lang="sr">jelenska koža</rdfs:label><rdfs:label xml:lang="fr">peau de chamois</rdfs:label><rdfs:label xml:lang="sv">sämskskinn</rdfs:label><rdfs:label xml:lang="nl">zeemleer</rdfs:label><rdfs:label xml:lang="el">σαμουά</rdfs:label><rdfs:label xml:lang="he">עור יעלים</rdfs:label><skos:exactMatch rdf:resource="http://vocab.getty.edu/aat/300032341"/><skos:scopeNote xml:lang="en">Soft, pliable oil-tanned leather originally made from the skins of the chamois, Antilopa rupicapra, a small deer; now made from the skins of lamb, sheep, goat, or from the flesh split of skins or hides. (AAT)</skos:scopeNote></owl:Class><owl:Class rdf:about="http://thesaurus.europeanafashion.eu/thesaurus/10537"><rdfs:subClassOf rdf:resource="http://thesaurus.europeanafashion.eu/thesaurus/10536"/><rdfs:label xml:lang="de">Chevreauleder</rdfs:label><rdfs:label xml:lang="de">Ziegenleder (junge Ziege)</rdfs:label><rdfs:label xml:lang="nl">geitenleer (jonge geiten)</rdfs:label><rdfs:label xml:lang="sr">jareća koža</rdfs:label><rdfs:label xml:lang="en">kidskin</rdfs:label><rdfs:label xml:lang="sv">killingskinn</rdfs:label><rdfs:label xml:lang="fr">peau de chevreau</rdfs:label><rdfs:label xml:lang="it">pelle di capretto</rdfs:label><rdfs:label xml:lang="es">piel de cabritilla</rdfs:label><rdfs:label xml:lang="el">δέρμα κατσικιού</rdfs:label><rdfs:label xml:lang="he">עור גדי</rdfs:label><skos:exactMatch rdf:resource="http://vocab.getty.edu/aat/300255987"/><skos:scopeNote xml:lang="en">The skin, usually of a young goat, occasionally a young lamb or related young animal, which when tanned, tawed, or manufactured, commonly finds use in the bookbinding and garment trades. (AAT)</skos:scopeNote></owl:Class><owl:Class rdf:about="http://thesaurus.europeanafashion.eu/thesaurus/10745"><rdfs:subClassOf rdf:resource="http://thesaurus.europeanafashion.eu/thesaurus/10538"/><rdfs:label xml:lang="el">Breitschwanz</rdfs:label><rdfs:label xml:lang="en">Breitschwanz</rdfs:label><rdfs:label xml:lang="fr">Broadtail</rdfs:label><rdfs:label xml:lang="de">Karakul</rdfs:label><rdfs:label xml:lang="de">Persianer</rdfs:label><rdfs:label xml:lang="fr">caracul</rdfs:label><rdfs:label xml:lang="en">karakul</rdfs:label><rdfs:label xml:lang="es">karakul</rdfs:label><rdfs:label xml:lang="it">karakul</rdfs:label><rdfs:label xml:lang="nl">karakul</rdfs:label><rdfs:label xml:lang="sr">karakul</rdfs:label><rdfs:label xml:lang="sv">karakul</rdfs:label><rdfs:label xml:lang="el">γούνα karakul</rdfs:label><rdfs:label xml:lang="he">כבש קרקול</rdfs:label></owl:Class><owl:Class rdf:about="http://thesaurus.europeanafashion.eu/thesaurus/10747"><rdfs:subClassOf rdf:resource="http://thesaurus.europeanafashion.eu/thesaurus/10538"/><rdfs:label xml:lang="de">Astrachan</rdfs:label><rdfs:label xml:lang="de">Halbpersianer</rdfs:label><rdfs:label xml:lang="es">astracán</rdfs:label><rdfs:label xml:lang="sr">astragan</rdfs:label><rdfs:label xml:lang="fr">astrakan</rdfs:label><rdfs:label xml:lang="it">astrakan</rdfs:label><rdfs:label xml:lang="nl">astrakan</rdfs:label><rdfs:label xml:lang="sv">astrakan</rdfs:label><rdfs:label xml:lang="en">astrakhan</rdfs:label><rdfs:label xml:lang="fr">breitschwanz</rdfs:label><rdfs:label xml:lang="nl">breitschwanz</rdfs:label><rdfs:label xml:lang="el">γούνα αστρακάν</rdfs:label><rdfs:label xml:lang="he">אסטרחן</rdfs:label><skos:exactMatch rdf:resource="http://vocab.getty.edu/aat/300417874"/></owl:Class><owl:Class rdf:about="http://thesaurus.europeanafashion.eu/thesaurus/10535"><rdfs:subClassOf rdf:resource="http://thesaurus.europeanafashion.eu/thesaurus/10684"/><rdfs:label xml:lang="de">Schlangenhaut</rdfs:label><rdfs:label xml:lang="de">Schlangenleder</rdfs:label><rdfs:label xml:lang="sv">ormskinn</rdfs:label><rdfs:label xml:lang="fr">peau de serpent</rdfs:label><rdfs:label xml:lang="it">pelle di serpente</rdfs:label><rdfs:label xml:lang="es">piel de serpiente</rdfs:label><rdfs:label xml:lang="nl">slangenleer</rdfs:label><rdfs:label xml:lang="en">snake skin</rdfs:label><rdfs:label xml:lang="sr">zmijska koža</rdfs:label><rdfs:label xml:lang="el">δέρμα φιδιού</rdfs:label><rdfs:label xml:lang="he">עור נחש</rdfs:label><skos:exactMatch rdf:resource="http://vocab.getty.edu/aat/300011850"/><skos:scopeNote xml:lang="en">Vegetable-tanned, durable, thin leather made from the skins of snakes. (AAT)</skos:scopeNote></owl:Class><owl:Class rdf:about="http://thesaurus.europeanafashion.eu/thesaurus/10792"><rdfs:subClassOf rdf:resource="http://thesaurus.europeanafashion.eu/thesaurus/10684"/><rdfs:label xml:lang="de">Echsenleder</rdfs:label><rdfs:label xml:lang="de">Eidechsenleder</rdfs:label><rdfs:label xml:lang="nl">hagedissenleer</rdfs:label><rdfs:label xml:lang="sr">koža guštera</rdfs:label><rdfs:label xml:lang="en">lizard skin</rdfs:label><rdfs:label xml:lang="fr">peau de lézard</rdfs:label><rdfs:label xml:lang="it">pelle di lucertola</rdfs:label><rdfs:label xml:lang="es">piel de lagarto</rdfs:label><rdfs:label xml:lang="sv">ödleskin</rdfs:label><rdfs:label xml:lang="el">δέρμα σαύρας</rdfs:label><rdfs:label xml:lang="he">עור לטאה</rdfs:label><skos:exactMatch rdf:resource="http://vocab.getty.edu/aat/300011848"/><skos:scopeNote xml:lang="en">Leather derived from lizards, which in common usage refers to reptiles of the genus Lacerta as well as any other reptiles resembling these in shape and general appearance. (AAT)</skos:scopeNote></owl:Class><owl:Class rdf:about="http://thesaurus.europeanafashion.eu/thesaurus/10793"><rdfs:subClassOf rdf:resource="http://thesaurus.europeanafashion.eu/thesaurus/10684"/><rdfs:label xml:lang="de">Krokodilhaut</rdfs:label><rdfs:label xml:lang="de">Krokodilleder</rdfs:label><rdfs:label xml:lang="en">crocodile skin</rdfs:label><rdfs:label xml:lang="nl">krokodillenleer</rdfs:label><rdfs:label xml:lang="sr">krokodilska koža</rdfs:label><rdfs:label xml:lang="sv">krokodilskinn</rdfs:label><rdfs:label xml:lang="fr">peau de crocodile</rdfs:label><rdfs:label xml:lang="it">pelle di coccodrillo</rdfs:label><rdfs:label xml:lang="es">piel de cocodrilo</rdfs:label><rdfs:label xml:lang="el">δέρμα κροκοδείλου</rdfs:label><rdfs:label xml:lang="he">עור תנין</rdfs:label></owl:Class><owl:Class rdf:about="http://thesaurus.europeanafashion.eu/thesaurus/10855"><rdfs:subClassOf rdf:resource="http://thesaurus.europeanafashion.eu/thesaurus/10535"/><rdfs:label xml:lang="de">künstliches Schlangenleder</rdfs:label><rdfs:label xml:lang="sv">ormskinnsimitation</rdfs:label><rdfs:label xml:lang="fr">peau de serpent synthétique</rdfs:label><rdfs:label xml:lang="it">pelle di serpente sintetica</rdfs:label><rdfs:label xml:lang="sr">sintetička zmijska koža</rdfs:label><rdfs:label xml:lang="en">synthetic snakeskin</rdfs:label><rdfs:label xml:lang="nl">synthetisch slangenleer</rdfs:label><rdfs:label xml:lang="el">απομίμηση δέρματος φιδιού</rdfs:label><rdfs:label xml:lang="he">עור נחש סיתטי</rdfs:label></owl:Class><owl:Class rdf:about="http://thesaurus.europeanafashion.eu/thesaurus/10540"><rdfs:subClassOf rdf:resource="http://thesaurus.europeanafashion.eu/thesaurus/10539"/><rdfs:label xml:lang="de">Kaninchenpelz</rdfs:label><rdfs:label xml:lang="de">Kanninchenfell</rdfs:label><rdfs:label xml:lang="fr">fourrure de lapin</rdfs:label><rdfs:label xml:lang="sv">kaninpäls</rdfs:label><rdfs:label xml:lang="nl">konijnenbont</rdfs:label><rdfs:label xml:lang="it">pelliccia di coniglio</rdfs:label><rdfs:label xml:lang="es">piel de conejo</rdfs:label><rdfs:label xml:lang="en">rabbit fur</rdfs:label><rdfs:label xml:lang="sr">zečije krzno</rdfs:label><rdfs:label xml:lang="el">λαγοτόμαρο</rdfs:label><rdfs:label xml:lang="he">פרוות ארנב</rdfs:label><skos:exactMatch rdf:resource="http://vocab.getty.edu/aat/300386669"/><skos:scopeNote xml:lang="en">Hair derived from rabbits. (AAT)</skos:scopeNote></owl:Class><owl:Class rdf:about="http://thesaurus.europeanafashion.eu/thesaurus/10541"><rdfs:subClassOf rdf:resource="http://thesaurus.europeanafashion.eu/thesaurus/10539"/><rdfs:label xml:lang="de">Fuchsfell</rdfs:label><rdfs:label xml:lang="de">Fuchspelz</rdfs:label><rdfs:label xml:lang="fr">fourrure de renard</rdfs:label><rdfs:label xml:lang="en">fox fur</rdfs:label><rdfs:label xml:lang="sr">lisičije krzno</rdfs:label><rdfs:label xml:lang="it">pelliccia di volpe</rdfs:label><rdfs:label xml:lang="es">piel de zorro</rdfs:label><rdfs:label xml:lang="sv">rävpäls</rdfs:label><rdfs:label xml:lang="nl">vossenbont</rdfs:label><rdfs:label xml:lang="nl">vossenpels</rdfs:label><rdfs:label xml:lang="el">γούνα αλεπούς</rdfs:label><rdfs:label xml:lang="he">פרוות שועל</rdfs:label></owl:Class><owl:Class rdf:about="http://thesaurus.europeanafashion.eu/thesaurus/10542"><rdfs:subClassOf rdf:resource="http://thesaurus.europeanafashion.eu/thesaurus/10539"/><rdfs:label xml:lang="de">Bieberfell</rdfs:label><rdfs:label xml:lang="de">Bieberpelz</rdfs:label><rdfs:label xml:lang="en">beaver fur</rdfs:label><rdfs:label xml:lang="nl">beverbont</rdfs:label><rdfs:label xml:lang="nl">beverpels</rdfs:label><rdfs:label xml:lang="sv">bäverpäls</rdfs:label><rdfs:label xml:lang="es">castor</rdfs:label><rdfs:label xml:lang="fr">fourrure de castor</rdfs:label><rdfs:label xml:lang="sr">krzno dabra</rdfs:label><rdfs:label xml:lang="it">pelliccia di castoro</rdfs:label><rdfs:label xml:lang="el">γούνα κάστορα</rdfs:label><rdfs:label xml:lang="he">פרוות בונה</rdfs:label></owl:Class><owl:Class rdf:about="http://thesaurus.europeanafashion.eu/thesaurus/10690"><rdfs:subClassOf rdf:resource="http://thesaurus.europeanafashion.eu/thesaurus/10539"/><rdfs:label xml:lang="de">Nerzfell</rdfs:label><rdfs:label xml:lang="sr">krzno kanadske kune</rdfs:label><rdfs:label xml:lang="en">mink fur</rdfs:label><rdfs:label xml:lang="sv">minkpäls</rdfs:label><rdfs:label xml:lang="nl">nertsenbont</rdfs:label><rdfs:label xml:lang="nl">nertsenpels</rdfs:label><rdfs:label xml:lang="it">pelliccia di visone</rdfs:label><rdfs:label xml:lang="es">piel de visón</rdfs:label><rdfs:label xml:lang="fr">vison</rdfs:label><rdfs:label xml:lang="el">γούνα μινκ</rdfs:label><rdfs:label xml:lang="he">פרוות מינק</rdfs:label></owl:Class><owl:Class rdf:about="http://thesaurus.europeanafashion.eu/thesaurus/10754"><rdfs:subClassOf rdf:resource="http://thesaurus.europeanafashion.eu/thesaurus/10539"/><rdfs:label xml:lang="de">Kunstfell</rdfs:label><rdfs:label xml:lang="de">Kunstpelz</rdfs:label><rdfs:label xml:lang="de">Pelzimitat</rdfs:label><rdfs:label xml:lang="en">fake fur</rdfs:label><rdfs:label xml:lang="fr">fausse fourrure</rdfs:label><rdfs:label xml:lang="en">faux fur</rdfs:label><rdfs:label xml:lang="sv">fuskpäls</rdfs:label><rdfs:label xml:lang="nl">imitatiebont</rdfs:label><rdfs:label xml:lang="it">pelliccia sintetica</rdfs:label><rdfs:label xml:lang="es">piel de imitación</rdfs:label><rdfs:label xml:lang="es">piel sintética</rdfs:label><rdfs:label xml:lang="sr">veštačko krzno</rdfs:label><rdfs:label xml:lang="el">ψεύτικη γούνα</rdfs:label><rdfs:label xml:lang="he">פרווה מזויפת</rdfs:label></owl:Class><owl:Class rdf:about="http://thesaurus.europeanafashion.eu/thesaurus/10755"><rdfs:subClassOf rdf:resource="http://thesaurus.europeanafashion.eu/thesaurus/10539"/><rdfs:label xml:lang="de">Hermelinfell</rdfs:label><rdfs:label xml:lang="en">ermine fur</rdfs:label><rdfs:label xml:lang="nl">hermelijn</rdfs:label><rdfs:label xml:lang="sr">hermelin</rdfs:label><rdfs:label xml:lang="sv">hermelin</rdfs:label><rdfs:label xml:lang="fr">hermine</rdfs:label><rdfs:label xml:lang="it">pelliccia di ermellino</rdfs:label><rdfs:label xml:lang="es">piel de armiño</rdfs:label><rdfs:label xml:lang="el">γούνα ερμίνας</rdfs:label><rdfs:label xml:lang="he">פרוות סמור</rdfs:label></owl:Class><owl:Class rdf:about="http://thesaurus.europeanafashion.eu/thesaurus/10756"><rdfs:subClassOf rdf:resource="http://thesaurus.europeanafashion.eu/thesaurus/10539"/><rdfs:label xml:lang="de">Marderfell</rdfs:label><rdfs:label xml:lang="sr">krzno kune</rdfs:label><rdfs:label xml:lang="en">marten fur</rdfs:label><rdfs:label xml:lang="nl">marter</rdfs:label><rdfs:label xml:lang="fr">martre</rdfs:label><rdfs:label xml:lang="sv">mård</rdfs:label><rdfs:label xml:lang="it">pelliccia di martora</rdfs:label><rdfs:label xml:lang="es">piel de marta</rdfs:label><rdfs:label xml:lang="el">γούνα κουναβιού</rdfs:label><rdfs:label xml:lang="he">פרוות נמייה</rdfs:label></owl:Class><owl:Class rdf:about="http://thesaurus.europeanafashion.eu/thesaurus/10757"><rdfs:subClassOf rdf:resource="http://thesaurus.europeanafashion.eu/thesaurus/10539"/><rdfs:label xml:lang="de">Leopardenfell</rdfs:label><rdfs:label xml:lang="sr">krzno leoparda</rdfs:label><rdfs:label xml:lang="sv">leopard</rdfs:label><rdfs:label xml:lang="en">leopard fur</rdfs:label><rdfs:label xml:lang="nl">luipaard</rdfs:label><rdfs:label xml:lang="fr">léopard</rdfs:label><rdfs:label xml:lang="it">pelliccia di leopardo</rdfs:label><rdfs:label xml:lang="es">piel de leopardo</rdfs:label><rdfs:label xml:lang="el">γούνα λεοπάρ</rdfs:label><rdfs:label xml:lang="he">פרוות נמר</rdfs:label></owl:Class><owl:Class rdf:about="http://thesaurus.europeanafashion.eu/thesaurus/10758"><rdfs:subClassOf rdf:resource="http://thesaurus.europeanafashion.eu/thesaurus/10539"/><rdfs:label xml:lang="de">Robbenfell</rdfs:label><rdfs:label xml:lang="de">Seehundfell</rdfs:label><rdfs:label xml:lang="sr">krzno foke</rdfs:label><rdfs:label xml:lang="it">pelliccia di foca</rdfs:label><rdfs:label xml:lang="fr">phoque</rdfs:label><rdfs:label xml:lang="es">piel de foca</rdfs:label><rdfs:label xml:lang="en">seal fur</rdfs:label><rdfs:label xml:lang="sv">säl</rdfs:label><rdfs:label xml:lang="nl">zeehondenbont</rdfs:label><rdfs:label xml:lang="el">δέρμα φώκιας</rdfs:label><rdfs:label xml:lang="he">פרוות כלב ים</rdfs:label></owl:Class><owl:Class rdf:about="http://thesaurus.europeanafashion.eu/thesaurus/10759"><rdfs:subClassOf rdf:resource="http://thesaurus.europeanafashion.eu/thesaurus/10539"/><rdfs:label xml:lang="de">Chinchillafell</rdfs:label><rdfs:label xml:lang="fr">chinchilla</rdfs:label><rdfs:label xml:lang="nl">chinchilla</rdfs:label><rdfs:label xml:lang="sv">chinchilla</rdfs:label><rdfs:label xml:lang="en">chinchilla fur</rdfs:label><rdfs:label xml:lang="sr">krzno činčile</rdfs:label><rdfs:label xml:lang="it">pelliccia di cincillà</rdfs:label><rdfs:label xml:lang="es">piel de chinchilla</rdfs:label><rdfs:label xml:lang="el">γούνα τσιντσιλά</rdfs:label><rdfs:label xml:lang="he">פרוות צ'ינצ'ילה</rdfs:label></owl:Class><owl:Class rdf:about="http://thesaurus.europeanafashion.eu/thesaurus/10760"><rdfs:subClassOf rdf:resource="http://thesaurus.europeanafashion.eu/thesaurus/10539"/><rdfs:label xml:lang="de">Zobelfell</rdfs:label><rdfs:label xml:lang="fr">fourrure de zibeline</rdfs:label><rdfs:label xml:lang="it">pelliccia di zibellino</rdfs:label><rdfs:label xml:lang="es">piel de marta cibelina</rdfs:label><rdfs:label xml:lang="nl">sabelmarter</rdfs:label><rdfs:label xml:lang="en">sable fur</rdfs:label><rdfs:label xml:lang="sr">samurovina</rdfs:label><rdfs:label xml:lang="sv">sobel</rdfs:label><rdfs:label xml:lang="en">zibellina</rdfs:label><rdfs:label xml:lang="el">γούνα ζιμπελίνας</rdfs:label><rdfs:label xml:lang="he">פרוות צובל</rdfs:label></owl:Class><owl:Class rdf:about="http://thesaurus.europeanafashion.eu/thesaurus/10761"><rdfs:subClassOf rdf:resource="http://thesaurus.europeanafashion.eu/thesaurus/10539"/><rdfs:label xml:lang="de">Waschbärfell</rdfs:label><rdfs:label xml:lang="sr">krzno rakuna</rdfs:label><rdfs:label xml:lang="it">pelliccia di orsetto lavatore</rdfs:label><rdfs:label xml:lang="es">piel de mapache</rdfs:label><rdfs:label xml:lang="en">raccoon fur</rdfs:label><rdfs:label xml:lang="fr">raton laveur</rdfs:label><rdfs:label xml:lang="sv">sjubb</rdfs:label><rdfs:label xml:lang="nl">wasbeer</rdfs:label><rdfs:label xml:lang="el">γούνα ρακούν</rdfs:label><rdfs:label xml:lang="he">פרוות רקון</rdfs:label></owl:Class><owl:Class rdf:about="http://thesaurus.europeanafashion.eu/thesaurus/10762"><rdfs:subClassOf rdf:resource="http://thesaurus.europeanafashion.eu/thesaurus/10539"/><rdfs:label xml:lang="de">Otterfell</rdfs:label><rdfs:label xml:lang="sr">krzno vidre</rdfs:label><rdfs:label xml:lang="fr">loutre</rdfs:label><rdfs:label xml:lang="nl">otter</rdfs:label><rdfs:label xml:lang="en">otter fur</rdfs:label><rdfs:label xml:lang="it">pelliccia di lontra</rdfs:label><rdfs:label xml:lang="es">piel de nutria</rdfs:label><rdfs:label xml:lang="sv">utter</rdfs:label><rdfs:label xml:lang="el">γούνα βίδρας</rdfs:label><rdfs:label xml:lang="he">פרוות לוטרה</rdfs:label></owl:Class><owl:Class rdf:about="http://thesaurus.europeanafashion.eu/thesaurus/10930"><rdfs:subClassOf rdf:resource="http://thesaurus.europeanafashion.eu/thesaurus/10583"/><rdfs:label xml:lang="de">Schildkrötenimitat</rdfs:label><rdfs:label xml:lang="sr">imitacija kornjačevine</rdfs:label><rdfs:label xml:lang="nl">imitatieschildpad</rdfs:label><rdfs:label xml:lang="en">imitation turtle</rdfs:label><rdfs:label xml:lang="fr">imitation écaille de tortue</rdfs:label><rdfs:label xml:lang="it">imitazione di tartaruga</rdfs:label><rdfs:label xml:lang="sv">skölpaddsimitation</rdfs:label><rdfs:label xml:lang="el">απομίμηση ταρταρούγας</rdfs:label><rdfs:label xml:lang="he">דמוי שריון צב</rdfs:label></owl:Class><owl:Class rdf:about="http://thesaurus.europeanafashion.eu/thesaurus/10590"><rdfs:subClassOf rdf:resource="http://thesaurus.europeanafashion.eu/thesaurus/10589"/><rdfs:label xml:lang="de">Marabufeder</rdfs:label><rdfs:label xml:lang="nl">maraboeveer</rdfs:label><rdfs:label xml:lang="en">marabou feather</rdfs:label><rdfs:label xml:lang="sv">maraboustorkfjäder</rdfs:label><rdfs:label xml:lang="sr">marabu pero</rdfs:label><rdfs:label xml:lang="it">piuma di marabù</rdfs:label><rdfs:label xml:lang="es">pluma de marabú</rdfs:label><rdfs:label xml:lang="fr">plume de marabou</rdfs:label><rdfs:label xml:lang="el">φτερό μαραμπού</rdfs:label><rdfs:label xml:lang="he">נוצת מאראבו</rdfs:label><skos:exactMatch rdf:resource="http://vocab.getty.edu/aat/300419426"/></owl:Class><owl:Class rdf:about="http://thesaurus.europeanafashion.eu/thesaurus/10767"><rdfs:subClassOf rdf:resource="http://thesaurus.europeanafashion.eu/thesaurus/10589"/><rdfs:label xml:lang="de">Straußenfeder</rdfs:label><rdfs:label xml:lang="sr">nojevo pero</rdfs:label><rdfs:label xml:lang="en">ostrich feather</rdfs:label><rdfs:label xml:lang="it">piuma di struzzo</rdfs:label><rdfs:label xml:lang="es">pluma de avestruz</rdfs:label><rdfs:label xml:lang="fr">plume d'autruche</rdfs:label><rdfs:label xml:lang="nl">struisvogelveer</rdfs:label><rdfs:label xml:lang="sv">strutsfjäder</rdfs:label><rdfs:label xml:lang="el">φτερό στρουθοκαμήλου</rdfs:label><rdfs:label xml:lang="he">נוצת יען</rdfs:label></owl:Class><owl:Class rdf:about="http://thesaurus.europeanafashion.eu/thesaurus/10931"><rdfs:subClassOf rdf:resource="http://thesaurus.europeanafashion.eu/thesaurus/10589"/><rdfs:label xml:lang="de">Hahnenfeder</rdfs:label><rdfs:label xml:lang="en">cock feather</rdfs:label><rdfs:label xml:lang="nl">hanenveer</rdfs:label><rdfs:label xml:lang="sr">pero petla</rdfs:label><rdfs:label xml:lang="it">piuma di gallo</rdfs:label><rdfs:label xml:lang="fr">plume de coq</rdfs:label><rdfs:label xml:lang="sv">tuppfjäder</rdfs:label><rdfs:label xml:lang="el">φτερά κόκορα</rdfs:label><rdfs:label xml:lang="he">נוצת תרנגול</rdfs:label></owl:Class><owl:Class rdf:about="http://thesaurus.europeanafashion.eu/thesaurus/10932"><rdfs:subClassOf rdf:resource="http://thesaurus.europeanafashion.eu/thesaurus/10589"/><rdfs:label xml:lang="de">Daunen</rdfs:label><rdfs:label xml:lang="nl">donsveer</rdfs:label><rdfs:label xml:lang="fr">panache</rdfs:label><rdfs:label xml:lang="it">pennacchio</rdfs:label><rdfs:label xml:lang="sr">perjanica</rdfs:label><rdfs:label xml:lang="sr">pero</rdfs:label><rdfs:label xml:lang="nl">pluim</rdfs:label><rdfs:label xml:lang="en">plume</rdfs:label><rdfs:label xml:lang="fr">plumet</rdfs:label><rdfs:label xml:lang="sv">plym</rdfs:label><rdfs:label xml:lang="el">πούπουλο</rdfs:label><rdfs:label xml:lang="he">נוצת מצנפת</rdfs:label></owl:Class><owl:Class rdf:about="http://thesaurus.europeanafashion.eu/thesaurus/10354"><rdfs:subClassOf rdf:resource="http://thesaurus.europeanafashion.eu/thesaurus/10353"/><rdfs:label xml:lang="de">Baumwolle</rdfs:label><rdfs:label xml:lang="pt">algodão</rdfs:label><rdfs:label xml:lang="es">algodón</rdfs:label><rdfs:label xml:lang="sv">bomull</rdfs:label><rdfs:label xml:lang="fr">coton</rdfs:label><rdfs:label xml:lang="it">cotone</rdfs:label><rdfs:label xml:lang="en">cotton</rdfs:label><rdfs:label xml:lang="nl">katoen</rdfs:label><rdfs:label xml:lang="sr">pamuk</rdfs:label><rdfs:label xml:lang="el">βαμβάκι</rdfs:label><rdfs:label xml:lang="he">כותנה</rdfs:label><skos:exactMatch rdf:resource="http://vocab.getty.edu/aat/300183670"/><skos:scopeNote xml:lang="en">White-to-yellowish seed-hair fibers of several species of the genus Gossypium, native to most subtropical areas of the world; used especially for making textile, cord, padding, rag paper, and for cellulose used for plastic and rayon. (AAT)</skos:scopeNote></owl:Class><owl:Class rdf:about="http://thesaurus.europeanafashion.eu/thesaurus/10355"><rdfs:subClassOf rdf:resource="http://thesaurus.europeanafashion.eu/thesaurus/10353"/><rdfs:label xml:lang="de">Leinen</rdfs:label><rdfs:label xml:lang="es">estopa</rdfs:label><rdfs:label xml:lang="es">hilo, lienzo</rdfs:label><rdfs:label xml:lang="sr">lan</rdfs:label><rdfs:label xml:lang="fr">lin</rdfs:label><rdfs:label xml:lang="sv">lin</rdfs:label><rdfs:label xml:lang="en">linen</rdfs:label><rdfs:label xml:lang="pt">linho</rdfs:label><rdfs:label xml:lang="nl">linnen</rdfs:label><rdfs:label xml:lang="es">lino</rdfs:label><rdfs:label xml:lang="it">lino</rdfs:label><rdfs:label xml:lang="el">λινάρι</rdfs:label><rdfs:label xml:lang="he">פשתן</rdfs:label><skos:exactMatch rdf:resource="http://vocab.getty.edu/aat/300014069"/><skos:scopeNote xml:lang="en">General name for textile woven from the spun fiber of the flax plant. (AAT)</skos:scopeNote></owl:Class><owl:Class rdf:about="http://thesaurus.europeanafashion.eu/thesaurus/10357"><rdfs:subClassOf rdf:resource="http://thesaurus.europeanafashion.eu/thesaurus/10353"/><rdfs:label xml:lang="de">Alginatfaser</rdfs:label><rdfs:label xml:lang="it">fibra d'alghe</rdfs:label><rdfs:label xml:lang="es">fibra de algas</rdfs:label><rdfs:label xml:lang="pt">fibras de algas</rdfs:label><rdfs:label xml:lang="fr">fibres d'algues</rdfs:label><rdfs:label xml:lang="fr">fibres marines</rdfs:label><rdfs:label xml:lang="en">seaweed fibre</rdfs:label><rdfs:label xml:lang="sv">sjögräsfibrer</rdfs:label><rdfs:label xml:lang="sr">vlakno od morskih algi</rdfs:label><rdfs:label xml:lang="nl">zeewiervezels</rdfs:label><rdfs:label xml:lang="el">φύκια</rdfs:label><rdfs:label xml:lang="he">סיבים מאצות</rdfs:label></owl:Class><owl:Class rdf:about="http://thesaurus.europeanafashion.eu/thesaurus/10477"><rdfs:subClassOf rdf:resource="http://thesaurus.europeanafashion.eu/thesaurus/10353"/><rdfs:label xml:lang="de">Espartogras</rdfs:label><rdfs:label xml:lang="de">Esperto</rdfs:label><rdfs:label xml:lang="fr">alfa</rdfs:label><rdfs:label xml:lang="es">esparto</rdfs:label><rdfs:label xml:lang="nl">esparto</rdfs:label><rdfs:label xml:lang="pt">esparto</rdfs:label><rdfs:label xml:lang="en">esparto grass</rdfs:label><rdfs:label xml:lang="sr">esparto trava</rdfs:label><rdfs:label xml:lang="sv">espartogräs</rdfs:label><rdfs:label xml:lang="it">paglia di sparto</rdfs:label><rdfs:label xml:lang="el">σπάρτο</rdfs:label><rdfs:label xml:lang="he">סיבים האספרטו</rdfs:label><skos:exactMatch rdf:resource="http://vocab.getty.edu/aat/300014036"/><skos:scopeNote xml:lang="en">The fiber of the grass species Macrochloa tenacissima, used to make cordage, shoes, and paper. It is sometimes used in combination with the poorer quality with fiber from another species of tall grass, Lygeum spartum. Esparto fibers are used extensively in England and Scotland for the production of paper, but rarely used in the U.S. because wood pulp is plentiful there. (AAT)</skos:scopeNote></owl:Class><owl:Class rdf:about="http://thesaurus.europeanafashion.eu/thesaurus/10478"><rdfs:subClassOf rdf:resource="http://thesaurus.europeanafashion.eu/thesaurus/10353"/><rdfs:label xml:lang="de">Hanf</rdfs:label><rdfs:label xml:lang="it">canapa</rdfs:label><rdfs:label xml:lang="fr">chanvre</rdfs:label><rdfs:label xml:lang="es">cáñamo</rdfs:label><rdfs:label xml:lang="pt">cânhamo</rdfs:label><rdfs:label xml:lang="sv">hampa</rdfs:label><rdfs:label xml:lang="en">hemp</rdfs:label><rdfs:label xml:lang="nl">hennep</rdfs:label><rdfs:label xml:lang="sr">konoplja</rdfs:label><rdfs:label xml:lang="el">κάνναβη</rdfs:label><rdfs:label xml:lang="he">קנבוס</rdfs:label><skos:exactMatch rdf:resource="http://vocab.getty.edu/aat/300014043"/><skos:scopeNote xml:lang="en">Fiber derived from the stalk of the species Cannabis sativa. Fibers range from 1-2 m in length and are yellow to brown in color. They have a high cellulose content with little lignin. Hemp is lustrous, strong, and durable with good resistance to water, salts, light, and insects; used for cordage, fish lines, sailcloth, canvas, burlap, packing, and as a fiber for paper or for plastic filler. (AAT)</skos:scopeNote></owl:Class><owl:Class rdf:about="http://thesaurus.europeanafashion.eu/thesaurus/10479"><rdfs:subClassOf rdf:resource="http://thesaurus.europeanafashion.eu/thesaurus/10353"/><rdfs:label xml:lang="de">Jute</rdfs:label><rdfs:label xml:lang="it">juta</rdfs:label><rdfs:label xml:lang="pt">juta</rdfs:label><rdfs:label xml:lang="sr">juta</rdfs:label><rdfs:label xml:lang="en">jute</rdfs:label><rdfs:label xml:lang="fr">jute</rdfs:label><rdfs:label xml:lang="nl">jute</rdfs:label><rdfs:label xml:lang="sv">jute</rdfs:label><rdfs:label xml:lang="es">yute</rdfs:label><rdfs:label xml:lang="el">γιούτα</rdfs:label><rdfs:label xml:lang="he">יוטה</rdfs:label><skos:exactMatch rdf:resource="http://vocab.getty.edu/aat/300014045"/><skos:scopeNote xml:lang="en">Bast fiber derived from either of two East Indian plants (Corchorus olitorius and C. capsularis). The pale brown fibers are soft, lustrous, and coarse, ranging in length from 4 to 10 feet. The brittle fibers are used to produce a thread called hessian. Jute becomes so weak when wet that a thin twine can be broken by hand. It turns brown and degrades with time, sunlight, water, acids, alkalis, and bleach. Jute has been used since prehistoric times. It is used to make sackcloth, burlap cloth, gunnysacks, twine, paper, and carpet backing. It was also used to make brown paper in Europe in the mid-19th century. (AAT)</skos:scopeNote></owl:Class><owl:Class rdf:about="http://thesaurus.europeanafashion.eu/thesaurus/10480"><rdfs:subClassOf rdf:resource="http://thesaurus.europeanafashion.eu/thesaurus/10353"/><rdfs:label xml:lang="de">Ramie</rdfs:label><rdfs:label xml:lang="nl">ramee</rdfs:label><rdfs:label xml:lang="pt">rami</rdfs:label><rdfs:label xml:lang="sv">rami</rdfs:label><rdfs:label xml:lang="en">ramie</rdfs:label><rdfs:label xml:lang="fr">ramie</rdfs:label><rdfs:label xml:lang="sr">ramija</rdfs:label><rdfs:label xml:lang="es">ramio</rdfs:label><rdfs:label xml:lang="it">ramié</rdfs:label><rdfs:label xml:lang="el">ραμί</rdfs:label><rdfs:label xml:lang="he">סיבים מצמח הרמי</rdfs:label><skos:exactMatch rdf:resource="http://vocab.getty.edu/aat/300014071"/><skos:scopeNote xml:lang="en">Bast fiber obtained from the stems of several varieties of the species Boehmeria nivea, native to tropical Asia but cultivated in China, Japan, Europe, South America, and the United States. The Ramie has been used in China for paper and fabric since prehistoric times. Its use spread through Europe in the Middle Ages. It is white or green in color, depending upon the variety. It is soft, fine, and durable fiber that is very lustrous and dyes well, used for twine, fishnets, sewing thread, and fabric for clothing, summer suits, dresses, canvas, tablecloths, and upholstery. Ramie has also been used to produce strong paper for linings, banknotes, and cigarettes. (AAT)</skos:scopeNote></owl:Class><owl:Class rdf:about="http://thesaurus.europeanafashion.eu/thesaurus/10481"><rdfs:subClassOf rdf:resource="http://thesaurus.europeanafashion.eu/thesaurus/10353"/><rdfs:label xml:lang="de">Kokosfaser</rdfs:label><rdfs:label xml:lang="de">Kokosnussfaser</rdfs:label><rdfs:label xml:lang="en">coconut fibre</rdfs:label><rdfs:label xml:lang="en">coir</rdfs:label><rdfs:label xml:lang="es">fibra de coco</rdfs:label><rdfs:label xml:lang="pt">fibra de côco</rdfs:label><rdfs:label xml:lang="it">fibra di cocco</rdfs:label><rdfs:label xml:lang="fr">fibre de coco</rdfs:label><rdfs:label xml:lang="sv">kokosnötsfiber</rdfs:label><rdfs:label xml:lang="sr">kokosovo vlakno</rdfs:label><rdfs:label xml:lang="nl">kokosvezel</rdfs:label><rdfs:label xml:lang="el">ίνες καρύδας</rdfs:label><rdfs:label xml:lang="he">סיבי קוקוס</rdfs:label><rdfs:label xml:lang="he">סיבים מדשא סיני</rdfs:label><skos:exactMatch rdf:resource="http://vocab.getty.edu/aat/300014056"/><skos:scopeNote xml:lang="en">Stiff, coarse, brown fibers derived from the outer bark of the fruit of the coconut palm, Cocos nucifera, used in making brushes, mats, cord, and coarse cloth. Coir is native to India and southeast Asia where it has been used since ancient times. It was introduced to Europe by Marco Polo in the 13th century. (AAT)</skos:scopeNote></owl:Class><owl:Class rdf:about="http://thesaurus.europeanafashion.eu/thesaurus/10482"><rdfs:subClassOf rdf:resource="http://thesaurus.europeanafashion.eu/thesaurus/10353"/><rdfs:label xml:lang="de">Ananasfaser</rdfs:label><rdfs:label xml:lang="sv">ananasfiber</rdfs:label><rdfs:label xml:lang="sr">ananasovo vlakno</rdfs:label><rdfs:label xml:lang="nl">ananasvezel</rdfs:label><rdfs:label xml:lang="pt">fibra de ananás</rdfs:label><rdfs:label xml:lang="es">fibra de piña</rdfs:label><rdfs:label xml:lang="it">fibra di ananas</rdfs:label><rdfs:label xml:lang="fr">fibre d'ananas</rdfs:label><rdfs:label xml:lang="en">pineapple fibre</rdfs:label><rdfs:label xml:lang="en">piña</rdfs:label><rdfs:label xml:lang="el">ίνες ανανά</rdfs:label><rdfs:label xml:lang="he">סיבי אננס</rdfs:label><skos:exactMatch rdf:resource="http://vocab.getty.edu/aat/300375581"/><skos:scopeNote xml:lang="en">Long bast fibers obtained from the leaves of the species Ananas comosus, native to tropical America. The fibers are fine, soft, lustrous, and light cream in color. They are resistant to salt water, strong, wear resistant, and easy to clean; used for fabric, rope, twine, and paper. (AAT)</skos:scopeNote></owl:Class><owl:Class rdf:about="http://thesaurus.europeanafashion.eu/thesaurus/10483"><rdfs:subClassOf rdf:resource="http://thesaurus.europeanafashion.eu/thesaurus/10353"/><rdfs:label xml:lang="de">Afrik</rdfs:label><rdfs:label xml:lang="de">Palmfaser</rdfs:label><rdfs:label xml:lang="es">fibra de palma</rdfs:label><rdfs:label xml:lang="pt">fibra de palmeira</rdfs:label><rdfs:label xml:lang="it">fibra di palma</rdfs:label><rdfs:label xml:lang="fr">fibre de palmier</rdfs:label><rdfs:label xml:lang="en">palm fibre</rdfs:label><rdfs:label xml:lang="sv">palmfiber</rdfs:label><rdfs:label xml:lang="sr">palmino vlakno</rdfs:label><rdfs:label xml:lang="nl">palmvezel</rdfs:label><rdfs:label xml:lang="el">ίνες φοίνικα</rdfs:label><rdfs:label xml:lang="he">סיבי תמר</rdfs:label><skos:exactMatch rdf:resource="http://vocab.getty.edu/aat/300014049"/><skos:scopeNote xml:lang="en">Fiber obtained from the palm plant. Among its numerous uses, such as the making of baskets, mats, and rope, it is used for securing mangrove poles in the framework of African houses. (AAT)</skos:scopeNote></owl:Class><owl:Class rdf:about="http://thesaurus.europeanafashion.eu/thesaurus/10522"><rdfs:subClassOf rdf:resource="http://thesaurus.europeanafashion.eu/thesaurus/10353"/><rdfs:label xml:lang="de">Agavenfaser</rdfs:label><rdfs:label xml:lang="en">agave fibre</rdfs:label><rdfs:label xml:lang="sv">agavefiber</rdfs:label><rdfs:label xml:lang="nl">agavevezel</rdfs:label><rdfs:label xml:lang="sr">agavino vlakno</rdfs:label><rdfs:label xml:lang="it">fibra d'agave</rdfs:label><rdfs:label xml:lang="es">pita</rdfs:label><rdfs:label xml:lang="fr">sisal</rdfs:label><rdfs:label xml:lang="el">ίνες αγαύης</rdfs:label><rdfs:label xml:lang="he">סיבי אגבה</rdfs:label><skos:exactMatch rdf:resource="http://vocab.getty.edu/aat/300375515"/><skos:scopeNote xml:lang="en">Species. The fiber has been used since pre-Columbian times; the Aztecs are known to have made clothing from it. From the late 1930s sisal has been cultivated commercially in Central and South America as well as in Africa. It is a strong, stiff fiber with a pale cream color. Sisal is typically dyed bright colors with direct or acid dyes. Sisal is used for cordage, ropes, sacks, brushes, upholstery padding, rugs, matting, handbags, hats, and in papermaking. (AAT)</skos:scopeNote></owl:Class><owl:Class rdf:about="http://thesaurus.europeanafashion.eu/thesaurus/10527"><rdfs:subClassOf rdf:resource="http://thesaurus.europeanafashion.eu/thesaurus/10353"/><rdfs:label xml:lang="de">Stroh</rdfs:label><rdfs:label xml:lang="sv">halm</rdfs:label><rdfs:label xml:lang="it">paglia</rdfs:label><rdfs:label xml:lang="fr">paille</rdfs:label><rdfs:label xml:lang="es">paja</rdfs:label><rdfs:label xml:lang="sr">slama</rdfs:label><rdfs:label xml:lang="en">straw</rdfs:label><rdfs:label xml:lang="nl">stro</rdfs:label><rdfs:label xml:lang="el">ψάθα</rdfs:label><rdfs:label xml:lang="he">קש</rdfs:label><skos:exactMatch rdf:resource="http://vocab.getty.edu/aat/300011908"/><skos:scopeNote xml:lang="en">Dried stalks of cereals or other grasses, used for many purposes, including weaving, plaiting, and braiding. (AAT)</skos:scopeNote></owl:Class><owl:Class rdf:about="http://thesaurus.europeanafashion.eu/thesaurus/10528"><rdfs:subClassOf rdf:resource="http://thesaurus.europeanafashion.eu/thesaurus/10353"/><rdfs:label xml:lang="de">Raffiabast</rdfs:label><rdfs:label xml:lang="de">Raphia</rdfs:label><rdfs:label xml:lang="de">Raphiabast</rdfs:label><rdfs:label xml:lang="sv">palm</rdfs:label><rdfs:label xml:lang="en">raffia</rdfs:label><rdfs:label xml:lang="nl">raffia</rdfs:label><rdfs:label xml:lang="es">rafia</rdfs:label><rdfs:label xml:lang="it">rafia</rdfs:label><rdfs:label xml:lang="sr">rafija</rdfs:label><rdfs:label xml:lang="fr">raphia</rdfs:label><rdfs:label xml:lang="el">ίνες φοίνικα raffia</rdfs:label><rdfs:label xml:lang="he">רפיה</rdfs:label><skos:exactMatch rdf:resource="http://vocab.getty.edu/aat/300014051"/><skos:scopeNote xml:lang="en">Strong fiber from leafstalks of palms of the genus Raphia, native to Africa and other places. Raffia fibers are used in their natural state by splitting apart thick sections and knotting the ends together. The fibers are a pale cream color and are often dyed to bright colors. Raffia is used to make skirts, woven into baskets, hats, bags, and mats. It is also used to make a fine grade of paper similar to Japanese papers. (AAT)</skos:scopeNote></owl:Class><owl:Class rdf:about="http://thesaurus.europeanafashion.eu/thesaurus/10529"><rdfs:subClassOf rdf:resource="http://thesaurus.europeanafashion.eu/thesaurus/10353"/><rdfs:label xml:lang="de">Reet</rdfs:label><rdfs:label xml:lang="de">Schilfgras</rdfs:label><rdfs:label xml:lang="de">Schilfrohr</rdfs:label><rdfs:label xml:lang="it">canna</rdfs:label><rdfs:label xml:lang="es">caña de junco</rdfs:label><rdfs:label xml:lang="en">reed</rdfs:label><rdfs:label xml:lang="nl">riet</rdfs:label><rdfs:label xml:lang="fr">roseau</rdfs:label><rdfs:label xml:lang="sr">trska</rdfs:label><rdfs:label xml:lang="sv">vass</rdfs:label><rdfs:label xml:lang="el">καλάμι</rdfs:label><rdfs:label xml:lang="he">קנה</rdfs:label><skos:exactMatch rdf:resource="http://vocab.getty.edu/aat/300011878"/><skos:scopeNote xml:lang="en">General term for material comprising the leaves and stems of various tall, stiff, wetland grasses of various genera in the order Poales. Used for construction and thatching roofs. (AAT)</skos:scopeNote></owl:Class><owl:Class rdf:about="http://thesaurus.europeanafashion.eu/thesaurus/10574"><rdfs:subClassOf rdf:resource="http://thesaurus.europeanafashion.eu/thesaurus/10353"/><rdfs:label xml:lang="de">Papier</rdfs:label><rdfs:label xml:lang="it">carta</rdfs:label><rdfs:label xml:lang="es">papel</rdfs:label><rdfs:label xml:lang="en">paper</rdfs:label><rdfs:label xml:lang="fr">papier</rdfs:label><rdfs:label xml:lang="nl">papier</rdfs:label><rdfs:label xml:lang="sr">papir</rdfs:label><rdfs:label xml:lang="sv">papper</rdfs:label><rdfs:label xml:lang="el">χαρτί</rdfs:label><rdfs:label xml:lang="he">נייר</rdfs:label><skos:exactMatch rdf:resource="http://vocab.getty.edu/aat/300014109"/><skos:scopeNote xml:lang="en">Refers generally to all types of thin matted or felted sheets or webs of fiber formed and dried on a fine screen from a pulpy water suspension. The fibers may be animal, such as hair, silk or wool, or mineral, such as asbestos, or synthetic. However most paper is made from cellulosic plant fiber, such as from wood pulp, grass, cotton, linen, and straw. (AAT)</skos:scopeNote></owl:Class><owl:Class rdf:about="http://thesaurus.europeanafashion.eu/thesaurus/10577"><rdfs:subClassOf rdf:resource="http://thesaurus.europeanafashion.eu/thesaurus/10353"/><rdfs:label xml:lang="de">Holz</rdfs:label><rdfs:label xml:lang="fr">bois</rdfs:label><rdfs:label xml:lang="sr">drvo</rdfs:label><rdfs:label xml:lang="nl">hout</rdfs:label><rdfs:label xml:lang="it">legno</rdfs:label><rdfs:label xml:lang="es">madera</rdfs:label><rdfs:label xml:lang="sv">trä</rdfs:label><rdfs:label xml:lang="en">wood</rdfs:label><rdfs:label xml:lang="el">ξύλο</rdfs:label><rdfs:label xml:lang="he">עץ</rdfs:label><skos:exactMatch rdf:resource="http://vocab.getty.edu/aat/300011914"/><skos:scopeNote xml:lang="en">The principal tissue of trees and other plants that provides both strength and a means of conducting nutrients. Wood is one of the most versatile materials known. (AAT)</skos:scopeNote></owl:Class><owl:Class rdf:about="http://thesaurus.europeanafashion.eu/thesaurus/10578"><rdfs:subClassOf rdf:resource="http://thesaurus.europeanafashion.eu/thesaurus/10353"/><rdfs:label xml:lang="de">Bambus</rdfs:label><rdfs:label xml:lang="nl">bamboe</rdfs:label><rdfs:label xml:lang="en">bamboo</rdfs:label><rdfs:label xml:lang="fr">bambou</rdfs:label><rdfs:label xml:lang="sv">bambu</rdfs:label><rdfs:label xml:lang="sr">bambus</rdfs:label><rdfs:label xml:lang="it">bambù</rdfs:label><rdfs:label xml:lang="es">bambú</rdfs:label><rdfs:label xml:lang="el">μπαμπού</rdfs:label><rdfs:label xml:lang="he">במבוק</rdfs:label><skos:exactMatch rdf:resource="http://vocab.getty.edu/aat/300011873"/><skos:scopeNote xml:lang="en">Material derived from the stem or stalk of the bamboo plant, which is any of 480 species of woody or treelike tropical and semitropical grass. (AAT)</skos:scopeNote></owl:Class><owl:Class rdf:about="http://thesaurus.europeanafashion.eu/thesaurus/10579"><rdfs:subClassOf rdf:resource="http://thesaurus.europeanafashion.eu/thesaurus/10353"/><rdfs:label xml:lang="de">Baumrinde</rdfs:label><rdfs:label xml:lang="de">Borke</rdfs:label><rdfs:label xml:lang="en">bark</rdfs:label><rdfs:label xml:lang="sv">bark</rdfs:label><rdfs:label xml:lang="it">corteccia</rdfs:label><rdfs:label xml:lang="es">corteza</rdfs:label><rdfs:label xml:lang="sr">kora</rdfs:label><rdfs:label xml:lang="nl">schors</rdfs:label><rdfs:label xml:lang="fr">écorce</rdfs:label><rdfs:label xml:lang="el">φλοιός</rdfs:label><rdfs:label xml:lang="he">קליפת עץ</rdfs:label><skos:exactMatch rdf:resource="http://vocab.getty.edu/aat/300011860"/><skos:scopeNote xml:lang="en">The external material that covers the woody parts of trees, as distinct and separate from the wood itself. (AAT)</skos:scopeNote></owl:Class><owl:Class rdf:about="http://thesaurus.europeanafashion.eu/thesaurus/10580"><rdfs:subClassOf rdf:resource="http://thesaurus.europeanafashion.eu/thesaurus/10353"/><rdfs:label xml:lang="de">Korken</rdfs:label><rdfs:label xml:lang="es">corcho</rdfs:label><rdfs:label xml:lang="en">cork</rdfs:label><rdfs:label xml:lang="pt">cortiça</rdfs:label><rdfs:label xml:lang="sv">kork</rdfs:label><rdfs:label xml:lang="nl">kurk</rdfs:label><rdfs:label xml:lang="fr">liège</rdfs:label><rdfs:label xml:lang="sr">pluta</rdfs:label><rdfs:label xml:lang="it">sughero</rdfs:label><rdfs:label xml:lang="el">φελός</rdfs:label><rdfs:label xml:lang="he">שעם</rdfs:label><skos:exactMatch rdf:resource="http://vocab.getty.edu/aat/300011862"/><skos:scopeNote xml:lang="en">The lightweight, elastic outer bark the cork oak, species Quercus suber native to the Mediterranean region. Cork is elastic, buoyant, and resilient, used to seal wine bottles, for insulation, floats, acoustical wall covering, flooring, shoe soles, gaskets, and handles. (AAT)</skos:scopeNote></owl:Class><owl:Class rdf:about="http://thesaurus.europeanafashion.eu/thesaurus/10816"><rdfs:subClassOf rdf:resource="http://thesaurus.europeanafashion.eu/thesaurus/10353"/><rdfs:label xml:lang="de">Kohle</rdfs:label><rdfs:label xml:lang="it">carbone</rdfs:label><rdfs:label xml:lang="fr">charbon</rdfs:label><rdfs:label xml:lang="en">charcoal</rdfs:label><rdfs:label xml:lang="nl">houtskool</rdfs:label><rdfs:label xml:lang="sv">träkol</rdfs:label><rdfs:label xml:lang="sr">ugalj</rdfs:label><rdfs:label xml:lang="el">κάρβουνο</rdfs:label><rdfs:label xml:lang="he">עץ בוק</rdfs:label><rdfs:label xml:lang="he">פחם</rdfs:label><skos:exactMatch rdf:resource="http://vocab.getty.edu/aat/300012862"/><skos:scopeNote xml:lang="en">A black, porous carbonaceous material comprising the carbon-containing residue from burned wood (e.g., willow, maple, beech, linden or plum) or other organic containing materials such as bone, plants or animals. It is used as a drawing material, for filtering liquids or air, and for other purposes. (AAT)</skos:scopeNote></owl:Class><owl:Class rdf:about="http://thesaurus.europeanafashion.eu/thesaurus/10927"><rdfs:subClassOf rdf:resource="http://thesaurus.europeanafashion.eu/thesaurus/10353"/><rdfs:label xml:lang="de">Bananenblatt</rdfs:label><rdfs:label xml:lang="en">banana leaf</rdfs:label><rdfs:label xml:lang="sv">bananblad</rdfs:label><rdfs:label xml:lang="nl">bananenblad</rdfs:label><rdfs:label xml:lang="fr">feuille de bananier</rdfs:label><rdfs:label xml:lang="it">foglia di banana</rdfs:label><rdfs:label xml:lang="sr">list banane</rdfs:label><rdfs:label xml:lang="el">φύλλο μπανανιάς</rdfs:label><rdfs:label xml:lang="he">עלה בננה</rdfs:label></owl:Class><owl:Class rdf:about="http://thesaurus.europeanafashion.eu/thesaurus/10928"><rdfs:subClassOf rdf:resource="http://thesaurus.europeanafashion.eu/thesaurus/10353"/><rdfs:label xml:lang="de">Bernstein</rdfs:label><rdfs:label xml:lang="en">amber</rdfs:label><rdfs:label xml:lang="nl">amber</rdfs:label><rdfs:label xml:lang="it">ambra</rdfs:label><rdfs:label xml:lang="fr">ambre</rdfs:label><rdfs:label xml:lang="sv">bärnsten</rdfs:label><rdfs:label xml:lang="sr">ćilibar</rdfs:label><rdfs:label xml:lang="el">κεχριμπάρι</rdfs:label><rdfs:label xml:lang="he">ענבר</rdfs:label><skos:exactMatch rdf:resource="http://vocab.getty.edu/aat/300012934"/><skos:scopeNote xml:lang="en">A yellowish, hard, glassy, translucent fossil tree resin found in largest deposits on the Baltic coast and dating 40-60 million years old. Types of amber are classified by location. Amber is composed of complex mixtures of oxidized and polymerized resin acids and resin alcohols. It has been gathered or mined since Paleolithic times. It is easy to carve and was often used in its natural state for jewelry, beads, amulets, and small vessels. It was also used as an ingredient in paint; dark color oil and amber varnishes are made by dissolving melted amber in amber oil, turpentine oil, or a drying oil. It develops an electrical charge when rubbed with a cloth. It is also valued because very ancient insects and plants may be preserved in the amber. (AAT)</skos:scopeNote></owl:Class><owl:Class rdf:about="http://thesaurus.europeanafashion.eu/thesaurus/11054"><rdfs:subClassOf rdf:resource="http://thesaurus.europeanafashion.eu/thesaurus/10353"/><rdfs:label xml:lang="de">Korb</rdfs:label><rdfs:label xml:lang="de">Weidenrute</rdfs:label><rdfs:label xml:lang="fr">osier</rdfs:label><rdfs:label xml:lang="sr">prut za pletenje</rdfs:label><rdfs:label xml:lang="sv">vide</rdfs:label><rdfs:label xml:lang="it">vimini</rdfs:label><rdfs:label xml:lang="nl">vlechtwerk</rdfs:label><rdfs:label xml:lang="en">wicker</rdfs:label><rdfs:label xml:lang="el">λυγαριά</rdfs:label><rdfs:label xml:lang="he">נצר</rdfs:label><skos:exactMatch rdf:resource="http://vocab.getty.edu/aat/300014690"/><skos:scopeNote xml:lang="en">Woven reed, rattan, twigs, or other material, especially used to construct furniture. (AAT)</skos:scopeNote></owl:Class><owl:Class rdf:about="http://thesaurus.europeanafashion.eu/thesaurus/11074"><rdfs:subClassOf rdf:resource="http://thesaurus.europeanafashion.eu/thesaurus/10353"/><rdfs:label xml:lang="de">Amarant</rdfs:label><rdfs:label xml:lang="sr">amarant</rdfs:label><rdfs:label xml:lang="sv">amarant</rdfs:label><rdfs:label xml:lang="fr">amarante</rdfs:label><rdfs:label xml:lang="en">amaranth</rdfs:label><rdfs:label xml:lang="nl">amaranthout</rdfs:label><rdfs:label xml:lang="it">amaranto</rdfs:label><rdfs:label xml:lang="sr">štir</rdfs:label><rdfs:label xml:lang="el">αμάραντος</rdfs:label><rdfs:label xml:lang="he">ירבוז</rdfs:label><skos:exactMatch rdf:resource="http://vocab.getty.edu/aat/300012419"/><skos:scopeNote xml:lang="en">Strong, elastic purplish wood derived from several species of the genus Peltogyne. The heartwood is brown when freshly cut becoming deep purple upon exposure to air, eventually turning to a dark brown with sharply demarcated off-white sapwood. Has a fine, uniform texture and grain that is straight or slightly roey. The durable, shock-resistant wood is sometimes used for carving and for vehicle construction. Also used widely in furniture-making, marquetry, veneers, flooring, etc. (AAT)</skos:scopeNote></owl:Class><owl:Class rdf:about="http://thesaurus.europeanafashion.eu/thesaurus/11075"><rdfs:subClassOf rdf:resource="http://thesaurus.europeanafashion.eu/thesaurus/10353"/><rdfs:label xml:lang="de">Samen</rdfs:label><rdfs:label xml:lang="sv">frö</rdfs:label><rdfs:label xml:lang="fr">graine</rdfs:label><rdfs:label xml:lang="en">seed</rdfs:label><rdfs:label xml:lang="it">seme</rdfs:label><rdfs:label xml:lang="sr">seme</rdfs:label><rdfs:label xml:lang="nl">zaad</rdfs:label><rdfs:label xml:lang="el">σπόρος</rdfs:label><rdfs:label xml:lang="he">אמרנט / אמרנטוס</rdfs:label><rdfs:label xml:lang="he">זרע</rdfs:label><skos:exactMatch rdf:resource="http://vocab.getty.edu/aat/300011902"/><skos:scopeNote xml:lang="en">Material comprising the seed of a plant, which is the nutrient material for development after germination that is enclosed in a protective coat. Seeds may be processed in various ways for use as materials, or they may be used whole as elements in a design. (AAT)</skos:scopeNote></owl:Class><owl:Class rdf:about="http://thesaurus.europeanafashion.eu/thesaurus/11076"><rdfs:subClassOf rdf:resource="http://thesaurus.europeanafashion.eu/thesaurus/10353"/><rdfs:label xml:lang="de">Brot</rdfs:label><rdfs:label xml:lang="en">bread</rdfs:label><rdfs:label xml:lang="nl">brood</rdfs:label><rdfs:label xml:lang="sv">bröd</rdfs:label><rdfs:label xml:lang="sr">hleb</rdfs:label><rdfs:label xml:lang="fr">pain</rdfs:label><rdfs:label xml:lang="it">pane</rdfs:label><rdfs:label xml:lang="el">ψωμί</rdfs:label><rdfs:label xml:lang="he">גרגיר</rdfs:label><rdfs:label xml:lang="he">לחם</rdfs:label><skos:exactMatch rdf:resource="http://vocab.getty.edu/aat/300262820"/><skos:scopeNote xml:lang="en">Use generally for cooked food made of dough composed of flour or meal of various plants, water, and other ingredients, with or without the addition of a leavening agent. Use specifically for loaves or cakes of dough made with flour and cooked by baking. (AAT)</skos:scopeNote></owl:Class><owl:Class rdf:about="http://thesaurus.europeanafashion.eu/thesaurus/11077"><rdfs:subClassOf rdf:resource="http://thesaurus.europeanafashion.eu/thesaurus/10353"/><rdfs:label xml:lang="de">Thujawurzel</rdfs:label><rdfs:label xml:lang="sr">koren tuje</rdfs:label><rdfs:label xml:lang="fr">racine de thuya</rdfs:label><rdfs:label xml:lang="it">radice di tuia</rdfs:label><rdfs:label xml:lang="en">thuja root</rdfs:label><rdfs:label xml:lang="nl">thujawortel</rdfs:label><rdfs:label xml:lang="sv">tuja</rdfs:label><rdfs:label xml:lang="el">ρίζα thuja</rdfs:label><rdfs:label xml:lang="he">שורש תויה</rdfs:label><skos:exactMatch rdf:resource="http://vocab.getty.edu/aat/300343675"/><skos:scopeNote xml:lang="en">Wood from trees of the Thuja genus. (AAT)</skos:scopeNote></owl:Class><owl:Class rdf:about="http://thesaurus.europeanafashion.eu/thesaurus/11078"><rdfs:subClassOf rdf:resource="http://thesaurus.europeanafashion.eu/thesaurus/10353"/><rdfs:label xml:lang="de">Harz</rdfs:label><rdfs:label xml:lang="nl">hars</rdfs:label><rdfs:label xml:lang="sv">harts</rdfs:label><rdfs:label xml:lang="sv">kåda</rdfs:label><rdfs:label xml:lang="en">resin</rdfs:label><rdfs:label xml:lang="it">resina</rdfs:label><rdfs:label xml:lang="fr">résine</rdfs:label><rdfs:label xml:lang="sr">smola</rdfs:label><rdfs:label xml:lang="el">ρητίνη</rdfs:label><rdfs:label xml:lang="he">שרף</rdfs:label><rdfs:label xml:lang="he">תויה</rdfs:label><skos:exactMatch rdf:resource="http://vocab.getty.edu/aat/300012882"/><skos:scopeNote xml:lang="en">General term for solid or semisolid organic substance usually obtained from plant secretions, but sometimes obtained from insects or synthetically produced. It is soluble in organic solvent but not in water, and is commonly used in varnish, printing ink, and size. It is distinguished from gum by not being dissoluble in water. To distinguish between natural and synthetic resins, use the narrower terms natural resin or synthetic resin. (AAT)</skos:scopeNote></owl:Class><owl:Class rdf:about="http://thesaurus.europeanafashion.eu/thesaurus/10922"><rdfs:subClassOf rdf:resource="http://thesaurus.europeanafashion.eu/thesaurus/10528"/><rdfs:label xml:lang="de">Raphiabastimitat</rdfs:label><rdfs:label xml:lang="sr">imitacija rafije</rdfs:label><rdfs:label xml:lang="nl">imitatieraffia</rdfs:label><rdfs:label xml:lang="en">imitation raffia</rdfs:label><rdfs:label xml:lang="it">imitazione della rafia</rdfs:label><rdfs:label xml:lang="sv">palmimitation</rdfs:label><rdfs:label xml:lang="fr">raphia artificiel</rdfs:label><rdfs:label xml:lang="el">απομίμηση raffia</rdfs:label><rdfs:label xml:lang="he">דמוי רפיה</rdfs:label></owl:Class><owl:Class rdf:about="http://thesaurus.europeanafashion.eu/thesaurus/10572"><rdfs:subClassOf rdf:resource="http://thesaurus.europeanafashion.eu/thesaurus/10574"/><rdfs:label xml:lang="de">Karton</rdfs:label><rdfs:label xml:lang="de">Pappe</rdfs:label><rdfs:label xml:lang="en">cardboard</rdfs:label><rdfs:label xml:lang="fr">carton</rdfs:label><rdfs:label xml:lang="it">cartone</rdfs:label><rdfs:label xml:lang="es">cartulina</rdfs:label><rdfs:label xml:lang="nl">karton</rdfs:label><rdfs:label xml:lang="sr">karton</rdfs:label><rdfs:label xml:lang="sv">kartong</rdfs:label><rdfs:label xml:lang="sv">papp</rdfs:label><rdfs:label xml:lang="el">χαρτόνι</rdfs:label><rdfs:label xml:lang="he">קרטון</rdfs:label><skos:exactMatch rdf:resource="http://vocab.getty.edu/aat/300014224"/><skos:scopeNote xml:lang="en">A type of stiff pasteboard that is thicker than 0.006 inches, typically consisting of good-quality chemical pulp or rag pasteboard, and varying greatly in type and stability. High quality archival cardboard is made from rag pulp and has a low acid content, used for mounting prints, drawings and watercolors. Other grades of cardboard is used for cards, signs, printed materials, and high-quality boxes. Inferior grades of cardboard, such as corrugated board, are made from coarsely ground sulfite treated wood pulp; for this board, use corrugated board. The first carboard box was produced in England in 1817. Corrugated cardboard was patented in 1871. (AAT)</skos:scopeNote></owl:Class><owl:Class rdf:about="http://thesaurus.europeanafashion.eu/thesaurus/10573"><rdfs:subClassOf rdf:resource="http://thesaurus.europeanafashion.eu/thesaurus/10574"/><rdfs:label xml:lang="de">Papier auf Karton</rdfs:label><rdfs:label xml:lang="it">carta su cartone</rdfs:label><rdfs:label xml:lang="sv">kartong</rdfs:label><rdfs:label xml:lang="es">papel sobre cartón</rdfs:label><rdfs:label xml:lang="el">paper on cardboard</rdfs:label><rdfs:label xml:lang="en">paper on cardboard</rdfs:label><rdfs:label xml:lang="fr">papier cartonné</rdfs:label><rdfs:label xml:lang="nl">papier op karton</rdfs:label><rdfs:label xml:lang="sr">papir na kartonu</rdfs:label><rdfs:label xml:lang="he">נייר על קרטון</rdfs:label></owl:Class><owl:Class rdf:about="http://thesaurus.europeanafashion.eu/thesaurus/10575"><rdfs:subClassOf rdf:resource="http://thesaurus.europeanafashion.eu/thesaurus/10574"/><rdfs:label xml:lang="de">Papiermaché</rdfs:label><rdfs:label xml:lang="de">Papiermaschee</rdfs:label><rdfs:label xml:lang="it">cartapesta</rdfs:label><rdfs:label xml:lang="es">papel maché</rdfs:label><rdfs:label xml:lang="fr">papier mâché</rdfs:label><rdfs:label xml:lang="nl">papier-maché</rdfs:label><rdfs:label xml:lang="sv">papier-maché</rdfs:label><rdfs:label xml:lang="en">papier-mâché</rdfs:label><rdfs:label xml:lang="sr">papir maše</rdfs:label><rdfs:label xml:lang="el">πεπιεσμένο χαρτί</rdfs:label><rdfs:label xml:lang="he">עיסת נייר</rdfs:label><skos:exactMatch rdf:resource="http://vocab.getty.edu/aat/300014245"/><skos:scopeNote xml:lang="en">Composite material used for molding objects; made of repulped or pulverized paper and a liquid adhesive binder. May also comprise strips of paper, sometimes reinforced with textiles, stuck together with a wet adhesive, and used to form an object. The object becomes solid when the paste dries; the object may then be sanded, lacquered, and painted. Such objects are very durable; they first developed in Asia and were common in Europe and elsewhere since the 17th century. (AAT)</skos:scopeNote></owl:Class><owl:Class rdf:about="http://thesaurus.europeanafashion.eu/thesaurus/10576"><rdfs:subClassOf rdf:resource="http://thesaurus.europeanafashion.eu/thesaurus/10574"/><rdfs:label xml:lang="de">Seidenpapier</rdfs:label><rdfs:label xml:lang="it">carta velina</rdfs:label><rdfs:label xml:lang="es">papel de seda</rdfs:label><rdfs:label xml:lang="fr">papier de soie</rdfs:label><rdfs:label xml:lang="fr">papier mousseline</rdfs:label><rdfs:label xml:lang="sv">silkepapper</rdfs:label><rdfs:label xml:lang="en">tissue paper</rdfs:label><rdfs:label xml:lang="sr">toaletni papir</rdfs:label><rdfs:label xml:lang="nl">zijdepapier</rdfs:label><rdfs:label xml:lang="el">χαρτομάντιλο</rdfs:label><rdfs:label xml:lang="he">ניר משי</rdfs:label><skos:exactMatch rdf:resource="http://vocab.getty.edu/aat/300014145"/><skos:scopeNote xml:lang="en">A thin, translucent paper that may be loosely felted to make it absorbent or it may have a hard, smooth surface making it an excellent wrapping paper. It is primarily used for packing, wrapping, or protecting delicate items. (AAT)</skos:scopeNote></owl:Class><owl:Class rdf:about="http://thesaurus.europeanafashion.eu/thesaurus/10801"><rdfs:subClassOf rdf:resource="http://thesaurus.europeanafashion.eu/thesaurus/10577"/><rdfs:label xml:lang="de">Ulme</rdfs:label><rdfs:label xml:lang="sv">alm</rdfs:label><rdfs:label xml:lang="sr">brest</rdfs:label><rdfs:label xml:lang="en">elm</rdfs:label><rdfs:label xml:lang="nl">olm</rdfs:label><rdfs:label xml:lang="it">olmo</rdfs:label><rdfs:label xml:lang="fr">orme</rdfs:label><rdfs:label xml:lang="el">φτελιά</rdfs:label><rdfs:label xml:lang="he">אולמוס</rdfs:label><skos:exactMatch rdf:resource="http://vocab.getty.edu/aat/300012070"/><skos:scopeNote xml:lang="en">Tough, durable, brown-color wood of the genus Ulmus that is used for ax handles, yokes, wheels, weapons, coffins, ships' structure, and gymnasium equipment. (AAT)</skos:scopeNote></owl:Class><owl:Class rdf:about="http://thesaurus.europeanafashion.eu/thesaurus/10802"><rdfs:subClassOf rdf:resource="http://thesaurus.europeanafashion.eu/thesaurus/10577"/><rdfs:label xml:lang="de">Ebenholz</rdfs:label><rdfs:label xml:lang="sr">abonos</rdfs:label><rdfs:label xml:lang="it">ebano</rdfs:label><rdfs:label xml:lang="nl">ebben</rdfs:label><rdfs:label xml:lang="sv">ebenholts</rdfs:label><rdfs:label xml:lang="en">ebony</rdfs:label><rdfs:label xml:lang="fr">ébène</rdfs:label><rdfs:label xml:lang="el">έβενος</rdfs:label><rdfs:label xml:lang="he">בוקיצה</rdfs:label><rdfs:label xml:lang="he">הובנה</rdfs:label><skos:exactMatch rdf:resource="http://vocab.getty.edu/aat/300012055"/><skos:scopeNote xml:lang="en">A hard, heavy, durable heartwood wood yielded by various trees of the genus Diospyros in tropical Asia and Africa, valued for its dense, smooth-grain from the earliest times; was imported to Egypt from Nubia and the Sudan. It is extremely durable, resistant to rotting, fungi and powder post beetles, but difficult to work and carve. It has been used for decorative items, inlay work, black piano keys, musical instruments, and tool handles. Several other dark, heavy woods from unrelated species are also called ebony because of their color, including cocuswood, coffeewood, blue ebony, and African blackwood. (AAT)</skos:scopeNote></owl:Class><owl:Class rdf:about="http://thesaurus.europeanafashion.eu/thesaurus/10803"><rdfs:subClassOf rdf:resource="http://thesaurus.europeanafashion.eu/thesaurus/10577"/><rdfs:label xml:lang="de">Birke</rdfs:label><rdfs:label xml:lang="nl">berk</rdfs:label><rdfs:label xml:lang="it">betulla</rdfs:label><rdfs:label xml:lang="en">birch</rdfs:label><rdfs:label xml:lang="sv">björk</rdfs:label><rdfs:label xml:lang="fr">bouleau</rdfs:label><rdfs:label xml:lang="sr">breza</rdfs:label><rdfs:label xml:lang="el">σημύδα</rdfs:label><rdfs:label xml:lang="he">ליבנה</rdfs:label><rdfs:label xml:lang="he">עץ שחור/ אבוני</rdfs:label><skos:exactMatch rdf:resource="http://vocab.getty.edu/aat/300011973"/><skos:scopeNote xml:lang="en">Strong, pale yellow-brown wood from trees of the genus Betula, having a close, straight grain and uniform texture that finishes to a smooth surface. It is sometimes dyed to imitate mahogany. Birch is used for tools handles, plywood, hoops, shoe heels, flooring, furniture, cabinetry, turnery, and firewood. The bark is also used for various purposes. (AAT)</skos:scopeNote></owl:Class><owl:Class rdf:about="http://thesaurus.europeanafashion.eu/thesaurus/10804"><rdfs:subClassOf rdf:resource="http://thesaurus.europeanafashion.eu/thesaurus/10577"/><rdfs:label xml:lang="de">Buche</rdfs:label><rdfs:label xml:lang="en">beech</rdfs:label><rdfs:label xml:lang="nl">beuk</rdfs:label><rdfs:label xml:lang="sv">bok</rdfs:label><rdfs:label xml:lang="sr">bukva</rdfs:label><rdfs:label xml:lang="it">faggio</rdfs:label><rdfs:label xml:lang="fr">hêtre</rdfs:label><rdfs:label xml:lang="el">οξιά</rdfs:label><rdfs:label xml:lang="he">אשור</rdfs:label><skos:exactMatch rdf:resource="http://vocab.getty.edu/aat/300011948"/><skos:scopeNote xml:lang="en">Pale reddish-brown, close-grain wood from any of several trees of the genus Fagus; it is hard and heavy, bends well, is durable under water, and gives a smooth shiny finish. Beech wood is commonly used for flooring, cabinetry, furniture (especially bentwood chairs), veneer, plywood, tool handles, and turnery. It was used in panel paintings in western Europe. (AAT)</skos:scopeNote></owl:Class><owl:Class rdf:about="http://thesaurus.europeanafashion.eu/thesaurus/11065"><rdfs:subClassOf rdf:resource="http://thesaurus.europeanafashion.eu/thesaurus/10577"/><rdfs:label xml:lang="de">Mahagoniholz</rdfs:label><rdfs:label xml:lang="fr">acajou</rdfs:label><rdfs:label xml:lang="sr">mahagoni</rdfs:label><rdfs:label xml:lang="en">mahogany</rdfs:label><rdfs:label xml:lang="sv">mahogny</rdfs:label><rdfs:label xml:lang="nl">mahonie</rdfs:label><rdfs:label xml:lang="it">mogano</rdfs:label><rdfs:label xml:lang="el">μαόνι</rdfs:label><rdfs:label xml:lang="he">מהגוני</rdfs:label><rdfs:label xml:lang="he">פחם עץ</rdfs:label><skos:exactMatch rdf:resource="http://vocab.getty.edu/aat/300012221"/><skos:scopeNote xml:lang="en">Refers to the wood of trees of the genus Swietenia, found in tropical climates, primarily in Mexico, Cuba, Central America, and the West Indies. It varies in color from yellow to a rich red brown, and is valued in furniture-making and sculpture-carving because it is hard, fine-grained, and takes a high polish. Mahogany has a fine, straight grain that takes a high polish. It is dimensionally stable and does not shrink, warp, or swell. The durable, dark reddish-brown wood was imported to Europe in the 18th century where it became popular for furniture, paneling and veneer. Ammonia brings out a rich, red color in mahogany wood. Mahogany is frequently attacked by pinhole borer beetles. Many woods of similar colors have also been called mahoganies, but usually do not have rich color or fine cutting characteristics of the true mahogany wood. However, the related African genus Khaya produces a similar wood. Mahogany was used by Chippendale, Hepplewhite, and the Adam brothers for high quality furniture. (AAT)</skos:scopeNote></owl:Class><owl:Class rdf:about="http://thesaurus.europeanafashion.eu/thesaurus/11066"><rdfs:subClassOf rdf:resource="http://thesaurus.europeanafashion.eu/thesaurus/10577"/><rdfs:label xml:lang="de">Buchsbaum</rdfs:label><rdfs:label xml:lang="it">albero di bosso</rdfs:label><rdfs:label xml:lang="en">boxwood (wood)</rdfs:label><rdfs:label xml:lang="fr">buis</rdfs:label><rdfs:label xml:lang="sv">buxbom</rdfs:label><rdfs:label xml:lang="en">buxus</rdfs:label><rdfs:label xml:lang="nl">buxus</rdfs:label><rdfs:label xml:lang="sr">šimšir</rdfs:label><rdfs:label xml:lang="el">πυξάρι</rdfs:label><rdfs:label xml:lang="he">עץ תאשור</rdfs:label><rdfs:label xml:lang="he">תולענה</rdfs:label><skos:exactMatch rdf:resource="http://vocab.getty.edu/aat/300012002"/><skos:scopeNote xml:lang="en">Dense, pale yellow wood from trees of the genus Buxus. Although difficult to carve, the wood has excellent dimensional stability and is very wear resistant. The hard, fine-grain wood is often used for printing blocks, rulers, mallets, architects scales, slide rules, modeling tools, musical instruments, engravings, inlays, small decorative items, and game pieces. (AAT)</skos:scopeNote></owl:Class><owl:Class rdf:about="http://thesaurus.europeanafashion.eu/thesaurus/11067"><rdfs:subClassOf rdf:resource="http://thesaurus.europeanafashion.eu/thesaurus/10577"/><rdfs:label xml:lang="de">Kiefer</rdfs:label><rdfs:label xml:lang="sr">bor</rdfs:label><rdfs:label xml:lang="nl">grenenhout</rdfs:label><rdfs:label xml:lang="fr">pin</rdfs:label><rdfs:label xml:lang="en">pine</rdfs:label><rdfs:label xml:lang="it">pino</rdfs:label><rdfs:label xml:lang="sv">tall</rdfs:label><rdfs:label xml:lang="el">πεύκο</rdfs:label><rdfs:label xml:lang="he">אורן</rdfs:label><skos:exactMatch rdf:resource="http://vocab.getty.edu/aat/300012620"/><skos:scopeNote xml:lang="en">Wood from numerous trees of the genus Pinus. Pine is used largely in the construction and paper industries, although it is also a source of turpentine, resins, and oils, among other products. (AAT)</skos:scopeNote></owl:Class><owl:Class rdf:about="http://thesaurus.europeanafashion.eu/thesaurus/11068"><rdfs:subClassOf rdf:resource="http://thesaurus.europeanafashion.eu/thesaurus/10577"/><rdfs:label xml:lang="de">Ahorn</rdfs:label><rdfs:label xml:lang="it">acero</rdfs:label><rdfs:label xml:lang="nl">esdoornhout</rdfs:label><rdfs:label xml:lang="sr">javor</rdfs:label><rdfs:label xml:lang="sv">lönn</rdfs:label><rdfs:label xml:lang="en">maple</rdfs:label><rdfs:label xml:lang="fr">érable</rdfs:label><rdfs:label xml:lang="el">σφεντάμι</rdfs:label><rdfs:label xml:lang="he">אדר</rdfs:label><skos:exactMatch rdf:resource="http://vocab.getty.edu/aat/300012236"/><skos:scopeNote xml:lang="en">Wood of trees belonging to the genus Acer, light reddish brown in color, with small pores, distinct rings, and rays that show as fine dashes in quarter sawed wood. Maple wood is used for fine furniture, cabinetry, flooring, shoe lasts, and musical instruments. (AAT)</skos:scopeNote></owl:Class><owl:Class rdf:about="http://thesaurus.europeanafashion.eu/thesaurus/11069"><rdfs:subClassOf rdf:resource="http://thesaurus.europeanafashion.eu/thesaurus/10577"/><rdfs:label xml:lang="de">Nussbaum</rdfs:label><rdfs:label xml:lang="it">noce</rdfs:label><rdfs:label xml:lang="nl">notenhout (hardhout)</rdfs:label><rdfs:label xml:lang="fr">noyer</rdfs:label><rdfs:label xml:lang="sr">orahovo drvo</rdfs:label><rdfs:label xml:lang="sv">valnöt</rdfs:label><rdfs:label xml:lang="en">walnut tree</rdfs:label><rdfs:label xml:lang="el">καρυδιά</rdfs:label><rdfs:label xml:lang="he">אגוז מלך</rdfs:label><rdfs:label xml:lang="he">עץ המייפל</rdfs:label><skos:exactMatch rdf:resource="http://vocab.getty.edu/aat/300012476"/><skos:scopeNote xml:lang="en">Wood of several trees belonging to the genus Juglans, ranging in color from grey-brown to purple brown, used in making cabinetwork, veneer, butts and rifle stocks. (AAT)</skos:scopeNote></owl:Class><owl:Class rdf:about="http://thesaurus.europeanafashion.eu/thesaurus/11070"><rdfs:subClassOf rdf:resource="http://thesaurus.europeanafashion.eu/thesaurus/10577"/><rdfs:label xml:lang="de">Padouk (Rotholz)</rdfs:label><rdfs:label xml:lang="nl">padoekhout</rdfs:label><rdfs:label xml:lang="fr">padouk</rdfs:label><rdfs:label xml:lang="sv">padouk</rdfs:label><rdfs:label xml:lang="it">padouk (legno corallo)</rdfs:label><rdfs:label xml:lang="en">padouk tree</rdfs:label><rdfs:label xml:lang="sr">paduk drvo</rdfs:label><rdfs:label xml:lang="el">δέντρο padouk</rdfs:label><rdfs:label xml:lang="he">עץ פדאוק</rdfs:label><skos:exactMatch rdf:resource="http://vocab.getty.edu/aat/300012335"/><skos:scopeNote xml:lang="en">Wood of the genus Pterocarpus, native to Africa and Asia. It is typically used for cabinetwork, shipbuilding, flooring, and joinery. The hard and heavy wood is noted for its ability to take a high polish. Varieties used for cabinetwork are usually red or rose color, often variegated with yellow. (AAT)</skos:scopeNote></owl:Class><owl:Class rdf:about="http://thesaurus.europeanafashion.eu/thesaurus/11071"><rdfs:subClassOf rdf:resource="http://thesaurus.europeanafashion.eu/thesaurus/10577"/><rdfs:label xml:lang="de">Palme</rdfs:label><rdfs:label xml:lang="nl">palm</rdfs:label><rdfs:label xml:lang="sv">palm</rdfs:label><rdfs:label xml:lang="en">palm tree</rdfs:label><rdfs:label xml:lang="it">palma</rdfs:label><rdfs:label xml:lang="fr">palmier</rdfs:label><rdfs:label xml:lang="sr">palmino drvo</rdfs:label><rdfs:label xml:lang="el">φοίνικας</rdfs:label><rdfs:label xml:lang="he">דקל</rdfs:label><skos:exactMatch rdf:resource="http://vocab.getty.edu/aat/300014049"/><skos:scopeNote xml:lang="en">Fiber obtained from the palm plant. Among its numerous uses, such as the making of baskets, mats, and rope, it is used for securing mangrove poles in the framework of African houses. (AAT)</skos:scopeNote></owl:Class><owl:Class rdf:about="http://thesaurus.europeanafashion.eu/thesaurus/11072"><rdfs:subClassOf rdf:resource="http://thesaurus.europeanafashion.eu/thesaurus/11071"/><rdfs:label xml:lang="de">Corozonuss</rdfs:label><rdfs:label xml:lang="en">corozo</rdfs:label><rdfs:label xml:lang="fr">corozo</rdfs:label><rdfs:label xml:lang="it">corozo</rdfs:label><rdfs:label xml:lang="nl">corozo</rdfs:label><rdfs:label xml:lang="sv">corozo</rdfs:label><rdfs:label xml:lang="sr">korozo</rdfs:label><rdfs:label xml:lang="el">φυτελέφας</rdfs:label><rdfs:label xml:lang="he">אגוז קורוזו</rdfs:label><skos:exactMatch rdf:resource="http://vocab.getty.edu/aat/300379935"/><skos:scopeNote xml:lang="en">The hard nut or seed of several types of palm tree which resembles ivory in hardness and appearance and serves as a substitute. Vegetable ivory is used for small, carved, ornamental items such as buttons and figurines. (AAT)</skos:scopeNote></owl:Class><owl:Class rdf:about="http://thesaurus.europeanafashion.eu/thesaurus/11079"><rdfs:subClassOf rdf:resource="http://thesaurus.europeanafashion.eu/thesaurus/11078"/><rdfs:label xml:lang="de">Bernstein</rdfs:label><rdfs:label xml:lang="nl">amber</rdfs:label><rdfs:label xml:lang="en">amber (fossil resin)</rdfs:label><rdfs:label xml:lang="it">ambra</rdfs:label><rdfs:label xml:lang="fr">ambre</rdfs:label><rdfs:label xml:lang="sv">bärnsten</rdfs:label><rdfs:label xml:lang="sr">ćilibar</rdfs:label><rdfs:label xml:lang="el">κεχριμπάρι</rdfs:label><rdfs:label xml:lang="he">ענבר</rdfs:label><skos:exactMatch rdf:resource="http://vocab.getty.edu/aat/300012934"/><skos:scopeNote xml:lang="en">A yellowish, hard, glassy, translucent fossil tree resin found in largest deposits on the Baltic coast and dating 40-60 million years old. Types of amber are classified by location. Amber is composed of complex mixtures of oxidized and polymerized resin acids and resin alcohols. It has been gathered or mined since Paleolithic times. It is easy to carve and was often used in its natural state for jewelry, beads, amulets, and small vessels. It was also used as an ingredient in paint; dark color oil and amber varnishes are made by dissolving melted amber in amber oil, turpentine oil, or a drying oil. It develops an electrical charge when rubbed with a cloth. It is also valued because very ancient insects and plants may be preserved in the amber. (AAT)</skos:scopeNote></owl:Class><owl:Class rdf:about="http://thesaurus.europeanafashion.eu/thesaurus/10050"><rdfs:subClassOf rdf:resource="http://thesaurus.europeanafashion.eu/thesaurus/10543"/><rdfs:label xml:lang="de">Münzen</rdfs:label><rdfs:label xml:lang="en">coins</rdfs:label><rdfs:label xml:lang="it">monete</rdfs:label><rdfs:label xml:lang="nl">munten</rdfs:label><rdfs:label xml:lang="sr">novčići</rdfs:label><rdfs:label xml:lang="fr">pièce</rdfs:label><rdfs:label xml:lang="el">νομίσματα</rdfs:label><skos:exactMatch rdf:resource="http://vocab.getty.edu/aat/300037222"/><skos:scopeNote xml:lang="en">Pieces of metal stamped by government authority for use as money. (AAT)</skos:scopeNote></owl:Class><owl:Class rdf:about="http://thesaurus.europeanafashion.eu/thesaurus/10429"><rdfs:subClassOf rdf:resource="http://thesaurus.europeanafashion.eu/thesaurus/10543"/><rdfs:label xml:lang="de">Pailletten</rdfs:label><rdfs:label xml:lang="pt">lantejoulas</rdfs:label><rdfs:label xml:lang="es">lentejuelas</rdfs:label><rdfs:label xml:lang="nl">pailletten</rdfs:label><rdfs:label xml:lang="fr">paillettes</rdfs:label><rdfs:label xml:lang="it">paillettes, lustrini</rdfs:label><rdfs:label xml:lang="sv">paljetter</rdfs:label><rdfs:label xml:lang="en">sequins</rdfs:label><rdfs:label xml:lang="sr">šljokice</rdfs:label><rdfs:label xml:lang="el">πούλιες</rdfs:label><rdfs:label xml:lang="he">נצנצים</rdfs:label><skos:exactMatch rdf:resource="http://vocab.getty.edu/aat/300183896"/><skos:scopeNote xml:lang="en">Adornment consisting of a small piece of shiny material used to decorate clothing (Wordnet)</skos:scopeNote></owl:Class><owl:Class rdf:about="http://thesaurus.europeanafashion.eu/thesaurus/10510"><rdfs:subClassOf rdf:resource="http://thesaurus.europeanafashion.eu/thesaurus/10543"/><rdfs:label xml:lang="de">Band</rdfs:label><rdfs:label xml:lang="sv">band</rdfs:label><rdfs:label xml:lang="es">caídas de talle</rdfs:label><rdfs:label xml:lang="es">fachas</rdfs:label><rdfs:label xml:lang="es">lazo</rdfs:label><rdfs:label xml:lang="nl">lint</rdfs:label><rdfs:label xml:lang="it">nastro</rdfs:label><rdfs:label xml:lang="en">ribbon</rdfs:label><rdfs:label xml:lang="fr">ruban</rdfs:label><rdfs:label xml:lang="sr">traka</rdfs:label><rdfs:label xml:lang="el">κορδέλα</rdfs:label><rdfs:label xml:lang="he">סרט</rdfs:label><rdfs:label xml:lang="he">פרגמנט תחרה</rdfs:label><skos:exactMatch rdf:resource="http://vocab.getty.edu/aat/300014668"/><skos:scopeNote xml:lang="en">Strips of fine textile, such as silk, satin, or velvet, often with a cord finish along both edges instead of selvage, forming a narrow strip or band, used for decorative trimming of a garment or for fastening or attaching something. May also refer to anything that resembles such objects, that is, any long, thin, flat, flexible strips of any material. (AAT)</skos:scopeNote></owl:Class><owl:Class rdf:about="http://thesaurus.europeanafashion.eu/thesaurus/10568"><rdfs:subClassOf rdf:resource="http://thesaurus.europeanafashion.eu/thesaurus/10543"/><rdfs:label xml:lang="de">Strass</rdfs:label><rdfs:label xml:lang="it">diamante artificiale</rdfs:label><rdfs:label xml:lang="es">estrás</rdfs:label><rdfs:label xml:lang="en">paste</rdfs:label><rdfs:label xml:lang="en">rhinestone</rdfs:label><rdfs:label xml:lang="nl">rijnsteen</rdfs:label><rdfs:label xml:lang="nl">stras</rdfs:label><rdfs:label xml:lang="en">strass</rdfs:label><rdfs:label xml:lang="fr">strass</rdfs:label><rdfs:label xml:lang="sv">strass</rdfs:label><rdfs:label xml:lang="sr">štras</rdfs:label><rdfs:label xml:lang="el">στρας</rdfs:label><rdfs:label xml:lang="he">יהלומים מלאכותיים (ריינסטון)</rdfs:label><skos:exactMatch rdf:resource="http://vocab.getty.edu/aat/300010806"/><skos:scopeNote xml:lang="en">A colorless artificial gem of paste or glass, often with facets that sparkle in imitation of a diamond. Also refers to foil-backed or silvered cut glass used to imitate diamonds. Rhinestones were originally quartz pebbles found in the Rhine River, thus the name. (AAT)</skos:scopeNote></owl:Class><owl:Class rdf:about="http://thesaurus.europeanafashion.eu/thesaurus/10595"><rdfs:subClassOf rdf:resource="http://thesaurus.europeanafashion.eu/thesaurus/10543"/><rdfs:label xml:lang="de">Perle</rdfs:label><rdfs:label xml:lang="sr">biseri</rdfs:label><rdfs:label xml:lang="nl">parel</rdfs:label><rdfs:label xml:lang="en">pearl</rdfs:label><rdfs:label xml:lang="es">perla</rdfs:label><rdfs:label xml:lang="it">perla</rdfs:label><rdfs:label xml:lang="fr">perle</rdfs:label><rdfs:label xml:lang="sv">pärla</rdfs:label><rdfs:label xml:lang="el">πέρλα</rdfs:label><rdfs:label xml:lang="he">פנינה</rdfs:label><skos:exactMatch rdf:resource="http://vocab.getty.edu/aat/300011827"/><skos:scopeNote xml:lang="en">A smooth round bead formed primarily within the shells of two distantly related groups of molluscan bivalves or clams, including the ocean-dwelling pearl oysters and the freshwater river mussels. Pearls are used in jewelry and for other ornamental puposes; they are considered a gem. (AAT)</skos:scopeNote></owl:Class><owl:Class rdf:about="http://thesaurus.europeanafashion.eu/thesaurus/10723"><rdfs:subClassOf rdf:resource="http://thesaurus.europeanafashion.eu/thesaurus/10543"/><rdfs:label xml:lang="de">Pelzbesatz</rdfs:label><rdfs:label xml:lang="nl">bonten afwerking</rdfs:label><rdfs:label xml:lang="it">bordo in pelliccia</rdfs:label><rdfs:label xml:lang="en">fur trimming</rdfs:label><rdfs:label xml:lang="fr">garniture de fourrure</rdfs:label><rdfs:label xml:lang="sr">krzneni rub</rdfs:label><rdfs:label xml:lang="sv">pälsbräm</rdfs:label><rdfs:label xml:lang="es">ribetes de piel</rdfs:label><rdfs:label xml:lang="el">γούνινη διακόσμηση</rdfs:label><rdfs:label xml:lang="he">קישוט פרווה</rdfs:label></owl:Class><owl:Class rdf:about="http://thesaurus.europeanafashion.eu/thesaurus/10725"><rdfs:subClassOf rdf:resource="http://thesaurus.europeanafashion.eu/thesaurus/10543"/><rdfs:label xml:lang="de">Quaste</rdfs:label><rdfs:label xml:lang="de">Troddel</rdfs:label><rdfs:label xml:lang="es">borla</rdfs:label><rdfs:label xml:lang="fr">gland</rdfs:label><rdfs:label xml:lang="sr">kićanka</rdfs:label><rdfs:label xml:lang="nl">kwast</rdfs:label><rdfs:label xml:lang="it">nappa</rdfs:label><rdfs:label xml:lang="en">tassel</rdfs:label><rdfs:label xml:lang="sv">tofs</rdfs:label><rdfs:label xml:lang="el">φούντα</rdfs:label><rdfs:label xml:lang="he">גדיל</rdfs:label><skos:exactMatch rdf:resource="http://vocab.getty.edu/aat/300232185"/><skos:scopeNote xml:lang="en">Pendant trimming. Before the 20th century, usually a wooden mold covered with strands of silk or worsted; now often merely a bunch of threads, cords, or other strands gathered together at the top. (AAT)</skos:scopeNote></owl:Class><owl:Class rdf:about="http://thesaurus.europeanafashion.eu/thesaurus/10765"><rdfs:subClassOf rdf:resource="http://thesaurus.europeanafashion.eu/thesaurus/10543"/><rdfs:label xml:lang="de">Bead</rdfs:label><rdfs:label xml:lang="en">bead</rdfs:label><rdfs:label xml:lang="es">cuenta</rdfs:label><rdfs:label xml:lang="nl">kraal</rdfs:label><rdfs:label xml:lang="de">künstliche Perle</rdfs:label><rdfs:label xml:lang="it">perla</rdfs:label><rdfs:label xml:lang="sr">perla</rdfs:label><rdfs:label xml:lang="fr">perle</rdfs:label><rdfs:label xml:lang="sv">pärla</rdfs:label><rdfs:label xml:lang="el">χάντρα</rdfs:label><rdfs:label xml:lang="he">חרוז</rdfs:label><skos:exactMatch rdf:resource="http://vocab.getty.edu/aat/300234006"/><skos:scopeNote xml:lang="en">Refers to small objects, of any shape or material, pierced so that they may be strung or hung or attached, as by sewing. (AAT)</skos:scopeNote></owl:Class><owl:Class rdf:about="http://thesaurus.europeanafashion.eu/thesaurus/10797"><rdfs:subClassOf rdf:resource="http://thesaurus.europeanafashion.eu/thesaurus/10543"/><rdfs:label xml:lang="de">Garn</rdfs:label><rdfs:label xml:lang="fr">fil</rdfs:label><rdfs:label xml:lang="it">filo</rdfs:label><rdfs:label xml:lang="nl">garen</rdfs:label><rdfs:label xml:lang="sv">garn</rdfs:label><rdfs:label xml:lang="es">hilo</rdfs:label><rdfs:label xml:lang="sr">konac</rdfs:label><rdfs:label xml:lang="sr">pređa</rdfs:label><rdfs:label xml:lang="en">yarn</rdfs:label><rdfs:label xml:lang="el">νήμα</rdfs:label><rdfs:label xml:lang="he">חוט</rdfs:label></owl:Class><owl:Class rdf:about="http://thesaurus.europeanafashion.eu/thesaurus/10888"><rdfs:subClassOf rdf:resource="http://thesaurus.europeanafashion.eu/thesaurus/10543"/><rdfs:label xml:lang="de">Borte</rdfs:label><rdfs:label xml:lang="sr">gajtan</rdfs:label><rdfs:label xml:lang="it">gallone</rdfs:label><rdfs:label xml:lang="en">galloon</rdfs:label><rdfs:label xml:lang="fr">galon</rdfs:label><rdfs:label xml:lang="nl">galon</rdfs:label><rdfs:label xml:lang="sv">galoner</rdfs:label><rdfs:label xml:lang="el">διακοσμητική φάσα</rdfs:label><rdfs:label xml:lang="he">בד מתנפנף</rdfs:label><rdfs:label xml:lang="he">רצועת תחרה</rdfs:label><skos:exactMatch rdf:resource="http://vocab.getty.edu/aat/300231784"/><skos:scopeNote xml:lang="en">Narrow ornamented band, tape, lace or braid, often with metal thread, and often with both edges scalloped, used as trimming or binding on costume and textile furnishings. (AAT)</skos:scopeNote></owl:Class><owl:Class rdf:about="http://thesaurus.europeanafashion.eu/thesaurus/10889"><rdfs:subClassOf rdf:resource="http://thesaurus.europeanafashion.eu/thesaurus/10543"/><rdfs:label xml:lang="de">Fransen</rdfs:label><rdfs:label xml:lang="fr">frange</rdfs:label><rdfs:label xml:lang="it">frangia</rdfs:label><rdfs:label xml:lang="nl">franje</rdfs:label><rdfs:label xml:lang="sv">frans</rdfs:label><rdfs:label xml:lang="en">fringe</rdfs:label><rdfs:label xml:lang="sr">resa</rdfs:label><rdfs:label xml:lang="el">κρόσσι</rdfs:label><rdfs:label xml:lang="he">גדיל</rdfs:label><rdfs:label xml:lang="he">פרנז'</rdfs:label><skos:exactMatch rdf:resource="http://vocab.getty.edu/aat/300227830"/><skos:scopeNote xml:lang="en">Trimming consisting of long or short lengths of straight or twisted thread, cord, or tassel; often grouped or knotted in various designs. (AAT)</skos:scopeNote></owl:Class><owl:Class rdf:about="http://thesaurus.europeanafashion.eu/thesaurus/10929"><rdfs:subClassOf rdf:resource="http://thesaurus.europeanafashion.eu/thesaurus/10543"/><rdfs:label xml:lang="de">Seil</rdfs:label><rdfs:label xml:lang="it">corda</rdfs:label><rdfs:label xml:lang="fr">corde</rdfs:label><rdfs:label xml:lang="sr">konopac</rdfs:label><rdfs:label xml:lang="sv">rep</rdfs:label><rdfs:label xml:lang="en">rope</rdfs:label><rdfs:label xml:lang="nl">touw</rdfs:label><rdfs:label xml:lang="sr">uže</rdfs:label><rdfs:label xml:lang="el">σκοινί</rdfs:label><rdfs:label xml:lang="he">חבל</rdfs:label><skos:exactMatch rdf:resource="http://vocab.getty.edu/aat/300014248"/><skos:scopeNote xml:lang="en">Heavy cord, at least 1/4 inch in diameter, formed by twisting or braiding three to six yarns of natural or artificial fiber. In ancient Egypt, ropes were made from reeds or date palm fibers. Ancient ropes were also made from flax, grass, esparto grass, hemp, sisal, coir, cotton, jute, papyrus, and camel hair. Up to 1850, most ropes were made from hemp or sisal. After this point, abaca and agave became the fibers of choice. By the 1950s, synthetic fibers (nylon, rayon, saran, polyester, etc.) became predominant. Glass and metallic fibers have also been incorporated into ropes for added strength and resistance to fire and chemicals. (AAT)</skos:scopeNote></owl:Class><owl:Class rdf:about="http://thesaurus.europeanafashion.eu/thesaurus/10933"><rdfs:subClassOf rdf:resource="http://thesaurus.europeanafashion.eu/thesaurus/10595"/><rdfs:label xml:lang="de">Kunstperlen</rdfs:label><rdfs:label xml:lang="sr">imitacija bisera</rdfs:label><rdfs:label xml:lang="nl">imitatieparel</rdfs:label><rdfs:label xml:lang="fr">imitation de perle de culture</rdfs:label><rdfs:label xml:lang="en">imitation pearl</rdfs:label><rdfs:label xml:lang="it">imitazione di perla</rdfs:label><rdfs:label xml:lang="sv">konstgjord pärla</rdfs:label><rdfs:label xml:lang="el">απομίμηση πέρλας</rdfs:label><rdfs:label xml:lang="he">פנינת חיקוי</rdfs:label></owl:Class><owl:Class rdf:about="http://thesaurus.europeanafashion.eu/thesaurus/10911"><rdfs:subClassOf rdf:resource="http://thesaurus.europeanafashion.eu/thesaurus/10797"/><rdfs:label xml:lang="de">Stickgarn</rdfs:label><rdfs:label xml:lang="nl">borduurgaren</rdfs:label><rdfs:label xml:lang="sv">broderigarn</rdfs:label><rdfs:label xml:lang="en">embroidery yarn</rdfs:label><rdfs:label xml:lang="fr">fil à broder</rdfs:label><rdfs:label xml:lang="it">filo da ricamo</rdfs:label><rdfs:label xml:lang="sr">konac za vezenje</rdfs:label><rdfs:label xml:lang="el">κλωστή κεντήματος</rdfs:label><rdfs:label xml:lang="he">חוטי רקמה</rdfs:label></owl:Class><owl:Class rdf:about="http://thesaurus.europeanafashion.eu/thesaurus/11073"><rdfs:subClassOf rdf:resource="http://thesaurus.europeanafashion.eu/thesaurus/10929"/><rdfs:label xml:lang="de">Schnur</rdfs:label><rdfs:label xml:lang="fr">ficelle</rdfs:label><rdfs:label xml:lang="nl">koordje</rdfs:label><rdfs:label xml:lang="sv">snöre</rdfs:label><rdfs:label xml:lang="it">spago</rdfs:label><rdfs:label xml:lang="en">string (thin rope)</rdfs:label><rdfs:label xml:lang="sr">žica</rdfs:label><rdfs:label xml:lang="el">σπάγγος</rdfs:label><rdfs:label xml:lang="he">חוט</rdfs:label><skos:exactMatch rdf:resource="http://vocab.getty.edu/aat/300014249"/><skos:scopeNote xml:lang="en">Cord thicker than thread and thinner than rope. (AAT)</skos:scopeNote></owl:Class><owl:ObjectProperty rdf:about="http://www.people#marry"><rdf:type rdf:resource="http://www.w3.org/2002/07/owl#SymmetricProperty"/><rdfs:domain rdf:resource="http://www.people#People"/><rdfs:range rdf:resource="http://www.people#People"/></owl:ObjectProperty><owl:ObjectProperty rdf:about="http://www.people#parent_of"><owl:inverseOf rdf:resource="http://www.people#son_of"/><rdfs:domain rdf:resource="http://www.people#People"/><rdfs:range rdf:resource="http://www.people#People"/></owl:ObjectProperty><owl:ObjectProperty rdf:about="http://www.people#son_of"><rdfs:domain rdf:resource="http://www.people#People"/><rdfs:range rdf:resource="http://www.people#People"/></owl:ObjectProperty><owl:DatatypeProperty rdf:about="http://www.people#birth_year"><rdfs:domain rdf:resource="http://www.people#People"/><rdfs:range rdf:resource="http://www.w3.org/2001/XMLSchema#int"/></owl:DatatypeProperty><owl:DatatypeProperty rdf:about="http://www.people#death_year"><rdfs:domain rdf:resource="http://www.people#People"/><rdfs:range rdf:resource="http://www.w3.org/2001/XMLSchema#int"/></owl:DatatypeProperty><owl:Class rdf:about="http://www.people#Married"><owl:equivalentClass><owl:Restriction><owl:onProperty rdf:resource="http://www.people#marry"/><owl:someValuesFrom rdf:resource="http://www.people#People"/></owl:Restriction></owl:equivalentClass><rdfs:subClassOf rdf:resource="http://www.people#People"/></owl:Class><owl:Class rdf:about="http://www.people#Parents"><owl:equivalentClass><owl:Restriction><owl:onProperty rdf:resource="http://www.people#parent_of"/><owl:someValuesFrom rdf:resource="http://www.people#People"/></owl:Restriction></owl:equivalentClass><rdfs:subClassOf rdf:resource="http://www.people#People"/></owl:Class><owl:Class rdf:about="http://www.people#People"/><owl:Class rdf:about="http://www.people#Sons"><owl:equivalentClass><owl:Restriction><owl:onProperty rdf:resource="http://www.people#son_of"/><owl:someValuesFrom rdf:resource="http://www.people#People"/></owl:Restriction></owl:equivalentClass><rdfs:subClassOf rdf:resource="http://www.people#People"/></owl:Class><owl:NamedIndividual rdf:about="http://www.people#berengaria_navarra"><rdf:type rdf:resource="http://www.people#People"/><www:birth_year rdf:datatype="http://www.w3.org/2001/XMLSchema#decimal">1165</www:birth_year><www:death_year rdf:datatype="http://www.w3.org/2001/XMLSchema#decimal">1230</www:death_year></owl:NamedIndividual><owl:NamedIndividual rdf:about="http://www.people#bianca_castiglia"><rdf:type rdf:resource="http://www.people#People"/><www:birth_year rdf:datatype="http://www.w3.org/2001/XMLSchema#decimal">1188</www:birth_year><www:death_year rdf:datatype="http://www.w3.org/2001/XMLSchema#decimal">1252</www:death_year></owl:NamedIndividual><owl:NamedIndividual rdf:about="http://www.people#eleonora_aquitania"><rdf:type rdf:resource="http://www.people#People"/><www:birth_year rdf:datatype="http://www.w3.org/2001/XMLSchema#decimal">1122</www:birth_year><www:death_year rdf:datatype="http://www.w3.org/2001/XMLSchema#decimal">1204</www:death_year></owl:NamedIndividual><owl:NamedIndividual rdf:about="http://www.people#enrico_II"><rdf:type rdf:resource="http://www.people#People"/><www:marry rdf:resource="http://www.people#eleonora_aquitania"/></owl:NamedIndividual><owl:NamedIndividual rdf:about="http://www.people#enrico_giovane"><rdf:type rdf:resource="http://www.people#People"/><www:marry rdf:resource="http://www.people#margherita_francia"/><www:son_of rdf:resource="http://www.people#eleonora_aquitania"/><www:son_of rdf:resource="http://www.people#enrico_II"/></owl:NamedIndividual><owl:NamedIndividual rdf:about="http://www.people#giovanni"><rdf:type rdf:resource="http://www.people#People"/><www:marry rdf:resource="http://www.people#isabella_angouleme"/><www:marry rdf:resource="http://www.people#isabella_gloucester"/><www:son_of rdf:resource="http://www.people#eleonora_aquitania"/><www:son_of rdf:resource="http://www.people#enrico_II"/></owl:NamedIndividual><owl:NamedIndividual rdf:about="http://www.people#isabella_angouleme"><rdf:type rdf:resource="http://www.people#People"/><www:birth_year rdf:datatype="http://www.w3.org/2001/XMLSchema#decimal">1186</www:birth_year><www:death_year rdf:datatype="http://www.w3.org/2001/XMLSchema#decimal">1246</www:death_year></owl:NamedIndividual><owl:NamedIndividual rdf:about="http://www.people#isabella_gloucester"><rdf:type rdf:resource="http://www.people#People"/><www:birth_year rdf:datatype="http://www.w3.org/2001/XMLSchema#decimal">1173</www:birth_year><www:birth_year rdf:datatype="http://www.w3.org/2001/XMLSchema#decimal">1217</www:birth_year></owl:NamedIndividual><owl:NamedIndividual rdf:about="http://www.people#luigi"><rdf:type rdf:resource="http://www.people#People"/><www:marry rdf:resource="http://www.people#bianca_castiglia"/></owl:NamedIndividual><owl:NamedIndividual rdf:about="http://www.people#margherita_francia"><rdf:type rdf:resource="http://www.people#People"/><www:birth_year rdf:datatype="http://www.w3.org/2001/XMLSchema#decimal">1157</www:birth_year><www:death_year rdf:datatype="http://www.w3.org/2001/XMLSchema#decimal">1197</www:death_year></owl:NamedIndividual><owl:NamedIndividual rdf:about="http://www.people#riccardo_I"><rdf:type rdf:resource="http://www.people#People"/><www:marry rdf:resource="http://www.people#berengaria_navarra"/><www:son_of rdf:resource="http://www.people#eleonora_aquitania"/><www:son_of rdf:resource="http://www.people#enrico_II"/></owl:NamedIndividual></rdf:RDF>